\section{Convex Conjugate Calculus Rules}
\label{appendix_sec:convex_conjugate_calculus_rules}

In this section, we provide common calculus rules for convex conjugates.
These rules are useful for discussions in Appendix~\ref{appendix_sec:convex_conjugate_for_GLM_loss_functions} and Appendix~\ref{appendix_sec:safe_lower_bound_more_discussions}.
These calculus rules can be found in standard optimization textbooks such as~\cite{}.

\textbf{Separable Sum Rule:} 

Let $f(\bx) = \sum_{i=1}^n f_i(x_i)$, where $f_i: \mathbb{R} \rightarrow \mathbb{R}$ is convex for all $i$.

Then, the convex conjugate of $f$ is given by $f^*(\bmu) = \sum_{i=1}^n f_i^*(\mu_i)$.

\textbf{Scalar Multiplication Rule:} 

Let $f(\bx)$ and $g(\bx)$ be a convex function and $\alpha > 0$ be a scalar.

Then, the convex conjugate of $f(\bx) = \alpha g(\bx)$ is given by $f^*(\bmu) = \alpha g^*(\bmu/\alpha)$.


% The convex conjugate of $f(\bx) = \alpha g(\bx / \balpha)$ is given by $f^*(\bmu) = \alpha g^*(\bmu)$

\textbf{Addition to Affine Function Rule:} 

Let $f(\bx)$ and $g(\bx)$ be a convex function and $\ba, \bb \in \mathbb{R}^n$ be two vectors.

Then, the convex conjugate of $f(\bx) = g(\bx) + \ba^T\bx + b$ is given by $f^*(\bmu) = g^*(\bmu - \ba) - \bb$.

% The convex conjugate of $f(\bx) = g(\bx - \ba) - \by$ is given by $f^*(\bmu) = g^*(\bmu) + \ba^T\bmu + \by$.

\textbf{Composition with Invertible Linear Mapping Rule:} 

Let $f(\bx)$ and $g(\bx)$ be a convex function and $\bA \in \mathbb{R}^{n \times n}$ be an invertible matrix.

Then, the convex conjugate of $f(\bx) = g(\bA \bx)$ is given by $f^*(\bmu) = g^*(\bA^{-T} \bmu)$.

\textbf{Infimal Convolution Rule:} 

Let $f(\bx)$, $g(\bx)$, and $h(\bx)$ be a convex function.

Then, the convex conjugate of $f(\bx) = \inf_{\by} \{g(\by) + h(\bx - \by)\}$ is given by $f^*(\bmu) = g^*(\bmu) + h^*(\bmu)$.
