\begin{table}[h]
    \caption{Convex Conjugates of GLM Loss Functions}
    \label{table:convex_conjugates_glm_loss_functions}
    \centering
    \begin{tabular}{>{\centering\arraybackslash}p{0.2\textwidth}>{\centering\arraybackslash}p{0.7\textwidth}}
        \hline
        \addlinespace[0.3cm]
        \multirow{2}{*}{\centering Linear Regression} & $F(\bX \bbeta) = \Vert{\bX \bbeta - \by}_2^2$ \\[0.2cm]
        & $F^*(-\bzeta) = \frac{1}{4} \Vert{\bzeta}_2^2 - \by^T \bzeta$ \\
        \addlinespace[0.3cm]
        \hline
        \addlinespace[0.3cm]
        \multirow{2}{*}{\centering Logistic Regression} & $F(\bX \bbeta) = \sum_{i=1}^n \log(1 + \exp(-y_i (\bX \bbeta)_i))$ \\[0.2cm]
        & $F^*(-\bzeta) = \sum_{i=1}^n \left( 1- \frac{\zeta_i}{y_i} \right) \log \left( 1-\frac{\zeta_i}{y_i} \right) + \frac{\zeta_i}{y_i} \log \left( \frac{\zeta_i}{y_i} \right)$ \\
        \addlinespace[0.3cm]
        \hline
        \addlinespace[0.3cm]
        \multirow{2}{*}{\centering Poisson Regression} & $F(\bX \bbeta) = \sum_{i=1}^n \left( (\bX \bbeta)_i - y_i \log((\bX \bbeta)_i) \right)$ \\[0.2cm]
        & $F^*(-\bzeta) = \sum_{i=1}^n \left( \exp(\zeta_i) - 1 \right)$ \\
        \addlinespace[0.3cm]
        \hline
    \end{tabular}
\end{table}