\section{Auxiliary Technical Lemmas}\label{ab_sec:aux}
\begin{lemma}\label{lem:tech_res_1}
Let $A$ and $A'$ be two bounded operators from $\mathcal{H}$ to $\mathbb{R}^d$, and $B$ and $B'$ be two bounded and invertible operators from $\mathcal{H}$ to itself. Assume that $B\geq \lambda\Id_{\mathcal{H}}$ and $B'\geq \lambda\Id_{\mathcal{H}}$. 
Then, the following inequalities hold:
\begin{gather*}
    \Verts{AB^{-1}-A'(B')^{-1}}_{\op} \leq \frac{\Verts{A}_{\op}}{\lambda^2}\Verts{B-B'}_{\op} + \frac{1}{\lambda}\Verts{A-A'}_{\op},\\
    \Verts{AB^{-1}}_{\op}\leq \lambda^{-1}\Verts{A}_{\op}, \qquad\Verts{A'(B')^{-1}}_{\op}\leq \lambda^{-1}\Verts{A'}_{\op}.
\end{gather*}
\end{lemma}

\begin{proof}
By the triangle inequality and the sub-multiplicative property of the operator norm $\|\cdot\|_{\op}$, we have:
\begin{align}
    \Verts{AB^{-1}-A'(B')^{-1}}_{\op}&\leq\left\|AB^{-1} - A(B')^{-1}\right\|_{\op}+\left\|A(B')^{-1} - A'(B')^{-1}\right\|_{\op}\nonumber\\
    &\leq\left\|A\left(B^{-1} - (B')^{-1}\right)\right\|_{\op}+\left\|\left(A - A'\right)(B')^{-1}\right\|_{\op}\nonumber\\
    &\leq\left\|A\right\|_{\op}\left\|B^{-1} - (B')^{-1}\right\|_{\op}+\left\|A-A'\right\|_{\op}\left\|(B')^{-1}\right\|_{\op}\nonumber\\
    &\leq\left\|A\right\|_{\op}\left\|B^{-1}\left(B'-B\right) (B')^{-1}\right\|_{\op}+\left\|A-A'\right\|_{\op}\left\|(B')^{-1}\right\|_{\op}\nonumber\\
    &\leq\left\|A\right\|_{\op}\left\|B^{-1}\right\|_{\op}\left\|B'-B\right\|_{\op}\left\|(B')^{-1}\right\|_{\op}+\left\|A-A'\right\|_{\op}\left\|(B')^{-1}\right\|_{\op}.
    \label{eq:technical_proof_1}
\end{align}
Since $B\geq \lambda\Id_{\mathcal{H}}$ and $B'\geq \lambda\Id_{\mathcal{H}}$, we obtain:
\begin{equation*}
    \left\|B^{-1}\right\|_{\op}\leq\frac{1}{\lambda}\quad\text{and}\quad\left\|(B')^{-1}\right\|_{\op}\leq\frac{1}{\lambda}.
\end{equation*}
Substituting these into \cref{eq:technical_proof_1}, we get:
\begin{align*}
    \Verts{AB^{-1}-A'(B')^{-1}}_{\op}\leq\frac{\Verts{A}_{\op}}{\lambda^2}\Verts{B-B'}_{\op} + \frac{1}{\lambda}\Verts{A-A'}_{\op}.
\end{align*}
This proves the first inequality. The remaining two inequalities follow directly from the sub-multiplicative property of the operator norm $\|\cdot\|_{\op}$ and the assumptions $B\geq \lambda\Id_{\mathcal{H}}$ and $B'\geq \lambda\Id_{\mathcal{H}}$.
\end{proof}


\begin{lemma}\label{lem:h_min_hstar}
Let $f:\mathcal{H}\to\mathbb{R}$ be a $\lambda$-strongly convex and Fr\'echet differentiable function. Denote by $h^\star\in\mathcal{H}$ its minimizer. Then, for any $h\in\mathcal{H}$, the following holds:
\begin{equation*}
    \left\|h-h^\star\right\|_\mathcal{H}\leq\frac{1}{\lambda}\left\|\partial_h f(h)\right\|_\mathcal{H}.
\end{equation*}
\end{lemma}

\begin{proof}
Let $h\in\mathcal{H}$. 

\textbf{Case 1: $h=h^\star$. }The proof is straightforward.

\textbf{Case 2: $h\neq h^\star$. }Given that $f$ is $\lambda$-strongly convex, we have:
\begin{align*}
    f(h)-f(h^\star)&\geq\left\langle\partial_h f(h^\star),h-h^\star\right\rangle_\mathcal{H}+\frac{\lambda}{2}\left\|h-h^\star\right\|_\mathcal{H}^2,\\
    \text{and }f(h^\star)-f(h)&\geq\left\langle\partial_h f(h),h^\star-h\right\rangle_\mathcal{H}+\frac{\lambda}{2}\left\|h-h^\star\right\|_\mathcal{H}^2.
\end{align*}
After summing these two inequalities, noticing that $\partial_h f(h^\star)=0$, and rearranging the terms, we obtain:
\begin{equation*}
    \left\langle\partial_h f(h),h-h^\star\right\rangle_\mathcal{H}\geq\lambda\left\|h-h^\star\right\|_\mathcal{H}^2.
\end{equation*}
After using the Cauchy-Schwarz inequality, we get:
\begin{equation*}
    \left\|\partial_h f(h)\right\|_\mathcal{H}\left\|h-h^\star\right\|_\mathcal{H}\geq\lambda\left\|h-h^\star\right\|_\mathcal{H}^2.
\end{equation*}
Dividing by $\lambda\left\|h-h^\star\right\|_\mathcal{H}\neq0$ concludes the proof.
\end{proof}


\begin{lemma}\label{lem:hs_identity}
{
Let $\mathcal{X}$ be a subset of $\mathbb{R}^p$, $\mathcal{Y}$ be a subset of $\mathbb{R}^q$, and $\mathbb{D}$ be a probability distribution over $\mathcal{X}\times\mathcal{Y}$. Given i.i.d. samples $(x_i,y_i)_{1\leq i\leq n}$ drawn from $\mathbb{D}$, consider a function $g:\mathcal{X}\times\mathcal{Y}\to\mathbb{R}$ of class $C^1$ such that the operator $A:\mathcal{H}\to\mathcal{H}$ defined as:
\begin{equation*}
    A\coloneqq\mathbb{E}_{(x,y)\sim\mathbb{D}}\brackets{g(x,y)K(x,\cdot)\otimes K(x,\cdot)}-\frac{1}{n}\sum_{i=1}^n g(x_i,y_i)K(x_i,\cdot)\otimes K(x_i,\cdot)
\end{equation*}
is Hilbert-Schmidt. Then, the following holds:
\begin{align*}
    \Verts{A}_{\hs}^2=&\mathbb{E}_{(x,y),(x',y')\sim\mathbb{D}\otimes\mathbb{D}}\Big[g(x,y)g(x',y')K^2(x,x')\Big]+\frac{1}{n^2}\sum_{i,j=1}^n g(x_i, y_i)g(x_j, y_j)K^2(x_i,x_j)\\
    &-\frac{2}{n}\sum_{i=1}^n\mathbb{E}_{(x,y)\sim\mathbb{D}}\Big[g(x_i, y_i)g(x, y)K^2(x,x_i)\Big].
\end{align*}
}
\end{lemma}

\begin{proof}
{
Define $s\coloneqq\mathbb{E}_{(x,y)\sim\mathbb{D}}\left[g(x,y)K(x,\cdot)\otimes K(x,\cdot)\right]$ and $\hat{s}\coloneqq\frac{1}{n}\sum_{i=1}^n g(x_i,y_i)K(x_i,\cdot)\otimes K(x_i,\cdot)$. We have:
\begin{equation}\label{eq:A}
    \Verts{A}_{\hs}^2=\Verts{s-\hat{s}}_{\hs}^2=\Verts{s}_{\hs}^2+\Verts{\hat{s}}_{\hs}^2-2\left\langle s,\hat{s}\right\rangle_{\hs}.
\end{equation}
Next, we compute each of the following quantities: $\Verts{s}_{\hs}^2$, $\Verts{\hat{s}}_{\hs}^2$, and $\left\langle s,\hat{s}\right\rangle_{\hs}$, separately. Simple calculations yield:
\begin{align*}
    \Verts{s}_{\hs}^2&=\left\|\mathbb{E}_{(x,y)\sim\mathbb{D}}\left[g(x,y)K(x,\cdot)\otimes K(x,\cdot)\right]\right\|_{\hs}^2\\
    &=\left\langle\mathbb{E}_{(x,y)\sim\mathbb{D}}\left[g(x,y)K(x,\cdot)\otimes K(x,\cdot)\right],\mathbb{E}_{(x',y')\sim\mathbb{D}}\left[g(x',y')K(x',\cdot)\otimes K(x',\cdot)\right]\right\rangle_{\hs}\\
    &=\mathbb{E}_{(x,y),(x',y')\sim\mathbb{D}\otimes\mathbb{D}}\bigg[g(x,y)g(x',y')\left\langle K(x,\cdot)\otimes K(x,\cdot),K(x',\cdot)\otimes K(x',\cdot)\right\rangle_{\hs}\bigg]\\
    &=\mathbb{E}_{(x,y),(x',y')\sim\mathbb{D}\otimes\mathbb{D}}\Big[g(x,y)g(x',y')K^2(x,x')\Big],\\
    \Verts{\hat{s}}_{\hs}^2&=\frac{1}{n^2}\left\|\sum_{i=1}^n g(x_i, y_i)K(x_i,\cdot)\otimes K(x_i,\cdot)\right\|_{\hs}^2\\
    &=\frac{1}{n^2}\left\langle\sum_{i=1}^n g(x_i, y_i)K(x_i,\cdot)\otimes K(x_i,\cdot),\sum_{j=1}^n g(x_j, y_j)K(x_j,\cdot)\otimes K(x_j,\cdot)\right\rangle_{\hs}\\
    &=\frac{1}{n^2}\sum_{i,j=1}^n\partial_v^2 g(x_i, y_i)g(x_j, y_j)\left\langle K(x_i,\cdot)\otimes K(x_i,\cdot),K(x_j,\cdot)\otimes K(x_j,\cdot)\right\rangle_{\hs}\\
    &=\frac{1}{n^2}\sum_{i,j=1}^n g(x_i, y_i)g(x_j, y_j)K^2(x_i,x_j),\\
    \left\langle s,\hat{s}\right\rangle_{\hs}&=\left\langle\mathbb{E}_{(x,y)\sim\mathbb{D}}\left[g(x, y)K(x,\cdot)\otimes K(x,\cdot)\right],\frac{1}{n}\sum_{i=1}^n g(x_i, y_i)K(x_i,\cdot)\otimes K(x_i,\cdot)\right\rangle_{\hs}\\
    &=\frac{1}{n}\sum_{i=1}^n\mathbb{E}_{(x,y)\sim\mathbb{D}}\left[g(x_i, y_i)g(x, y)\left\langle K(x,\cdot)\otimes K(x,\cdot),K(x_i,\cdot)\otimes K(x_i,\cdot)\right\rangle_{\hs}\right]\\
    &=\frac{1}{n}\sum_{i=1}^n\mathbb{E}_{(x,y)\sim\mathbb{D}}\Big[g(x_i, y_i)g(x, y)K^2(x,x_i)\Big].
\end{align*}
After substituting the obtained results into \cref{eq:A} and rearranging, we obtain:
\begin{align*}
    \left\|A\right\|_{\hs}^2=&\mathbb{E}_{(x,y),(x',y')\sim\mathbb{D}\otimes\mathbb{D}}\Big[g(x,y)g(x',y')K^2(x,x')\Big]+\frac{1}{n^2}\sum_{i,j=1}^n g(x_i, y_i)g(x_j, y_j)K^2(x_i,x_j)\\
    &-\frac{2}{n}\sum_{i=1}^n\mathbb{E}_{(x,y)\sim\mathbb{D}}\Big[g(x_i, y_i)g(x, y)K^2(x,x_i)\Big].
\end{align*}
}
\end{proof}