\section{Useful Definitions and Lemmas}
We list some useful definitions and lemmas here. 

\begin{lemma}[Freedman's Inequality]  
Fix any \(\lambda>0\) and \(\delta \in(0,1)\). Let \(X_t\) be a random process with respect to a filtration \(\mathcal{F}_t\) such that \(\mu_t = \mathbb{E}\left[X_t \mid \mathcal{F}_{t-1}\right]\) and \(V_t = \mathbb{E}\left[X_t^2 \mid \mathcal{F}_{t-1}\right]\), and satisfying \(\lambda X_t \le 1\). Then, with probability at least \(1-\delta\), we have for all \(t\),  
$$  
\sum_{s=1}^t X_s - \mu_s \le \lambda \sum_{s=1}^t V_s + \frac{\log(1 / \delta)}{\lambda}.  
$$  
\end{lemma}

\begin{lemma}[Lemma 5, \citet{GraphAlon15} ]
\label{lem: graph_inverse}
Let $G=(V, E)$ be a directed graph with $|V|=K$, in which each node $i \in V$ is assigned a positive weight $w_i$. Assume that $\sum_{i \in V} w_i \le 1$, and that $w_i \geq \epsilon$ for all $i \in V$ for some constant $0<\epsilon<\frac{1}{2}$. Then
$$
\sum_{i \in V} \frac{w_i}{w_i+\sum_{j \in N^{\operatorname{in}(i)}} w_j} \le 4 \alpha \ln \frac{4 K}{\alpha \epsilon}
$$

where $\alpha=\alpha(G)$ is the independence number of $H$.
\end{lemma}

\begin{lemma}[Lemma 11, \citet{Sch23}]
\label{lem: exp3 update}
Let $z\in[-\frac{1}{2},\frac{1}{2}]^K$, $x\in\Delta([K])$ and $\widetilde x\propto x\circ\exp(z)$. Then for all $k\in[K]$:
\begin{align*}
    x_k \exp(z_k - 2\ip{x,|z|})\le \widetilde x_k \le x_k \exp(z_k + \ip{x,|z|})\,.
\end{align*}
\end{lemma}

We now extend several lemmas in \citet{Sch23} to the graphical feedback setting. 
%
The proofs of our lemmas are similar to those of the lemmas in ~\citet{Sch23}.
%
This is because these lemmas are all about the concentration of the empirical importance $\widehat{w}_e(a)$. 
%
Although our empirical importance 
\[\widehat{w}_e(a) = \frac{2}{L} \sum_{t \in \Time_{e-1}^f}  \frac{s_{e,c_t}(\NodeIn(a))}{2}\] is different from the empirical importance in ~\citet{Sch23} \[\widehat{w}_e(a) =  \frac{2}{L} \sum_{t \in \Time_{e-1}^f}  \frac{s_{e,c_t}(a)}{2},\] both of them are estimating the expected importance $w_e(a)$ in essentially the same way, thus sharing the same concentration properties.
%
Readers familiar with \citet{Sch23} can just read the statements and skip these proofs safely. Here we write these proofs down for the sake of completeness.

We first define the following sequences of indicator variables. Each sequence of indicator variables represents a special type of concentration.

\begin{definition}
For each epoch $e$, we define the following two indicator variables:
\[F_e \triangleq \indi\left(\forall a,\left|\widehat{w}_e(a)-w_e(a)\right| \le 2 \max \left\{\sqrt{\frac{w_e(a) \iota}{L}}, \frac{\iota}{L}\right\}\right)\]
and 
\[L_e \triangleq \indi\left(\max _{c \in[M], a \in[K]} \sum_{t \in \Time_e} \widetilde{\ell}_{t,c}(a) \le L+\frac{\iota}{\gamma}\right).\]
\end{definition}

The first sequence of indicator variables $\{ F_e\}$ represents the concentration of our empirical importance $\widehat{w}_e(a)$ around the expected importance $w_e(a)$. The second sequence of indicator variables $\{ L_e\}$ represents that the pseudo loss estimates $\widetilde{\ell}$ are not too large. Given these sequences of indicator variables, we have the following lemmas.

\begin{lemma}[Extension of Lemma 6 in \citet{Sch23}]
\label{lem: indicator_F}
    For any $e \in[T / L], e>1$, event $F_e$ holds with probability at least $1-2 K \exp (-\iota)$.
\end{lemma}
\begin{proof}
Fix an arm $a \in [K]$. Consider a random variable $X$ defined via $X = s_{e, c}(\NodeIn(a))$ where $c \sim \nu$ (so $\E[X] = w_{e}(a)$). Note that $\widehat{w}_{e}(a)$ is distributed according to $\sum_{i=1}^{L/2}\frac{X_i}{L/2}$, where the $X_i$ are i.i.d. copies of $X$. Then $\sum_{i=1}^{L/2}\E[(X_i-w_{e}(a))^2]\le \frac{L}{2}\cdot \frac{w_{e}(a)}{2}$, since $(X_i-w_{e}(a))\in[-1/2,1/2]$.

Now, for any $\zeta\le 2$, we have by Bernstein's inequality with probability at least $1-\exp(-\iota)$
\begin{align*}
    \sum_{i=1}^{L/2} \frac{X_i}{L/2} - w_{e}(a) < \frac{\zeta w_{e}(a)}{2}+\frac{2\iota}{\zeta L}\,. 
\end{align*}
Set $\zeta = \min\left\{2,2\sqrt{\frac{\iota}{w_{e}(a)L}}\right\}$, which shows that with probability at least $1-\exp(-\iota)$
\begin{align*}
    \widehat{w}_{e}(a)-w_{e}(a) \le 2\max\left\{\sqrt{\frac{w_{e}(a)\iota}{L}},\frac{\iota}{L}\right\}\,.
\end{align*}
Repeating the same argument for $\sum_i-X_i$ and taking a union bound completes the proof.
\end{proof}

\begin{lemma}[Extension of Lemma 7 in \citet{Sch23}]
\label{lem: indicator_L}

    For any $e \in[T / L], e>1$, event $L_e$ holds with probability at least $1-K \exp (-\iota)$.
\end{lemma}
\begin{proof}
We have
\begin{align*}
    \max_{c\in[M]}\sum_{t\in T_e}\widetilde{\ell}_{t,c}(a)\le \sum_{t\in \Time_e} \frac{2\indi(A_t = a,S_t=1,t \in \Time_{e}^{\ell})/w_{e}(a)}{1+\gamma/w_{e}(a)}\,.
\end{align*}

Applying Bernstein's inequality on the summation \[\sum_{t\in \Time_e} \frac{2\indi(A_t = a,S_t=1,t \in \Time_{e}^{\ell})/w_{e}(a)}{1+\gamma/w_{e}(a)}\] proves that
\begin{align*}
    \sum_{t\in\Time_e}\widetilde{\ell}_t \le L +\frac{\iota}{\gamma}\,.
\end{align*}
Taking a union bound over $a \in [K]$ completes the proof.
\end{proof}

Given these two lemmas, we define another indicator variable.

\begin{definition}
Let $Q$ be the indicator of the event that all previous events $w_e$ and $L_e$ hold
\[Q = \prod_e w_e L_e.\]
\end{definition}

By the previous two lemmas, it is easy to see that $\Pr(Q) \ge 1 - 3 K(T / L) \exp (-\iota)$.

For each epoch $e$ and arm $a$, we consider the following ratio
\[\beta_e(a) = \frac{w_e(a) + \gamma}{\widehat{w}_e(a) + \frac{3}{2} \gamma}.\]
For this ratio, we have the following lemma.

\begin{lemma}[Extensions of Lemma 8 in \citet{Sch23}]
\label{lem: beta_concentration}
Let $\gamma \geq \frac{4 \iota}{L}$, then under event $Q$, for all $t \in \Time_e, a \in[K]$, we have that
$$
\frac{1}{2} \le \beta_{e}(a) \le 2
$$
and
$$
\left|1-\beta_e(a)\right| \le 3 \sqrt{\frac{\iota}{w_{e}(a) L}}+\frac{\gamma \sqrt{L}}{4 \sqrt{\iota w_{e}(a)}}. 
$$
\end{lemma}

\begin{proof}
The first statement is equivalent to showing that $\frac{1}{\beta_{e}(a)}-1 \in [-\frac{1}{2},1]$.
Using the facts that $2\max\left\{\sqrt{\frac{w_{e}(a)\iota}{L}},\frac{2\iota}{L}\right\}\le \frac{w_e(a)}{2}+\frac{2\iota}{L}$, $F_e = 1$ and $\gamma\geq \frac{4\iota}{L}$, we have
\begin{align*}
    &\frac{1}{\beta_{e}(a)}-1 = \frac{\widehat{w}_{e}(a)-w_{e}(a)+\frac{1}{2}\gamma}{w_e(a)+\gamma}\geq \frac{-\frac{1}{2}w_e(a)-\frac{2\iota}{L}+\frac{1}{2}\gamma}{w_e(a)+\gamma}\geq -\frac{1}{2}\\
    &\frac{1}{\beta_{e}(a)}-1 = \frac{\widehat{w}_{e}(a)-w_{e}(a)+\frac{1}{2}\gamma}{w_e(a)+\gamma}\le \frac{w_e(a)+\frac{2\iota}{L}+\frac{1}{2}\gamma}{w_e(a)+\gamma}\le 1\,,
\end{align*}
which proves that $\beta_{e}(a)\in[1/2,2]$.
If $w_{e}(a)\le \frac{\iota}{L}$, then the second condition follows directly from the first. Otherwise we have
\begin{align*}
    &\beta_{e}(a)-1 \le \frac{ 2\sqrt{\frac{w_{e}(a)\iota}{L}}-\frac{1}{2}\gamma}{w_{e}(a)-2\sqrt{\frac{w_{e}(a)\iota}{L}}+\frac{3}{2}\gamma} \le \frac{ 2\sqrt{\frac{w_{e}(a)\iota}{L}}}{w_{e}(a)-2\sqrt{\frac{w_{e}(a)\iota}{L}}+2\gamma}\le \frac{ 4\sqrt{\frac{w_{e}(a)\iota}{L}}}{\frac{7}{8}w_{e}(a)}\le 3\sqrt{\frac{\iota}{w_{e}(a)L}}\\
    &1-\beta_{e}(a) \le \frac{ 2\sqrt{\frac{w_{e}(a)\iota}{L}}+\frac{1}{2}\gamma}{w_{e}(a)+2\sqrt{\frac{w_{e}(a)\iota}{L}}+\frac{3}{2}\gamma} \le \sqrt{\frac{\iota}{w_{e}(a)L}}+\frac{\gamma\sqrt{L}}{4\sqrt{\iota w_{e}(a)}}\,.
\end{align*}
\end{proof}

Let $p_t(a)$ denote $\E_{c \sim \nu}\left[p_{t,c}(a)\right]$ and $\widetilde{p}_t(a)$ denote $\E_{c \sim \nu}\left[\widetilde{p}_{t,c}(a)\right]$. We have the following lemma.

\begin{lemma}[Extension of Lemma 9 in \citet{Sch23}]
\label{lem:s_smaller_p_smaller_2s}
    If $\gamma \geq \frac{4 \iota}{L}$ and $\eta \le \frac{\log (2)}{5 L}$, then under event $Q$, we have for all $t \in \Time_e, a \in[K], c \in[M]$ simultaneously

$$
2 s_{e,c}(a) \geq p_{t,c}(a) \geq s_{e,c}(a) / 2 \quad \text { and } \quad 2 s_{e,c}(a) \geq \widetilde{p}_{t,c}(a) \geq s_{e,c}(a) / 2
$$


This implies that

$$
\E_{c \sim \nu}\left[p_{t,c}(a)\right] \le 4 w_{e}(a) \quad \text { and } \quad \E_{c \sim \nu}\left[\widetilde{p}_{t,c}(a)\right] \le 4 w_{e}(a)
$$
In addition, this implies that $q_t=p_t$ for all $t \in \Time_e$.

\end{lemma}
\begin{proof}
We have that $p_{t,c}(a) \propto \exp(-\eta(\sum_{t'\in\Time^{\ell}_{e-1} \cup \Time^{\ell}_e,t'<t} \widehat{\ell}_{t',c}(a))) s_{e,c}(a)$, and $\widetilde{p}_{t,c}(a) \propto \exp( -\eta( \sum_{t'\in\Time^{\ell}_{e-1}} \widehat{\ell}_{t',c}(a) + \sum_{t'\in\Time^{\ell}_e,t'<t} \widetilde{\ell}_{t',c}))s_{e,c}(a)$.
By definition, $Q=1$ implies that $L_{e-1}=L_e=1$. Hence for any $a\in[K],c\in[M]$,
\begin{align*}
    \sum_{t'\in\Time^{\ell}_{e-1}\cup\Time^{\ell}_{e}}\widetilde{\ell}_{t,c}(a) \le 2(L+\frac{\iota}{\gamma} )\le \frac{5}{2}L\,.
\end{align*}
Furthermore, by \Cref{lem: beta_concentration}, we can bound sums of $\widehat{\ell}$ via
\begin{align*}
    &\sum_{t'\in\Time^{\ell}_{e-1}\cup\Time^{\ell}_{e}}\widehat{\ell}_{t,c}(a) =\sum_{t'\in\Time^{\ell}_{e-1}}\beta_{e-1,k}\widetilde{\ell}_{t,c}(a)+\sum_{t'\in\Time^{\ell}_{e}}\beta_{e}(a)\widetilde{\ell}_{t,c}(a) \le 5L\\
    &\sum_{t'\in\Time^{\ell}_{e-1}}\widehat{\ell}_{t,c}(a)+\sum_{t'\in\Time^{\ell}_{e}}\widetilde{\ell}_{t,c}(a) \le 5L\,.
\end{align*}

Finally, this implies for any $a \in [K]$ that
\begin{align*}
    \exp\left(-5\eta L \right)s_{e}(a)\le p_{t,c}(a)\le \exp\left(5\eta L\right) s_{e}(a)
\end{align*}
and for $\widetilde{p}_{t,c}(a)$ accordingly.
Using $\eta\le \frac{\log(2)}{5L}$ completes the first part of the proof.
The second statement follows directly from the definition of $w_{e}(a)$. Finally, the last statement follows from the definition of $q_t$ since $q_{tc} = p_{tc}$ whenever $p_{t,c}(a) \geq s_{e,c}(a)/2$ for all $a \in[K]$. 
\end{proof}

In following analysis, let $\E_e[X]$ denote $\E\left[ X | s_e \right]$ for any random variable $X$.

\begin{lemma}[Extension of Lemma 10 \citet{Sch23}]
\label{lem: bounding_1_minus_beta}
If $\gamma \geq \frac{16 \iota}{L}$ and $\exp (-\iota) \le \frac{\gamma}{8 K}$, then

$$
0 \le \E_e\left[\left(1-\beta_e(a)\right) F_e\right] \le \frac{\gamma}{w_{e}(a)}
$$

\end{lemma}
\begin{proof}
Since $F_e\in\{0,1\}$, we have
\begin{align*}
    (1-\beta_{e}(a))F_e = \left(1-\frac{w_{e}(a)+\gamma}{\widehat{w}_{e}(a)+\frac{3}{2}\gamma}\right)F_e = \frac{(\widehat{w}_{e}(a)-w_{e}(a))F_e +\frac{1}{2}\gamma}{w_{e}(a)+(\widehat{w}_{e}(a)-w_{e}(a))F_e+\frac{3}{2}\gamma} - (1-F_e)\frac{\gamma}{2w_{e}(a)+3\gamma}\,.
\end{align*}
The second term is in expectation bounded by
\begin{align*}
    \E_{e}\left[(1-F_e)\frac{\gamma}{2w_{e}(a)+3\gamma}\right]
    \le 2K\exp(-\iota)\frac{\gamma}{2w_{e}(a)+3\gamma}\le \frac{\gamma^2}{4(2w_{e}(a)+3\gamma)}\,.
\end{align*}
It remains to bound the first term. Denote $C_{e}(a)=2\max\{\sqrt{\frac{w_{e}(a)\iota}{L}},\frac{\iota}{L}\}$. The random variable $(\widehat{w}_{e}(a)-w_{e}(a))F_e$ is bounded in $\{-C_{e}(a),C_{e}(a)\}$ due to the indicator $F_e$.
Let $\mu=\E_{e}[(\widehat{w}_{e}(a)-w_{e}(a))F_e]$ and assume for now that $\mu\in[-\frac{1}{4}\gamma,\frac{1}{4}\gamma]$ which we show later. By Jensen's inequality we have
\begin{align*}
    \E_{e}\left[\frac{(\widehat{w}_{e}(a)-w_{e}(a))F_e +\frac{1}{2}\gamma}{w_{e}(a)+(\widehat{w}_{e}(a)-w_{e}(a))F_e+\frac{3}{2}\gamma}\right] \le \frac{\mu+\frac{1}{2}\gamma}{w_{e}(a)+\mu+\frac{3}{2}\gamma}\le \frac{\gamma}{w_{e}(a)}\,.
\end{align*}
On the other hand, again due to convexity, the smallest expected value is obtained for the distribution that takes values in $\{-C_{e}(a),C_{e}(a)\}$ such that it conforms with mean $\mu$. Hence

\begin{align*}
    \E_{e}\left[\frac{(\widehat{w}_{e}(a)-w_{e}(a))F_e +\frac{1}{2}\gamma}{w_{e}(a)+(\widehat{w}_{e}(a)-w_{e}(a))F_e+\frac{3}{2}\gamma}\right] &\geq \left(\frac{C_{e}(a)+\mu}{2C_{e}(a)}\right)\frac{C_{e}(a)+\frac{1}{2}\gamma}{w_{e}(a)+C_{e}(a)+\frac{3}{2}\gamma}+\left(\frac{C_{e}(a)-\mu}{2C_{e}(a)}\right)\frac{-C_{e}(a)+\frac{1}{2}\gamma}{w_{e}(a)-C_{e}(a)+\frac{3}{2}\gamma}\\
    &=\frac{(w_{e}(a)+\frac{3}{2}\gamma)(\gamma+2\mu)-(\gamma\mu+2C_{e}(a)^2)}{2(w_{e}(a)+C_{e}(a)+\frac{3}{2}\gamma)(w_{e}(a)-C_{e}(a)+\frac{3}{2}\gamma)}\\
    &\geq\frac{\frac{1}{2}\gamma w_{e}(a)+\gamma^2-2C_{e}(a)^2}{2(w_{e}(a)+\frac{3}{2}\gamma)^2-2C_{e}(a)^2}\geq \frac{\frac{1}{2}\gamma^2}{2(w_{e}(a)+\frac{3}{2})^2}\,,
\end{align*}
where the last inequality uses the fact that  $\frac{1}{2}\gamma w_{e}(a)+\frac{1}{2}\gamma^2\geq 2C_{e}(a)^2$, since $\gamma\geq \frac{16\iota}{L}$\,.

Finally we need to verify $\mu\in[-\frac{\gamma}{2},\frac{\gamma}{2}]$.
We begin by bounding the expectation of $\E_{e}\left[(\widehat{w}_{e}(a)-w_{e}(a))(1-F_e)\right]$.
By construction $\widehat{w}_{e}(a)-w_{e}(a)\in[-\frac{1}{2},\frac{1}{2}]$ and $E_{e}[(1-F_e)]\le 2K\exp(-\iota)\le \gamma/2$. Hence
due to $\E_{e}[\widehat{w}_{e}(a)-w_{e}(a)]=0$, we have
$\mu = - \E_{e}\left[(\widehat{w}_{e}(a)-w_{e}(a))(1-F_e)\right]\in[-\frac{\gamma}{4},\frac{\gamma}{4}]$.
\end{proof}

\begin{lemma}[Extension of Lemma 12 in \citet{Sch23}]
\label{lem: pure_concentration}
 Assume $\eta \le \frac{\gamma}{2(2 L \gamma+\iota)}$. Then under event $Q$, for all $t \in \Time_e$ and $c \in \mathcal{C}$, we have that

$$
\sum_{a=1}^K\left|\widetilde{p}_{t,c}(a)-p_{t,c}(a)\right| \cdot\left|1-\beta_{e}(a)\right| \le 3 \sum_{a=1}^K \widetilde{p}_{t, c}(a)\left(1-\beta_{e}(a)\right)^2
$$
\begin{proof}
By definition, $p_{t,c}(a)\propto \widetilde{p}_{t,c}(a)\exp(-\eta\sum_{t'\in T_e,t'<t}(\widehat{\ell}_{t,c}(a)-\widetilde{\ell}_{t,c}(a)))$.
We can simplify the argument of the exponential via
\begin{align*}
    -\sum_{t'\in T_e,t'<t}(\widehat{\ell}_{t',c}(a)-\widetilde{\ell}_{t',c}(a)))=(1-\beta_{e}(a))\sum_{t'\in T_e,t'<t}\widetilde{\ell}_{t',c}(a).
\end{align*}
By \Cref{lem: beta_concentration} and the definition of $L_e$, we have
\begin{align*}
    \eta\left|\sum_{t'\in T_e,t'<t}(\widehat{\ell}_{t',c}(a)-\widetilde{\ell}_{t',c}(a))\right|=\eta(1-\beta_{e}(a))\sum_{t'\in T_e,t'<t}\widetilde{\ell}_{t',c}(a) \le \eta(L+\frac{\iota}{2\gamma}) \le \frac{1}{2}\,.
\end{align*}
\Cref{lem: exp3 update} now implies that
\begin{align*}
    |p_{t,c}(a)-\widetilde{p}_{t,c}(a)| &\le e\widetilde{p}_{t,c}(a)\eta\left(|1-\beta_{e}(a)|+\sum_{i=1}^K\widetilde{p}_{t,c}(i)|1-\beta_{e}(a)|\right)\left(L+\frac{2\iota}{\gamma}\right)\\
    &\le \frac{e}{2}\widetilde{p}_{t,c}(a)\left(|1-\beta_{e}(a)|+\sum_{i=1}^K\widetilde{p}_{t,c}(i)|1-\beta_{e}(a)|\right)\,.
\end{align*}
Hence
\begin{align*}
    \sum_{a=1}^K|\widetilde{p}_{t,c}(a)-p_{t,c}(a)|\cdot|1-\beta_{e}(a)| &\le \frac{e}{2}\left(\sum_{a=1}^K\widetilde{p}_{t,c}(a)(1-\beta_{e}(a))^2+\left(\sum_{a=1}^K\widetilde{p}_{t,c}(a)(1-\beta_{e}(a)\right)^2\right)\\
    &\le e\sum_{a=1}^K\widetilde{p}_{t,c}(a)(1-\beta_{e}(a))^2.\tag{Jensen's inequality}
\end{align*}
\end{proof}

\end{lemma}

\section{Proof of \Cref{thm:main}}

Here we give the formal proof of \Cref{thm:main}. We decompose the regret as
\begin{align*}
\Reg(\pi) &= \E\left[\sum_{t=1}^T \ip{q_{t, c_t}- \pi_{c_t}, \ell_{t, c_t}}\right] \\
&=  \underbrace{\E\left[\sum_{t=1}^T \ip{q_{t, c_t} - p_{t, c_t}, \ell_{t, c_t}}\right]}_{\bias{1}} \\
&+ \underbrace{\E\left[\sum_{t=1}^T \ip{p_{t, c_t}- \pi_{c_t}, \ell_{t, c_t}-\widetilde{\ell}_{t, c_t}}\right]}_{\bias{2}} \\
& +\underbrace{\E\left[\sum_{t=1}^T \ip{\widetilde{p}_{t, c_t}-\pi_{c_t}, \widetilde{\ell}_{t, c_t}-\widehat{\ell}_{t, c_t}}\right]}_{\bias{3}} \\
& +\underbrace{\E\left[\sum_{t=1}^T\ip{ p_{t, c_t}-\widetilde{p}_{t, c_t}, \widetilde{\ell}_{t, c_t}-\widehat{\ell}_{t, c_t}}\right]}_{\bias{4}}\\
& +\underbrace{\E\left[\sum_{t=1}^T\ip{ p_{t, c_t}-\pi_{c_t}, \widehat{\ell}_{t, c_t}}\right]}_{\mathbf{ftrl}}.
\end{align*}

We bound those terms separately.

\paragraph{Bounding $\bias{1}$.} By \Cref{lem:s_smaller_p_smaller_2s}, we have that $p_t = q_t$ under event $Q$. Thus we have
\begin{align*}
    \bias{1} =&\E\left[\sum_{t=1}^T \ip{q_{t, c_t} - p_{t, c_t}, \ell_{t, c_t}}\right] \\
    =& \E\left[Q \sum_{t=1}^T \ip{q_{t, c_t} - p_{t, c_t}, \ell_{t, c_t}} \right]  + \E\left[(1-Q) \sum_{t=1}^T \ip{q_{t, c_t} - p_{t, c_t}, \ell_{t, c_t}} \right] \\
    =& \E\left[(1-Q) \sum_{t=1}^T \ip{q_{t, c_t} - p_{t, c_t}, \ell_{t, c_t}}\right]\\
    \le& \left( 1- \Pr(Q) \right) T.
\end{align*}

\paragraph{Bounding $\bias{2}$.} We have
\begin{align*}
    \bias{2} &= \E\left[\sum_{t=1}^T \ip{p_{t, c_t}- \pi_{c_t}, \ell_{t, c_t}-\widetilde{\ell}_{t, c_t}}\right] \\
    &= \sum_{t=1}^T \E\left[ \ip{p_{t, c_t}- \pi_{c_t}, \E[\ell_{t, c_t}-\widetilde{\ell}_{t, c_t} \big| \His_{t-1}]} \right]\\
    &= \sum_{t=1}^T \E[\sum_{a} \left( p_{t, c_t}(a) - \pi_{c_t}(a) \right) \left( \ell_{t, c_t}(a) - \frac{w_e(a)}{w_e(a) + \gamma} \ell_{t, c_t}(a)\right) ]\\
    &= \sum_{t=1}^T \E[\sum_{a} \left( p_{t, c_t}(a) - \pi_{c_t}(a) \right) \ell_{t, c_t}(a) \frac{\gamma}{w_e(a) + \gamma} ] \\
    &\le  \gamma \sum_{t=1}^T \E[\sum_{a} \sum_c p_{t, c}(a) \Pr(c) \frac{1}{w_e(a) + \gamma} ] \\
    &= \gamma \E\left[\sum_{t=1}^T\sum_{a\in[K]} \frac{p_t(a)}{w_e(a)+ \gamma} \right].
\end{align*}
The final term is within $\sqrt{\alpha}$ with high probability.

\paragraph{Bounding $\bias{3}$.} We have
\begin{align*}
    \bias{3}   =&\E\left[\sum_{t=1}^T \ip{\widetilde{p}_{t, c_t}-\pi_{c_t}, \widetilde{\ell}_{t, c_t}-\widehat{\ell}_{t, c_t}}\right]\\
    =&\sum_e \sum_{t \in \Time_e} \E\left[\E_e\left[ \ip{\widetilde{p}_{t, c_t}-\pi_{c_t}, \widetilde{\ell}_{t, c_t}-\widehat{\ell}_{t, c_t}}\right]\right]\\
    =&\sum_e \sum_{t \in \Time_e} \E\left[ \ip{\widetilde{p}_{t, c_t}-\pi_{c_t}, \E_e\left[\widetilde{\ell}_{t, c_t}-\widehat{\ell}_{t, c_t} \right]}\right]\\
%
    =& \sum_e \sum_{t \in \Time_e} \E\left[ \ip{\widetilde{p}_{t, c_t}-\pi_{c_t}, \E_e\left[\left(\widetilde{\ell}_{t, c_t}-\widehat{\ell}_{t, c_t} \right)F_e\right]}\right] + \sum_e \sum_{t \in \Time_e} \E\left[ \ip{\widetilde{p}_{t, c_t}-\pi_{c_t}, \E_e\left[\left(\widetilde{\ell}_{t, c_t}-\widehat{\ell}_{t, c_t} \right) (1 - F_e)\right]}\right] \\
%
    \le& \sum_e \sum_{t \in \Time_e} \E\left[ \sum_a \widetilde{p}_{t,c_t}(a) \frac{\gamma}{w_e(a) + \gamma} \right] + \sum_e \sum_{t \in \Time_e} \E\left[ \ip{\widetilde{p}_{t, c_t}-\pi_{c_t}, \E_e\left[\left(\widetilde{\ell}_{t, c_t}-\widehat{\ell}_{t, c_t} \right) (1 - F_e)\right]}\right] \tag{\Cref{lem: bounding_1_minus_beta}}\\
%
    \le& \sum_e \sum_{t \in \Time_e} \E\left[ \sum_a \widetilde{p}_{t,c_t}(a) \frac{\gamma}{w_e(a) + \gamma} \right] + \sum_e \sum_{t \in \Time_e} \left(1 - \Pr(F_e)\right) \frac{2}{\gamma}  \\
%
    \le& \sum_e \sum_{t \in \Time_e} \E\left[ \sum_a \sum_c \widetilde{p}_{t,c}(a) \Pr(c) \frac{\gamma}{w_e(a) + \gamma} \right] + T \left(1 - \Pr(Q)\right) \frac{2}{\gamma} \\
%
    =& \sum_e \sum_{t \in \Time_e} \E\left[ \sum_a \widetilde{p}_t(a)  \frac{\gamma}{w_e(a) + \gamma} \right] + T \left(1 - \Pr(Q)\right) \frac{2}{\gamma} \\
%
    \le& 4 \gamma \E\left[\sum_{t=1}^T\sum_{a\in[K]} \frac{p_t(a)}{w_e(a)+ \gamma} \right] + T \left(1 - \Pr(Q)\right) \frac{2}{\gamma}. \tag{\Cref{lem:s_smaller_p_smaller_2s}}.
\end{align*}

\paragraph{Bounding $\bias{4}$.} We have
\begin{align*}
\bias{4} =& \mathbb{E} \left[ \sum_e \sum_{t \in \Time_e} \ip{p_{t,c_t} - \widetilde{p}_{t,c_t}, \widetilde{\ell}_{t,c_t} - \widehat{\ell}_{t,c_t}} \right] \\
%
=& \mathbb{E} \left[ \sum_e \sum_{t \in \Time_e} \ip{p_{t,c_t} - \widetilde{p}_{t,c_t}, \widetilde{\ell}_{t,c_t} - \widehat{\ell}_{t,c_t}} Q \right] + \mathbb{E} \left[ \sum_e \sum_{t \in \Time_e} \ip{p_{t,c_t} - \widetilde{p}_{t,c_t}, \widetilde{\ell}_{t,c_t} - \widehat{\ell}_{t,c_t}} (1-Q) \right]\\
%
\le& \mathbb{E} \left[ \sum_e \sum_{t \in \Time_e} \ip{p_{t,c_t} - \widetilde{p}_{t,c_t}, \widetilde{\ell}_{t,c_t} - \widehat{\ell}_{t,c_t}} Q \right] + \left(1-\Pr(Q)\right) \frac{2}{\gamma}\\
%
=& \mathbb{E} \left[ \sum_{e=1}^{T/L} \sum_{t \in T_e} \sum_{a=1}^{K} (p_{t,c_t}(a) - \widetilde{p}_{t,c_t}(a))(1 - \beta_{e}(a)) \widetilde{\ell}_{t,c_t}(a) Q\right] + \left(1-\Pr(Q)\right) \frac{2}{\gamma}\\
%
\le& \mathbb{E} \left[ \sum_{e=1}^{T/L} \sum_{t \in T_e} \sum_{a=1}^{K} |p_{t,c_t}(a) - \widetilde{p}_{t,c_t}(a)| \cdot |1 - \beta_{e}(a)| Q \right]  + \left(1-\Pr(Q)\right) \frac{2}{\gamma}\\
%
\le& \mathbb{E} \left[ \sum_{e=1}^{T/L} \sum_{t \in T_e} \sum_{a=1}^{K} |p_{t,c_t}(a) - \widetilde{p}_{t,c_t}(a)| \cdot |1 - \beta_{e}(a)| Q \right]  + \left(1-\Pr(Q)\right) \frac{2}{\gamma} \\
%
\le& \mathbb{E} \left[ \sum_{e=1}^{T/L} \sum_{t \in T_e} \sum_{c=1}^{C} \sum_{a=1}^{K} 3 \Pr(c) \widetilde{p}_{t,c}(a)(1 - \beta_{e}(a))^2 Q \right] +  \left(1-\Pr(Q)\right) \frac{2}{\gamma} \tag{\Cref{lem: pure_concentration}}\\ 
%
=& \left(\frac{98 \iota}{L}  + \frac{\gamma^2 L }{\iota} \right) \E\left[\sum^T_{t=1} \sum_{a\in[K]} \frac{p_t(a)}{w_e(a)+ \gamma} \right] +  \left(1-\Pr(Q)\right) \frac{2}{\gamma} \tag{\Cref{lem: beta_concentration}, \Cref{lem:s_smaller_p_smaller_2s}}. 
\end{align*}

\paragraph{Bounding ftrl.} We have
\begin{align*}
\mathbf{ftrl} &= \mathbb{E} \left[ \sum_{e=1}^{T/L} \sum_{t \in T_e} \ip{ p_{t,c_t} - \pi_{c_t}, \widehat{\ell}_{t,c_t} } \right] \\
&\le \frac{\log(K)}{\eta} + \eta \mathbb{E} \left[ 
\sum_{c} \Pr(c) \sum_{e=1}^{T/L} \sum_{t \in T_e} \sum_{a \in[K]} p_{t,c}(a) \widehat{\ell}^2_{t,c}(a) \right] \tag{Standard FTRL analysis}\\
%
&\le \frac{\log(K)}{\eta} + \eta \E\left[
\sum_{e=1}^{T/L} \sum_{t \in T_e} \sum_{a \in[K]} \sum_{c \in [M]} 
\Pr(c) p_{t,c}(a) \frac{w_{e}(a)}{\left( \widehat{w}_{e}(a) + \frac{3}{2} \gamma \right)^2} \right] \\
%
&\le \frac{\log(K)}{\eta} + \eta \E\left[
\sum_{t=1}^T \sum_{a \in[K]} p_t(a) \frac{w_{e}(a)}{\left( \widehat{w}_{e}(a) + \frac{3}{2} \gamma \right)^2} Q \right] + \eta \E\left[
\sum_{t=1}^T \sum_{a \in[K]}  p_{t}(a) \frac{w_{e}(a)}{\left( \widehat{w}_{e}(a) + \frac{3}{2} \gamma \right)^2} (1-Q) \right] \\
%
&\leq \frac{\log(K)}{\eta} + 4\eta\E\left[\sum_{t=1}^T \sum_{a\in[K]} \frac{p_t(a)}{w_e(a)+ \gamma}  \right] + \eta \frac{1}{\gamma^2} \left(1 - \Pr(Q)\right) \tag{\Cref{lem:s_smaller_p_smaller_2s}}.
\end{align*}

\paragraph{Combining the pieces together.} We have
\begin{align*}
    \Reg(\pi) &= \bias{1} + \bias{2} + \bias{3} + \bias{4} + \textbf{ftrl} \\
%
    &\le \left( 1- \Pr(Q) \right) T + \gamma \E\left[\sum_{t=1}^T\sum_{a\in[K]} \frac{p_t(a)}{w_e(a)+ \gamma} \right]  +  4 \gamma  \E\left[\sum_{t=1}^T\sum_{a\in[K]} \frac{p_t(a)}{w_e(a)+ \gamma} \right]  + T \left(1 - \Pr(Q)\right) \frac{2}{\gamma} \\
    &+ (\frac{98 \iota}{L}  + \frac{\gamma^2 L }{\iota}) \E\left[\sum_{t=1}^T\sum_{a\in[K]} \frac{p_t(a)}{w_e(a)+ \gamma} \right]  +  \left(1-\Pr(Q)\right) \frac{2}{\gamma}  \\
    &+ 4\eta\E\left[\sum_{t=1}^T\sum_{a\in[K]} \frac{p_t(a)}{w_e(a)+ \gamma} \right] + \eta \frac{1}{\gamma^2} \left(1 - \Pr(Q)\right) \\
%
    &\le \left(T + \frac{2}{\gamma}T + \frac{\eta}{\gamma^2} \right) \left(1-\Pr(Q) \right) +  \frac{98 K T_\ell}{L} + \frac{\gamma^2 L K T}{\iota}  + (5\gamma+ 4\eta + \frac{98 \iota}{L}  + \frac{\gamma^2 L }{\iota}) \E\left[\sum_{t=1}^T\sum_{a\in[K]} \frac{p_t(a)}{w_e(a)+ \gamma} \right].
\end{align*}

Applying \Cref{lem: graph_inverse} and the fact $1 - \Pr(Q) \le 3KT\exp(-\iota)/L$ shows that 
\[\Reg(\pi) \le \widetilde{O}(\sqrt{\alpha T}).\]