\iffalse

\section{General Case (Any arm) Explore First Analysis}
Let $\tau$ denote $2t'$ and $\pi^{\tau}$ denote the solution obtained with $\hat{A}^{\tau}$ after $2t'$ rounds of exploration. $k_i:=\argmax_{j\in [m]}A_{i, j}$ and $k_i^t:=\argmax_{j\in [m]}\widehat{A}^t_{i, j}$ with ties broken arbitrarily.
\newline
\textbf{Social welfare regret:}
\begin{align*}
    \tau + \sum_{t=\tau+1}^T\sum_{i=1}^n A_i(\pi^*-\pi^\tau) & = \tau + (T-\tau)\sum_{i=1}^n \left(A_i(\pi^*-\pi^\tau) - \widehat{A}_i^\tau \pi^\tau + \widehat{A}_i^\tau \pi^\tau \right)\\
    & = \tau + (T-\tau)\sum_{i=1}^n \left( (\widehat{A}^\tau_i-A_i)\pi^\tau + A_i\pi^* - \widehat{A}_i^\tau \pi^\tau \right)\\
    & \leq  \tau + (T-\tau)\sum_{i=1}^n \left( (\widehat{A}^\tau_i-A_i)\pi^\tau + \overline{A}^\tau_i\pi^* - \widehat{A}_i^\tau \pi^\tau \right) \ (\textup{w.p. }\geq 1-\delta)\\
    & = \tau + (T-\tau)\sum_{i=1}^n \left( (\widehat{A}^\tau_i-A_i)\pi^\tau + \widehat{A}^\tau_i\pi^* + \langle \pi^*,\epsilon^\tau \rangle - \widehat{A}_i^\tau \pi^\tau \right)\\
    & \leq  \tau + (T-\tau)\sum_{i=1}^n \left( (\widehat{A}^\tau_i-A_i)\pi^\tau + \langle \pi^*,\epsilon^\tau \rangle \right) \ (\because \pi^\tau \ \textup{is the solution of the empirical LP})\\
    &= \tau + (T-\tau)\sum_{i=1}^n \left( \langle \pi^\tau, \epsilon^\tau \rangle + \langle \pi^*,\epsilon^\tau \rangle \right)\\
    &\leq  \tau + 2(T-\tau)n \epsilon/\sqrt{\min_{j\in [m]} N_j^\tau}\\
    & =  O(\tau + (T-\tau)/\sqrt{\tau})
\end{align*}
On choosing $\tau$ as $T^{2/3}$, we get $\mathcal{R}_\textsc{SW}(T)=\tilde{O}(T^{2/3})$.
\newline
\newline
\textbf{Fairness regret:}
\begin{align*}
    \tau + \sum_{i=1}^n(T-\tau)|cA_{i, k_i}-A_i\pi^t|_+ &= \tau + \sum_{i=1}^n\sum_{t=\tau}^T|cA_{i, k_i}-A_i\pi^\tau|_+ \\
    & = \tau + \sum_{i=1}^n (T-\tau)|cA_{i,k_i}-A_i\pi^\tau - \widehat{A}_i^\tau \pi^\tau + \widehat{A}_i^\tau \pi^\tau - c\widehat{A}^\tau_{i, k_i^\tau}+c\widehat{A}^\tau_{i, k_i^\tau}|_+\\
    &= \tau + \sum_{i=1}^n (T-\tau)|cA_{i,k_i}- c\widehat{A}^\tau_{i, k_i^\tau}  + (\widehat{A}_i^\tau -A_i)\pi^\tau +c\widehat{A}^\tau_{i, k_i^\tau}- \widehat{A}_i^\tau \pi^\tau|_+\\
    &\leq \tau + \sum_{i=1}^n (T-\tau)\left(|cA_{i,k_i}- c\widehat{A}^\tau_{i, k_i^\tau}|_+  + |(\widehat{A}_i^\tau -A_i)\pi^\tau|_+ +|c\widehat{A}^\tau_{i, k_i^\tau}- \widehat{A}_i^\tau \pi^\tau|_+\right)\\
    & = \tau + \sum_{i=1}^n (T-\tau)\left(|cA_{i,k_i}- c\widehat{A}^\tau_{i, k_i^\tau}|_+  + |(\widehat{A}_i^\tau -A_i)\pi^\tau|_+\right) \ (\because \pi^\tau \textup{ is the solution of the empirical LP})\\
    & = \tau + \sum_{i=1}^n (T-\tau)\left(c\epsilon/\sqrt{N_{k_i^\tau}^\tau} + \epsilon/\sqrt{\min_{j\in [m]}N_j^\tau}\right)\\
    & = O(\tau + n(T-\tau)/\sqrt{\tau})
\end{align*}
Again on choosing $\tau$ as $T^{2/3}$, we get $\mathcal{R}_\textsc{SW}(T)=\tilde{O}(T^{2/3})$.

\fi