\begin{proof}[Proof of lemma~\ref{lem:lemOne}]
Let $i^*\in \argmin_{i \in [n] \setminus [n_1]}\left(\frac{1 - c}{ 1 - \frac{{A}_{i,1}}{{A}_{i,2}}}\right)$ and $i'\in \argmin_{i :\widehat{A}_{i, 1}<\widehat{A}_{i, 2}}\left(\frac{1 - c}{ 1 - \frac{\widehat{A}_{i,1}}{\widehat{A}_{i,2}}}\right)$.
\begin{align*}
    x^*-x^t&= \min \left( 1,  \min_{i \in [n] \setminus [n_1]}\frac{1 - c}{ 1 - \frac{A_{i,1}}{A_{i,2}}} \right)-\min \left( 1, \min_{i:\widehat{A}_{i, 1}<\widehat{A}_{i, 2}} \frac{1 - c}{ 1 - \frac{\widehat{A}_{i,1}}{\widehat{A}_{i,2}}} \right)
\end{align*}
When $\{i: \widehat{A}_{i, 1}<\widehat{A}_{i, 2}\}\neq \phi$, $x^*-x^t = \min\left(1, \frac{1-c}{1-\frac{A_{i^*,1}}{{A_{i^*,2}}}}\right)
    - \min\left(1, \frac{1-c}{1-\frac{\widehat{A}_{i',1}}{{\widehat{A}_{i',2}}}}\right),$ else, $x^*-x^t=\min\left(1, \frac{1-c}{1-\frac{A_{i^*,1}}{{A_{i^*,2}}}}\right)
    - 1.$
\newline
We bound $x^*-x^t$ under the event $E_\delta=\left\{\frac{\widehat{A}_{i', 1}}{\widehat{A}_{i', 2}}\leq \frac{A_{i', 1}}{A_{i', 2}}-\frac{2c\delta}{1+\delta}\right\}$ for $\delta\in \left(0, 1\right)$ and $i'\in [n]$ when $\frac{\widehat{A}_{i', 1}}{\widehat{A}_{i', 2}}<c$. As $\frac{\widehat{A}_{i', 1}}{\widehat{A}_{i', 2}}<c$, the event $E_\delta$ implies $\frac{\widehat{A}_{i', 1}}{\widehat{A}_{i', 2}}\leq \frac{1+\delta}{(1+3\delta)}\frac{A_{i', 1}}{A_{i', 2}}$.
Further, $E_\delta \cap \left\{ \widehat{A}_{i', 2} \leq  \left(1+3\delta \right)A_{i', 2} \right\}\subseteq \left\{ \widehat{A}_{i', 2} \leq  \left(1+3\delta \right)A_{i', 2} \right\}\cap \left\{ \widehat{A}_{i', 1} \leq  \left(1+\delta \right)A_{i', 1} \right\}.$
\begin{align*}
    \mathbb{P}\left(E_\delta \cap \left\{ \widehat{A}_{i', 2} \leq  \left(1+3\delta \right)A_{i', 2} \right\}\right) 
    &\leq \mathbb{P}\left(\left\{ \widehat{A}_{i', 2} \leq  \left(1+3\delta \right)A_{i', 2} \right\}\right) \mathbb{P}\left(\left\{ \widehat{A}_{i', 1} \leq  \left(1+\delta \right)A_{i', 1} \right\}\right) \ \tag{From independence of $\widehat{A}_{i', 1} \ \& \ \widehat{A}_{i', 2}$} \\
    &\leq \mathbb{P}\left(\left\{ \widehat{A}_{i', 1} \leq  \left(1+\delta \right)A_{i', 1} \right\}\right)  \\
    &\leq \exp\left( -\frac{t'}{2}\left(A_{i', 1}/\sigma\right)^2\delta^2 \right) \ \tag{From Lemma~\ref{lemma:chernoff-utb}}
\end{align*}
Also, $\mathbb{P}\left(E_\delta \cap \left\{ \widehat{A}_{i', 2} >  \left(1+3\delta \right)A_{i', 2} \right\}\right) \leq  \mathbb{P}(\widehat{A}_{i', 1}\leq (1+\delta) A_{i', 1}) \leq \exp\left( -\frac{t'}{2}\left(A_{i', 1}/\sigma\right)^2\delta^2 \right)$ (Lemma~\ref{lemma:chernoff-utb}). Thus, we have the following.
\begin{align*}
    \mathbb{P}(E_\delta)&=  \mathbb{P}\left(E_\delta \cap \left\{ \widehat{A}_{i', 2} \leq  \left(1+3\delta \right)A_{i', 2} \right\}\right) + \mathbb{P}\left(E_\delta \cap \left\{ \widehat{A}_{i', 2} >  \left(1+3\delta \right)A_{i', 2} \right\}\right)\\
    &\leq  2\exp\left( -\frac{t'}{2}\left(A_{i', 1}/\sigma\right)^2\delta^2 \right)\\
    &\leq 2\exp\left( -\frac{t'}{2}\left(a_{\min}/\sigma\right)^2\delta^2 \right).
\end{align*}
Now, we begin the proof of upper-bounding $x^*-x^t$.
\newline
\textbf{Case (I) $x^*<1$,\ $x^t<1$:}
We first note that $x^*<1\implies \frac{A_{i^*, 1}}{A_{i^*, 2}}<c$ and $x^t<1\implies \frac{\widehat{A}_{i', 1}}{\widehat{A}_{i', 2}}<c$.
\begin{align*}
    x^*-x^t & = \frac{1-c}{1-\frac{A_{i^*,1}}{A_{i^*,2}}}-\frac{1-c}{1-\frac{\widehat{A}_{i',1}}{\widehat{A}_{i',2}}} \\
    &\leq \frac{1-c}{1-\frac{A_{i',1}}{A_{i',2}}}-\frac{1-c}{1-\frac{\widehat{A}_{i',1}}{\widehat{A}_{i',2}}} \ \tag{From the definition of $i^*$ and $\widebar{E_\delta}$}
\end{align*}
The last inequality follows by noting that under $\widebar{E_\delta},\ i'\in ([n]\setminus [n_1])$ and then we use the fact that $i^*$ is the argmin obtained after searching over the set $([n]\setminus [n_1])$. Thus, with probability at least $1-\mathbb{P}(E_\delta)$, we have the following
\begin{align*}
    x^*-x^t&\leq (1-c)\frac{\frac{2c\delta}{1+\delta}}{(1-c)\left(1-\frac{A_{i', 1}}{A_{i', 2}} \right)}\\
    &\leq (1-c)\frac{\frac{2c\delta}{1+\delta}}{(1-c)\left(1-\frac{\widehat{A}_{i', 1}}{\widehat{A}_{i', 2}} +\frac{2c\delta}{1+\delta} \right)} \ \tag{under $\widebar{E_\delta}$}\\
    &\leq \frac{2c\delta}{1+\delta}.
\end{align*}
\textbf{Case (II) $x^*<1$,\ $x^t=1$:} Here, $x^*-x^t<0$.
% We first note that $x^*<1\implies \frac{A_{i^*, 1}}{A_{i^*, 2}}<c$. 
% \begin{align*}
%     x^*-x^t = \frac{\frac{A_{i^*, 1}}{A_{i^*, 2}}-c}{1-\frac{A_{i^*, 1}}{A_{i^*, 2}}}\leq 0 \ \left(\because 0<\frac{A_{i^*, 1}}{A_{i^*, 2}}<c\right).
% \end{align*}
\newline
\textbf{Case (III) $x^*=1$,\ $x^t<1$}: 
We first note that $x^*=1\implies \frac{A_{i^*, 1}}{A_{i^*, 2}}\geq c$ as $[n]\setminus [n_1]$ is always taken to be non-empty. 

\begin{align*}
x^* - x^t = \frac{c - \frac{\widehat{A}_{i',1}}{\widehat{A}_{i',2}}}{1 - \frac{\widehat{A}_{i',1}}{\widehat{A}_{i',2}}}
\end{align*}
As RHS is a decreasing function in $\frac{\widehat{A}_{i', 1}}{\widehat{A}_{i', 2}}$, with probability $1-\mathbb{P}(E_\delta)$, we have the following.
\begin{align*}
    x^*-x^t\leq & \frac{c-\frac{A_{i', 1}}{A_{i', 2}}+\frac{2c\delta}{1+\delta}}{1-\frac{A_{i', 1}}{A_{i', 2}}+\frac{2c\delta}{1+\delta}}
\end{align*}
This RHS is a decreasing function of $\frac{A_{i', 1}}{A_{i', 2}}$. We know that if $i'\in [n]\setminus [n_1]$, $\frac{A_{i', 1}}{A_{i', 2}}\geq \frac{A_{i^*, 1}}{A_{i^*, 2}}\geq c$. Also, if $i'\in [n_1]$, $\frac{A_{i', 1}}{A_{i', 2}}\geq 1\geq c$. Thus, we have the following,
\begin{align*}
    x^*-x^t\leq & \frac{\frac{2c\delta}{1+\delta}}{1-c+\frac{2c\delta}{1+\delta}}=\frac{2c\delta}{(1-c)+\delta(1+c)} \leq \frac{2c\delta}{(1-c)(1+\delta)}.
\end{align*}
This proves our claim that with probability $\mathbb{P}(\bar{E_\delta})$ i.e. with probability at least $\left(1-2\exp\left( -\frac{t'}{2}\left(a_{\min}/\sigma\right)^2\delta^2 \right)\right)$, we have $x^*-x^t\leq \frac{2c\delta}{(1-c)(1+\delta)}.$

% \piyushi{$\mathbb{P}(E_\delta)$ had to be changed as the previous proof uses $\frac{A_{i', 1}}{A_{i', 2}}<c$ but here, we have $\frac{\widehat{A}_{i', 1}}{\widehat{A}_{i', 2}}<c$. In this new proof, we are only using the upper-tail bound, not the lower tail bound.}
% \piyushi{We could've also defined $E_\delta=\{\frac{\widehat{A}_{i', 1}}{\widehat{A}_{i', 2}}\leq \frac{(1-\delta)}{(1+\delta)}\frac{A_{i^*, 1} }{A_{i^*, 2}}\}$ but the original $E_\delta$ is used in the fairness regret's proof also.}
\end{proof}