\section{Proof of SRPQSI with incoherent measurement}

\subsection{Proof of property for purity collision}
    \begin{lemma} \label{lem:purity_collision_property}
        The expectation and variance of the purity estimation satisfying
        \begin{equation}
            \mathbb{E} [\tilde{g}]  = \frac{m-1}{m}\sum_{i=0}^{d-1} p_i^2,    
        \end{equation}
        and
        \begin{equation}
            \Var[\tilde{g}] \leq \frac{\mathbb{E} [\tilde{g}]}{m^2} + \frac{2}{m} \sum_{i=0}^{d-1} p_i^3.
        \end{equation}
    \end{lemma}
    \begin{proof}
        
    \label{proof: purity_collision_property}
    The expectation of $\tilde{g}$ satisfying
    \begin{equation}
        \begin{aligned}
            \mathbb{E} [\tilde{g}] = & \mathbb{E}\left[\frac{1}{m^2} \sum_{i=0}^{d-1} \left[ \sum_{j=1}^m \indicator\{x_j =i\}\right]^2\right] - \frac{1}{m}\\
            = & \mathbb{E}\left[\frac{1}{m^2} \sum_{i=0}^{d-1} \left[ \sum_{j=1}^m \sum_{k=1}^m \indicator\{x_j =i\}\indicator\{x_k =i\}\right]\right] - \frac{1}{m}\\
            = & \mathbb{E}\left[\frac{1}{m^2} \sum_{i=0}^{d-1} \left[ \sum_{j=1}^m \sum_{k=1}^m \indicator\{x_j =i\}\indicator\{x_k =i\}\right]\right] - \frac{1}{m}\\
            = & \mathbb{E}\left[\frac{1}{m^2} \sum_{i=0}^{d-1} \left[ \sum_{j=1}^m \indicator\{x_j =i\}+ \sum_{j=1}^m \sum_{k\neq j} \indicator\{x_j =i\}\indicator\{x_k =i\}\right]\right] - \frac{1}{m}\\
            = & \frac{1}{m^2} \sum_{i=0}^{d-1}  \sum_{j=1}^m \mathbb{E}\left[\indicator\{x_j =i\}\right]+ \frac{1}{m^2} \sum_{j=1}^m \sum_{k\neq j} \mathbb{E} [\indicator\{x_j =i\}\indicator\{x_k =i\}] - \frac{1}{m}\\
            = & \frac{m}{m^2} + \frac{m-1}{m} \sum_{j=1}^m p_j^2 - \frac{1}{m}
            = \frac{m-1}{m} \sum_{j=1}^m p_j^2.
        \end{aligned}
    \end{equation}
    The expectation of $\tilde{g}^2$ satisfying
    \begin{equation*}
        \begin{aligned}
            \mathbb{E} [\tilde{g}^2] = & \mathbb{E}\left[\left[\frac{1}{m^2}  \sum_{i=0}^{d-1}\left[ \sum_{j=1}^m \indicator\{x_j =i\}\right]^2 -\frac{1}{m}\right]^2\right] \\
            = & \frac{1}{m^4} \mathbb{E} \left[\sum_{j_1\neq j_2,l_1 \neq l_2}^m\left[\sum_{i,k}^{d-1} \indicator\{x_{j_1} =i\} \indicator\{x_{j_2} =i\} \indicator\{x_{l_1} =k\} \indicator\{x_{l_2} =k\}\right] \right]\\
            = & \frac{1}{m^4} \left[ m(m-1)\mathbb{E}[\tilde{g}] + m(m-1)^2(m-2)\mathbb{E}[\tilde{g}]^2 + 2m(m-1)(m-2)\sum_{j=1}^n p_j^3\right]\\
            \leq & \frac{1}{m^2} \mathbb{E}[\tilde{g}] + \mathbb{E}[\tilde{g}]^2+ \frac{2}{m} \sum_{i=0}^{d-1} p_i^3
        \end{aligned}
    \end{equation*}
    
    
    Then, we have
    
    \begin{equation}
        \begin{aligned}
            \Var[\tilde{g}] & = \mathbb{E}[\tilde{g}^2] - \mathbb{E}[\tilde{g}]^2\\
            & \leq \frac{1}{m^2} \mathbb{E}[\tilde{g}] + \frac{2}{m} \sum_{i=0}^{d-1} p_i^3.
        \end{aligned}
    \end{equation}

    \end{proof}

\subsection{proof of Theorem \ref{thm:alg_SRPQSI}}
\label{subsec:PQSI_alg1}

    By the definition of $w(\cdot,\cdot)$ and the definition of $\Delta_{(\cdot)}$, we have
    \begin{equation*}
        \begin{aligned}
            & \mathbb{P}(w({\rho^\star,k}) \leq w({\rho_{(i)},k})) \\
            = & \mathbb{P}\left( (w(\rho_{(i)},k) -  w(\rho^\star,k))  \geq \frac{(m-1)\Delta_{(i)}}{m}\right).
        \end{aligned}
    \end{equation*}
    Since $w(\cdot,\cdot) \in [0,1]$, by Lemma \ref{lem: g_var} and Bernstein's inequality, we have
    \begin{equation}
        \begin{aligned}
            & \mathbb{P}\left( (w(\rho_{(i)},k) -  w(\rho^\star,k))  \geq \frac{(m-1)\Delta_{(i)}}{m}\right) \\
            \leq & \exp\left(-\frac{\lfloor \frac{N_k}{m}\rfloor \left(\frac{m-1}{m(d+1)}\Delta_{(i)}\right)^2}{O(\frac{1}{d^3} + \frac{1}{m^2d} + \frac{1}{md^2}) + \frac{2\Delta_{(i)}}{3(d+1)}}\right) \\
            \leq & \exp\left( -\Omega\left( \frac{\sqrt{c}N_k \Delta_{(i)}}{d}\right)\right).
        \end{aligned}
    \end{equation}

    By a union bound of error probability, we have 

    \begin{equation} \label{eq:err_upper1}
        \begin{aligned} 
            e_n & \leq \sum_{k=1}^{K-1}\sum_{i = K+1-k}^K \mathbb{P}(w({\rho^\star,k}) \leq w({\rho_{(i)},n_k})) \\
            & \leq \sum_{k=1}^{K-1}\sum_{i = K+1-k}^K \exp\left( - \Omega\left(\frac{\sqrt{c}N_k \Delta_{(i)}}{d}\right)\right) \\
            &  \leq \sum_{k=1}^{K-1} k \exp\left( -\Omega\left( \frac{\sqrt{c}N_k \Delta_{(K+1-k)}}{d}\right)\right). \\
        \end{aligned}
    \end{equation}
    By definition of $N_k$, we have
    \begin{equation} \label{eq:err_upper2}
        \begin{aligned}
            & \frac{\sqrt{c}N_k \Delta_{(K+1-k)}}{d} \\
            = & \left\lceil \frac{\sqrt{c}}{\overline{\log}(K)} \frac{N-K}{K+1-k}\right\rceil\frac{\Delta_{(K+1-k)}}{d} \\
            = &\Theta\left( \frac{\sqrt{c}N}{\overline{\log}(K)} \times \frac{\Delta_{(K+1-k)}}{K+1-k}\right). \\
        \end{aligned}
    \end{equation}
    Combining equation \eqref{eq:err_upper1} and \eqref{eq:err_upper2}, we have
    \begin{equation*}
        \begin{aligned}
            e_n & \leq \sum_{k=1}^{K-1} k \exp\left( -\Omega\left(\frac{\sqrt{c}N}{\overline{\log}(K)d} \times\frac{\Delta_{(K+1-k)}}{K+1-k}\right)\right) \\
            & \leq \frac{K(K-1)}{2} \exp\left( -\Omega\left(\frac{\sqrt{c}NH_1}{\overline{\log}(K)d}\right)\right)
        \end{aligned}
    \end{equation*}
    where $H_1 = \min_{i \in \{1,...,K\}} \frac{\Delta_{(i)}}{i}$.

    
\subsection{proof of Lemma \ref{lem2:PQSI_alg}}
\label{subsec:PQSI_alg2}

\begin{proof}
    By the definition of $w(\cdot,\cdot)$ and the definition of $\Delta_{(\cdot)}$, we have
    \begin{equation*}
        \begin{aligned}
            & \mathbb{P}(w({\rho^\star,k}) \leq w({\rho_{(i)},k})) \\
            = & \mathbb{P}\left( (w(\rho_{(i)},k) -  w(\rho^\star,k))  \geq \frac{(m-1)\Delta_{(i)}}{m}\right).
        \end{aligned}
    \end{equation*}
    Since $w(\cdot,\cdot) \in [0,1]$, by Lemma \ref{lem: g_var} and Bernstein's inequality, we have
    \begin{equation}
        \begin{aligned}
            & \mathbb{P}\left( (w(\rho_{(i)},k) -  w(\rho^\star,k))  \geq \frac{(m-1)\Delta_{(i)}}{m}\right) \\
            \leq & \exp\left(-\frac{\lfloor \frac{N_k}{d}\rfloor \left(\frac{m-1}{m(d+1)}\Delta_{(i)}\right)^2}{O(\frac{1}{d^3}) + \frac{2\Delta_{(i)}}{3(d+1)}}\right) \\
            \leq & \exp\left( -\Omega\left( \min\left( \frac{N_k \Delta_{(i)}}{d^2}, N_k \Delta_{(i)}^2\right)\right)\right).
        \end{aligned}
    \end{equation}

    By a union bound of error probability, we have 

    \begin{equation} \label{eq:error_upper1}
        \begin{aligned} 
            e_n & \leq \sum_{k=1}^{K-1}\sum_{i = K+1-k}^K \mathbb{P}(w({\rho^\star,k}) \leq w({\rho_{(i)},n_k})) \\
            & \leq \sum_{k=1}^{K-1}\sum_{i = K+1-k}^K \exp\left( - \Omega\left( \min\left( \frac{N_k \Delta_{(i)}}{d^2}, N_k \Delta_{(i)}^2\right)\right)\right) \\
            &  \leq \sum_{k=1}^{K-1} k \exp\left( -\Omega\left( \min\left( \frac{N_k \Delta_{(K+1-k)}}{d^2}, N_k \Delta_{(K+1-k)}^2\right)\right)\right). \\
        \end{aligned}
    \end{equation}
    By definition of $N_k$, and combining equation \eqref{eq:error_upper1}, we have
    \begin{equation*}
    \begin{aligned}
        e_N  \leq \frac{K(K-1)}{2} \exp\left(- \Omega\left(\min\left(\frac{N H_2}{\overline{\log}(K)}, \frac{N H_1}{\overline{\log}(K)d^2}\right)\right) \right),
    \end{aligned}
    \end{equation*}
    where $H_1 = \min_{i \in \{2,...,K\}} \frac{\Delta_{(i)}}{i}$, and $H_2 = \min_{i \in \{2,...,K\}} \frac{\Delta^2_{(i)}}{i}$.

\end{proof}


