\newpage
\section{Proof of Lemma \ref{lem:regretbound}}
\begin{proof}
From the convexity of $f_t$'s, for $x^\star$ satisfying Assumption \eqref{feas-constr}, we have 
$$f_t(x_t) - f_t(x^\star) \le \nabla f_t^T (x_t-x^\star).$$
From the choice of Algorithm \ref{coco_alg_1} for $x_{t+1}$, we have 
\begin{align*} ||x_{t+1}-x^\star||^2 & = || \cP_{S_{t}}(y_t) - x^\star||^2 \\
& \stackrel{(a)}\le || y_t - x^\star||^2, \\
& = ||\cP_{S_{t-1}}\left(x_t - \eta_t \nabla f_t(x_t)\right)-x^\star||^2, \\
& \stackrel{(n)}\le || (x_t-\eta_t\nabla f_t^T(x_t)) - x^\star||^2,
\end{align*}
where inequalities $(a)$ and $(b)$ follow since $x^\star \in S_t$ for all $t$.
Hence
\begin{align*}
 ||x_{t+1}-x^\star||^2 & \le  ||x_t-x^\star||^2 + \eta_t^2||\nabla f_t(x_t)||^2 - 2\eta_t \nabla f_t^T(x_t)(x_t-x^\star), \\
 \nabla f_t^T(x_t)(x_t-x^\star) & \le \frac{||x_t-x^\star||^2-||x_{t+1}-x^\star||^2 }{\eta_t} + \eta_t G^2.
\end{align*}
Summing this over $t=1$ to $T$, we get 
\begin{align*}
2\sum_{t=1}^T (f_t(x_t) - f_t(x^\star)) & \le \sum_{t=1}^T\nabla f_t^T (x_t-x^\star), \\
& \le \sum_{t=1}^T  \frac{||x_t-x^\star||^2-||x_{t+1}-x^\star||^2 }{\eta_t} + \sum_{t=1}^T\eta_t G^2, \\
& \le D^2 \frac{1}{\eta_T} + G^2 \sum_{t=1}^T\eta_t,\\
& \le O( DG \sqrt{T}),
\end{align*}
where the final inequality follows by choosing $\eta_t = \frac{D}{G\sqrt{t}}$.
\end{proof}