%
%
% \appendices
\appendix  \label{sec:appendix}
\numberwithin{equation}{section}
%
%
%% Lie Algebra %%
\section*{Lie Algebra}
\begin{equation} \label{eq:Adjoint_definition}
    \textnormal{Ad}_{\bm{g}} = \begin{bmatrix}
                                    \bm{R} & \bm{0}_{3 \times 3} \\
                                    \tilde{\bm{r}} \bm{R} & \bm{R}
                                \end{bmatrix} \, ,
\end{equation}
\begin{equation} \label{eq:coAdjoint_definition}
\textnormal{Ad}^{*}_{\bm{g}} = \begin{bmatrix}
                                    \bm{R} & \tilde{\bm{r}} \bm{R} \\
                                    \bm{0}_{3 \times 3} & \bm{R}
                                \end{bmatrix} \, ,
\end{equation}
\begin{equation} \label{eq:adjoint_definition}
    \textnormal{ad}_{\bm{\xi}, \, \bm{\eta}} = \begin{bmatrix}
      \tilde{\bm{\kappa}}, \, \tilde{\bm{w}} & \bm{0}_{3 \times 3} \\
      \tilde{\bm{\sigma}}, \, \tilde{\bm{v}} & \tilde{\bm{\kappa}}, \, \tilde{\bm{w}}
    \end{bmatrix} \, ,
\end{equation}
\begin{equation} \label{eq:coadjoint_definition}
    \textnormal{ad}^{*}_{\bm{\xi}, \, \bm{\eta}} = \begin{bmatrix}
      \tilde{\bm{\kappa}}, \, \tilde{\bm{w}} & \tilde{\bm{\sigma}}, \, \tilde{\bm{v}}  \\
      \bm{0}_{3 \times 3} & \tilde{\bm{\kappa}}, \, \tilde{\bm{w}}
    \end{bmatrix} \, ,
\end{equation}
\begin{equation} \label{eq:logSE3_definition}
    \begin{split}
        &\log_{SE(3)} \left(\bm {g}\right) = \beta \left( \alpha_0 \bm{I}_4 - \alpha_1 \bm{g} + \alpha_2 \bm{g}^2 - \alpha_3 \bm{g}^3\right) \, ,
    \end{split}
\end{equation}
where $\beta = \frac{1}{8}\csc ^{3}\left(\frac{\theta}{2}\right)\sec \left(\frac{\theta}{2}\right)$, $\alpha_0 = \theta \cos \left(2\theta \right) - \sin \left(\theta \right)$, $\alpha_1 = \theta \cos \left(\theta \right)+2\theta \cos \left(2\theta \right)-\sin \left(\theta \right)-\sin \left(2\theta \right)$, $\alpha_2 = 2\theta \cos \left(\theta \right)+\theta \cos \left(2\theta \right)-\sin \left(\theta \right)-\sin \left(2\theta \right)$, $\alpha_3 = \theta \cos \left(\theta \right)-\sin \left(\theta \right)$, and
$\theta = \arccos\left(\frac{1}{2} \mathrm{tr}\left(\bm{g}\right) - 1\right)$.
\begin{equation} \label{eq:distso3_definition}
    \textnormal{dist}_{SO(3)}\left(\bm{R}_1, \bm{R}_2\right) = \abs{\arccos\left[\frac{1}{2}\left(\mathrm{tr}\left(\Delta\bm{R}\right) - 1\right)\right]} ,
\end{equation}
where $\Delta\bm{R} = \bm{R}_1^{\top} \bm{R}_2$.
\begin{equation} \label{eq:distse3_defintion}
    \textnormal{dist}_{SE(3)}\left(\bm{g}_1, \, \bm{g}_2\right) = \norm{\log_{SE(3)}\left(\bm{g}_{1}^{-1} \bm{g}_2\right)^{\vee}}_2 \, ,
\end{equation}

\section*{Functional Basis for \ac{GVS}}
\textit{Polynomial Basis}:
\begin{equation} \label{eq:polynomial_basis}
    \xi_i(s, t) - \xi_i^{*}(s) = \sum_{h = 0}^{n - 1} q_h s^{h} \, ,
\end{equation}
\textit{Fourier Basis}:
\begin{equation} \label{eq:fourier_basis}
    \xi_i(s, t) - \xi_i^{*}(s) = \sum_{h = 0}^{n - 1} q_{h, 1} \cos(h k) + q_{h, 2} \sin(h k) \, ,
\end{equation}
\textit{Gaussian Basis}:
\begin{equation} \label{eq:gaussian_basis}
    \xi_i(s, t) - \xi_i^{*}(s) = \sum_{h = 0}^{n - 1} q_{h} \exp\left(- \frac{\left(s - h/n\right)^{2}}{c^2} \right) \, ,
\end{equation}
where $c = \left(2 \sqrt{\ln\left(2\right)} n\right)^{-1}$.

%% Fourier Properties %%
\section*{Properties of Fourier Transform}
\begin{equation} \label{eq:fourier_definition}
    \fourier{f(t)} = F(j \omega) = \int_{-\infty}^{+\infty} f(t) \, e^{- j \omega t} \, \textnormal{d} t \, ,
\end{equation}
\begin{equation} \label{eq:fourier_linearity}
    \fourier{\alpha f(t) + \beta g(t)} = \alpha F(j \omega) + \beta G(j \omega) \, ,
\end{equation}
\begin{equation} \label{eq:fourier_delay}
    \fourier{f(t - T_0)} = F(j \omega) e^{-j \omega T_0}\, ,
\end{equation}
\begin{equation} \label{eq:fourier_diff}
    \fourier{\dot{f}(t)} = j \omega \, F(j \omega) \, ,
\end{equation}
\begin{equation} \label{eq:fourier_conv}
    \fourier{f(t) \cdot g(t)} = F(j \omega) \ast G(j \omega) \, ,
\end{equation}
\begin{equation} \label{eq:fourier2d_product}
    \fourier{f(s, t) = g(s) \cdot h(t)} = G(j k) \cdot H(j \omega) \, ,
\end{equation}
\begin{equation} \label{eq:fourier_parseval}
    \int_{-\infty}^{+\infty} \abs{f(t)}^2 \, \textnormal{d}t = \frac{1}{2 \pi} \int_{-\infty}^{+\infty} \abs{F(j \omega)}^2 \, \textnormal{d} \omega \, .
\end{equation}