This section provides a numerical example of the result of section \ref{Section LMI}.
%an example to show how to determine stability of the system using Theorem \ref{Theorem Exponential decay} and Section VII. 
%
% Let the plant and controller be defined as
% \begin{equation*}
% \begin{aligned}
%     \left[ \begin{smallmatrix} 
%         \dot{x}_p \\ \epsilon \dot{z}_p
%     \end{smallmatrix} \right]
%     &=
%     \left[ \begin{smallmatrix} 
%         A_{11}^p & A_{12}^p \\
%         A_{21}^p & A_{22}^p
%     \end{smallmatrix} \right]
%     \left[ \begin{smallmatrix} 
%         x_p \\ z_p
%     \end{smallmatrix} \right] 
%     + 
%     \left[ \begin{smallmatrix} 
%         A_{13}^p \\ A_{23}^p
%     \end{smallmatrix} \right]
%         \hat{u}_s ,
%     \\
%      y_f
%     &=
%     \left[ \begin{smallmatrix} 
%          A_x^{p_f} & A_z^{p_f}
%     \end{smallmatrix} \right]
%     \left[ \begin{smallmatrix} 
%         x_p \\ z_p
%     \end{smallmatrix} \right],
%     \\ 
%     \dot{x}_c 
%     &=
%     A_{11}^c 
%      x_c 
%     + 
%     A_{14}^c 
%    \hat{y}_f,
%     \quad 
%     u_s
%     =
%     A_x^{c_s}
%     x_c .
% \end{aligned}
% \end{equation*}
% %
Consider system \eqref{eqn: linear plant and controller} with
where $A_{11}^p = a_1$, 
$A_{12}^p = \left[ \begin{smallmatrix}
    a_2 & 0
\end{smallmatrix} \right]$,
$A_{21}^p = \left[ \begin{smallmatrix}
    0 \\ a_3
\end{smallmatrix} \right]$,
$A_{22}^p = \left[ \begin{smallmatrix}
    -a_2 & 0 \\ -a_2 & -a_4
\end{smallmatrix} \right]$,
$A_{13}^p = n_1$,
$A_{23}^p = \left[ \begin{smallmatrix}
    -n_2 \\ -n_2
\end{smallmatrix} \right]$,
$A_{x}^{p_f} = 1$,
$A_{z}^{p_f} = \left[ \begin{smallmatrix}
    0 & 1
\end{smallmatrix} \right]$,
$A_{11}^c = -a_5$,
$A_{14}^c = a_6$,
$A_{x}^{c_s}= -k$,
%
$a_1 =10^{-4}$, $a_2 = 0.2$, $a_3 = 0.6$, $a_4 = 0.73$, $a_5 = 1.11$, $a_6 = 0.37$, $k = 1.5$, $n_1 = 0.02$ and $n_2 = 0.0018$ are designed such that the controller stabilizes the plant under perfect communication. 

%Let $x = (x_p, x_c)$, $z = z_p$, $e_s = e_{u_s}\coloneqq \hat{u}_s - u_s$ and $e_f = e_{y_f}  \coloneqq \hat{y}_f - y_f$, then 
The hybrid model $\mathcal{H}_1$ is given by \eqref{eqn:full system}. We note that our plant and controller are simpler compared to \eqref{eqn: linear plant and controller}, since $u_f$, $y_s$ and $z_c$ does not exist in the system, nor do matrices such as $A_{14}^p$, $A_x^{p_s}$, $A_{21}^c$, etc. Consequently, the flow map $F$ in $\mathcal{H}_1$ has to be modified accordingly. Specifically, we have 
$A_{11} = \left[\begin{smallmatrix}A_{11}^p & A_{13}^p A_x^{c_s}\\ A_{14}^c A_x^{p_f} & A_{11}^c \end{smallmatrix} \right]$, 
%
$A_{12} = \left[\begin{smallmatrix}  A_{13}^p \\ 0\end{smallmatrix}\right]$,
%
$A_{13} = \left[\begin{smallmatrix} A_{12}^p  \\ A_{14}^c A_z^{p_f} \end{smallmatrix} \right]$,
%
$A_{14} = \left[ \begin{smallmatrix}0 \\ A_{14}^c\end{smallmatrix} \right]$,
%
$A_x^s = \left[\begin{smallmatrix}
     0 & -A_x^{c_s}
\end{smallmatrix} \right]$,
$A_x^f = \left[\begin{smallmatrix}
    -A_x^{p_f} & 0
\end{smallmatrix} \right]$, 
$A_z^f = -A_z^{p_f}$, 
%
$A_{31} = \left[\begin{smallmatrix}
    A_{21}^p & A_{23}^p A_x^{c_s}
\end{smallmatrix}\right]$,
%
$A_{32} = A_{23}^p$,
%
$A_{33} = 
    A_{22}^p$,
%
$A_{34} = 0$.
%with $f_x(x,z,e_s,e_f) = \big(a_1 x_p  + a_2 z_1 -n_1 k x_c + n_1e_s, -a_5 x_c + a_6 x_p+a_6 z_2+a_6 e_f \big)$, $f_{e_s}(x,z,e_s,e_f) = -a_5 k x_c + a_6 k(x_p + z_2 + e_f)$, $g_z(x,z,e_s,e_f) = (-a_2 z_1 + n_2 k x_c - n_2 e_s, a_3 x_p - a_2 z_1 - a_4 z_2 + n_2 k x_c -n_2 e_s )$ and $g_{e_f}(x,z,e_s,e_f,\epsilon) = -\epsilon (a_1 x_p  + a_2 z_1 - n_1 k x_c + n_1 e_s ) - (a_3 x_p - a_2 z_1 - a_4 z_2 + n_2 k x_c - n_2 e_s )$. 
%
% 
%By \eqref{eqn: H bar linear}, we have $\overline{H}(x,e_s) = \big(\tfrac{n_2}{a_2}(k x_c - e_s), \tfrac{a_3}{a_4}x_p\big)$. We define $y \coloneqq z - \overline{H}(x,e_s) $. 
%
%$h_y(x,e_s,y) = (y_1 - \tfrac{n_2}{a_2} e_s, y_2)$ by \eqref{eqn: h_y linear}. 
%
Then by \eqref{eqn: linear functions} we have
$A_{11}^s = \left[\begin{smallmatrix} a_1 & -\overline{n} k \\ a_6(1+\tfrac{a_3}{a_4}) & -a_5\end{smallmatrix} \right]$, 
$A_{12}^s = \left[\begin{smallmatrix} \overline{n}  \\ 0\end{smallmatrix} \right]$,
$A_{21}^s = \left[\begin{smallmatrix} a_6(1+\tfrac{a_3}{a_4})k & -a_5k \end{smallmatrix} \right]$, 
%$A_{22}^s = 0$,
$A_{11}^f = \left[\begin{smallmatrix} -a_2 & 0 \\ -a_2 & -a_4\end{smallmatrix} \right]$ and
$A_{12}^f = \left[\begin{smallmatrix} 0  \\ 0\end{smallmatrix} \right]$,
$A_{21}^f = \left[\begin{smallmatrix} a_2 & a_4 \end{smallmatrix} \right]$
%and $A_{22}^f = 0$,
where
$\overline{n} \coloneqq n_1 - n_2$.
% \begin{equation*}
%     \mathcal{H}_r \!: \! 
%     \begin{cases}
%     \begin{aligned} % Used to align \right\}
%     \left.
%     \begin{aligned} %Used to align flow map
%     \dot{x}_p &= x_p + (-k x_c + e_s)\\
%     \dot{x}_c &= 2a x_p-a x_c,\; \dot{e}_{s}=2ak x_p - ak x_c  \\
%     \dot{\tau}_s &= 1, \;  \dot{\kappa}_s = 0 \\
%     \end{aligned}
%     \right\}
%     & \begin{aligned}&\text{when } \\ & \xi^y \in \mathcal{C}_{2,r}^{y,0}\end{aligned} 
%     \\[1mm]
%     \left. 
%     \begin{aligned}
%     x^+ &= x,\;  e_{s}^+ = 0
%     \\
%     \tau_s^+ &= \tau_s, \; \kappa_s^+ = \kappa_s + 1
%     \end{aligned}
%     \qquad \qquad \qquad  \right\} 
%     &\begin{aligned}&\text{when } \\ & \xi^y \in \mathcal{D}_s^{y,0}.\end{aligned}
%     \end{aligned}
%     \end{cases}
%     %\label{eqn: example reduced system}
% \end{equation*}

%%%%%%%%%%%%%%%
%
Next, we find Lyapunov functions $W_s$ and $W_f$ in Claim \ref{Claim for LTI section}.
%
% First, we show that Assumption \ref{Assumption reduced model}, along with \eqref{eqn: Ws exponential sandwich bound} and \eqref{eqn: Vs exponential sandwich bound} in Assumption \ref{Assumption Exponential}, hold. 
% We write the flow map of $\mathcal{H}_r$ in the following state-space form:
% \begin{equation*}
%     \left[ \begin{smallmatrix} 
%         \dot{x} \\ \dot{e}_s
%     \end{smallmatrix} \right]
%     =
%     \left[ \begin{smallmatrix} 
%         A_{11}^s & A_{12}^s \\ A_{21}^s & 0
%     \end{smallmatrix} \right]
%     \left[ \begin{smallmatrix} 
%         x \\ e_s
%     \end{smallmatrix} \right],
% \end{equation*}
% where $A_{11}^s = \left[\begin{smallmatrix} a_1 & -\overline{n} k \\ a_6(1+\tfrac{a_3}{a_4}) & -a_5\end{smallmatrix} \right]$, $A_{12}^s = \left[\begin{smallmatrix} \overline{n}  \\ 0\end{smallmatrix} \right]$, $A_{21}^s = \left[\begin{smallmatrix} a_6(1+\tfrac{a_3}{a_4})k & -a_5k \end{smallmatrix} \right]$ and $\overline{n} \coloneqq n_1 - n_2$.
%
Since both $u_s$ and $y_f$ are scalars, the protocols are given by $h_s(\kappa_s, e_s) = 0$ and $h_f(\kappa_f, e_f) = 0$, which are UGES protocols. 
Let $W_s(\kappa_s,e_s) \coloneqq |e_s|$, then \eqref{eqn: NCS assumption Ws sandwich bound} and \eqref{eqn: Ws exponential sandwich bound} hold with $\underline{a}_{W_s}(s) = \overline{a}_{W_s}(s) = s$, \eqref{eqn: NCS assumption Ws jump} and \eqref{eqn: NCS Ws dot} hold for $\lambda_s = 0 $, $L_s = 0$ and $A_{H_s} = A_{21}^s$. 
%
%\aim{Let $P_s = \left[\begin{smallmatrix} p_{11}^s & p_{12}^s \\ p_{12}^s & p_{22}^s\end{smallmatrix} \right] > 0$, $V_s(x) = x^\top P_s x$, then \eqref{eqn: Vs exponential sandwich bound} is satisfied with $\underline{a}_{V_s} = \lambda_{\text{min}}(P_s)$ and $\overline{a}_{V_s} = \lambda_{\text{max}}(P_s)$.}
% \aim{Moreover, we can calculate that 
% \begin{equation}
%     \begin{aligned}
%         &\left< \tfrac{\partial {V_s}(x)}{\partial x},f_x(x,\overline{H}(x,e_s),e_s, 0) \right> \\ 
%         = & x^\top(A_{11}^{s^\top} P_s + P_s A_{11})x + e_s^\top A_{12}^{s^\top} P_s x + x^\top P_s A_{12}^s e_s .
%     \end{aligned}
%     \label{eqn: Example Vs equation 1}
% \end{equation}
% On the other hand, by \eqref{eqn: NCS Vs flow} in Assumption \ref{Assumption reduced model} and the $a_{\rho_s}s^2 \leq \rho_s(s)$ in Assumption \ref{Assumption Exponential}, we want
% %
% \begin{equation}
%     \begin{aligned}
%         &\left< \tfrac{\partial {V_s}(x)}{\partial x},f_x(x,\overline{H}(x,e_s),e_s, 0) \right> \\
%         \leq & -a_{\rho_s} x^\top x -a_{\rho_s} e_s^\top e_s - x^\top A_{21}^{s^\top} A_{21}^s x + \gamma_s^2 e_s^\top e_s .
%     \end{aligned}
% \end{equation}
% By substituting \eqref{eqn: Example Vs equation 1} into the above equation, we get
% $
% \left[\begin{smallmatrix}
%     x \\ e_s
% \end{smallmatrix}\right]^\top 
% \Gamma_s
% \left[\begin{smallmatrix}
%     x \\ e_s
% \end{smallmatrix}\right]
% < 0
% $,
% where $$\Gamma_s = \left[ \begin{smallmatrix} 
%     A_{11}^{s^\top} P_s + P_s A_{11}^s + a_{\rho_s} I + A_{21}^{s^\top} A_{21}^s & P_s A_{12}^s \\
%     A_{12}^{s^\top} P_s & (a_{\rho_s} - \gamma_s^2)I
% \end{smallmatrix} \right]. $$
% Then \eqref{eqn: NCS Vs flow} is satisfied if $\Gamma_s$ is negative definite.
% }
%
%
%
% The flow map of the boundary-layer system can be written in the following state-space form:
% \begin{equation*}
%     \left[ \begin{smallmatrix} 
%         \tfrac{\partial y}{\partial \sigma} \\ \tfrac{\partial e_f}{\partial \sigma}
%     \end{smallmatrix} \right]
%     =
%     \left[ \begin{smallmatrix} 
%         A_{11}^f & A_{12}^f \\ A_{21}^f & 0
%     \end{smallmatrix} \right]
%     \left[ \begin{smallmatrix} 
%         y \\ e_f
%     \end{smallmatrix} \right],
% \end{equation*}
% where $A_{11}^f = \left[\begin{smallmatrix} -a_2 & 0 \\ -a_2 & -a_4\end{smallmatrix} \right]$, $A_{12}^f = \left[\begin{smallmatrix} 0  \\ 0\end{smallmatrix} \right]$ and $A_{21}^f = \left[\begin{smallmatrix} a_2 & a_4 \end{smallmatrix} \right]$.
%
%
Let $W_f(\kappa_f,e_f) \coloneqq |e_f|$, then \eqref{eqn: NCS assumption Wf sandwich bound} and \eqref{eqn: Wf exponential sandwich bound} hold with $\underline{a}_{W_f}(s) = \overline{a}_{W_f}(s) = s$, \eqref{eqn: NCS assumption Wf jump} and \eqref{eqn: NCS Wf dot} hold for $\lambda_f = 0 $, $L_f = 0$ and $A_{H_f} = A_{21}^f$. 
% \cyan{Let $P_f = \left[\begin{smallmatrix} p_{11}^f & p_{12}^f \\ p_{12}^f & p_{22}^f\end{smallmatrix} \right] > 0$, $V_f(y) = y^\top P_f y$, \eqref{eqn: Vf exponential sandwich bound} holds with $\underline{a}_{V_f} = \lambda_{\text{min}}(P_f)$ and $\overline{a}_{V_f} = \lambda_{\text{max}}(P_f)$. Moreover, we can show that
% \begin{equation}
%     \begin{aligned}
%         &\left< \tfrac{\partial {V_f}(x,y)}{\partial y},g_z(x,y+ \overline{H}(x, e_s),e_s,e_f)  \right> \\
%         =& y^\top (A_{11}^{f^\top} P_f + P_f A_{11}^f) y.
%         \label{eqn: example Vf equation 1}
%     \end{aligned}
% \end{equation}
% By \eqref{eqn: NCS Vf flow} from Assumption \ref{Assumption boundary layer system} and $a_{\rho_f} s^2 \leq \rho_f(s)$ from Assumption \ref{Assumption Exponential}, we need
% \begin{equation*}
%     \begin{aligned}
%          &\left< \tfrac{\partial {V_f}(x,y)}{\partial y},g_z(x,y+ \overline{H}(x, e_s),e_s,e_f)  \right> \\
%          \leq & -a_{\rho_f} y^\top y - a_{\rho_f} e_f^\top e_f - y^\top A_{21}^{f^\top} A_{21}^f y + \gamma_f^2 e_f^\top e_f.
%     \end{aligned}
% \end{equation*}
% By substituting \eqref{eqn: example Vf equation 1} into the above inequality, we have 
% $
% \left[\begin{smallmatrix}
%     y \\ e_f
% \end{smallmatrix}\right]^\top 
% \Gamma_f
% \left[\begin{smallmatrix}
%     y \\ e_f
% \end{smallmatrix}\right]
% < 0
% $,
% where $$\Gamma_f = \left[ \begin{smallmatrix} 
%     A_{11}^{f^\top} P_f + P_f A_{11}^f + a_{\rho_f} I + A_{21}^{s^\top} A_{21}^s & P_f A_{12}^f \\
%     A_{12}^{f^\top} P_f & (a_{\rho_f} - \gamma_f^2)I
% \end{smallmatrix} \right]. $$
% Then \eqref{eqn: NCS Vf flow} is guaranteed
% if $\Gamma_f$ is negative definite.
% }



% Next, we show that Assumption \ref{Assumption interconnection Exponential} holds.
% Let $U_s$ and $U_f$ be defined by \eqref{eqn: Us and Uf}. Suppose Assumptions \ref{Assumption reduced model}, \ref{Assumption boundary layer system} and \ref{Assumption Exponential} holds, we can show $\left< \tfrac{\partial U_s}{\partial \xi_s}, F_s^y(x,0,e_s,0) \right> \leq a_s \psi_s^2(|(x,e_s)|)$ and $\left< \tfrac{\partial U_f}{\partial \xi_f}, F_f^y(x,y,e_s,e_f,0) \right> \leq a_f \psi_f^2(|(y,e_f)|)$, where $a_s = a_{\rho_s}$, $\psi_s(s) = s$, $a_f = a_{\rho_f}$ and $\psi_f(s) = s$.
%
Since $W_s(x,e_s) = |e_s|$, we have $\left|\tfrac{\partial W_s(\kappa_s,e_s)}{\partial e_s} \right| \leq L_1$ where $L_1 = 1$. Then by \eqref{eqn: Lambda_b1}, we have 
$
    \Lambda_{b_1} = 2
            \left[ \begin{smallmatrix}
            a_2 |p_{11}^s| & a_6 |p_{12}^s|                    & 0 \\
            a_2 |p_{12}^s| & 0                               & a_6 |p_{22}^s| \\
            0          & \tfrac{\gamma_s}{\lambda_s^*}a_6k & \tfrac{\gamma_s}{\lambda_s^*}a_6k
        \end{smallmatrix} \right]$
%
% such that 
% \begin{equation*}
%     \begin{aligned}
%         &\Big < \tfrac{\partial {U_s}}{\partial \xi_s}, F_s^y(x,y,e_s,e_f) - F_s^y(x,0,e_s,0)  \Big> \\
%         \leq & 
%     \left[ \begin{smallmatrix} 
%         |x_1| \\ |x_2| \\ |e_s|
%     \end{smallmatrix} \right]^\top
%     \Lambda_{b_1}
%     \left[ \begin{smallmatrix} 
%         |y_1| \\ |y_2| \\ |e_f|
%     \end{smallmatrix} \right]
%         \\
%         \leq & b_1 \psi_s(|(x,e_s)|) \psi_f(|(y,e_f)|),
%     \end{aligned}
% \end{equation*}
and $b_1 = \sqrt{\lambda_{\text{max}} (\Lambda_{b_1}^\top \Lambda_{b_1})}$. Similarly, we can show that $b_2 = \sqrt{\lambda_{\text{max}}(\Lambda_{b_2}^\top \Lambda_{b_2}) }$ and $b_3 = \lambda_{\text{max}}(\Lambda_{b_3})$ satisfy \eqref{eqn: Lambda_b2 and Lambda_b3}, where %$\Lambda_{b_2}$ and $\Lambda_{b_3}$ are given below. 
$
        \Lambda_{b_2} = 2 
        \left[ \begin{smallmatrix} 
            a_1 \tfrac{a_3}{a_4} |p_{12}^f|   &  a_1 \tfrac{a_3}{a_4} |p_{22}^f| & a_1 \tfrac{\gamma_f}{\lambda_f^*} \\
            \tfrac{a_3}{a_4} \overline{n} k |p_{12}^f| & \tfrac{a_3}{a_4} \overline{n} k |p_{12}^f|& \overline{n} k \tfrac{\gamma_f}{\lambda_f^*} \\
            \tfrac{a_3}{a_4}\overline{n} |p_{12}^f|   &  \tfrac{a_3}{a_4} \overline{n}|p_{22}^f| & \overline{n}\tfrac{\gamma_f}{\lambda_f^*}
        \end{smallmatrix} \right]$ 
        and
        $\Lambda_{b_3}=
        \left[ \begin{smallmatrix} 
            2  a_2 \tfrac{a_3}{a_4} |p_{12}^f| & \star & \star \\
            a_2 \tfrac{a_3}{a_4} |p_{22}^f|   &     0      &                \star              \\
            a_2 \tfrac{\gamma_f}{\lambda_f^*} & 0 &        0              
        \end{smallmatrix} \right].$
% such that 
% \begin{equation*}
%     \begin{aligned}
%         & \Big< \tfrac{\partial {U_f}}{\partial \xi_s} - \tfrac{\partial {U_f}}{\partial y} \tfrac{\partial \overline{H}}{\partial \xi_s} - \tfrac{\partial {U_f}}{\partial e_f} \tfrac{\partial \tilde k}{\partial \xi_s} ,  F_s^y(x,y,e_s,e_f) \Big> \\
%         \leq &
%         \left[ \begin{smallmatrix} 
%             |x_1| \\ |x_2| \\ |e_s|
%         \end{smallmatrix} \right]^\top
%         \Lambda_{b_2}
%         \left[ \begin{smallmatrix} 
%             |y_1| \\ |y_2| \\ |e_f|
%         \end{smallmatrix} \right]
%         + 
%         \left[ \begin{smallmatrix} 
%         |y_1| \\ |y_2| \\ |e_f|
%         \end{smallmatrix} \right]^\top
%         \Lambda_{b_3}
%         \left[ \begin{smallmatrix} 
%             |y_1| \\ |y_2| \\ |e_f|
%         \end{smallmatrix} \right]
%         \\
%         \leq & b_2 \psi_s(|(x,e_s)|) \psi_f(|(y,e_f)|) + b_3 \psi_f^2(|(y,e_f)|),
%     \end{aligned}
% \end{equation*}
% where $b_2 = \sqrt{\lambda_{\text{max}}(\Lambda_{b_2}^\top \Lambda_{b_2}) }$, $b_3 = \lambda_{\text{max}}(\Lambda_{b_3})$, and we show \eqref{eqn: SPNCS interconnection 2} is satisfied. 
%
Finally, by \eqref{eqn: lambda_1 and lambda_2}, we show that Assumption \ref{Assumption Vf at slow transmission} holds
% Since $h_y(x,e_s,y) = (y_1 - e_s, y_2)$, we have 
% \begin{equation*}
%     \begin{aligned}
%         &V_f(x, h_y(x,e_s,y)) - V_f(x,y) \\
%         =& -2 \tfrac{n_2}{a_2} (p_{11}^f y_1 + p_{12}^f y_2) e_s +  \tfrac{n_2}{a_2}^2p_{11}^f e_s^2 \\
%         \leq & \lambda_1 W_s^2(\kappa_s,e_s) + \lambda_2 \sqrt{V_f(x,y) W_s^2(\kappa_s, e_s)} ,
%     \end{aligned}
% \end{equation*}
with $\lambda_1 = \tfrac{n_2}{a_2}^2|p_{11}^f|$ and $\lambda_2 = \tfrac{2\frac{n_2}{a_2}(|p_{11}^f| + |p_{12}^f|)}{\sqrt{\lambda_\text{min}(P_f)}}$.


%Now we have shown that Assumptions \ref{Assumption Vf at slow transmission} and \ref{Assumption interconnection Exponential} hold if Assumption \ref{Assumption reduced model}, \ref{Assumption boundary layer system} and \ref{Assumption Exponential} hold. Then we start looking for the value of unknown variables that satisfy the above-mentioned Assumptions.


We want to satisfy the LMI \eqref{eqn: LMIs} for all $\ell \in \{s,f\}$ and maximize $T(L_s,\gamma_s, \lambda_s^*)$, $T(L_f,\gamma_f, \lambda_f^*)$, $\epsilon^*$ under the following constraints: $P_s > 0$, $\gamma_\star > 0$, $a_{\rho_\star} > 0$, $\gamma_\star>0$, $\lambda_\star^* \in (0,1)$ and $\Lambda_\star < 0$ for $\star \in \{s,f\}$. We note that $\epsilon^*$ is given by \eqref{eqn: epsilon star} with $d = d^*$ defined by \eqref{eqn: d star exponential}.
%
We pose this problem as an optimisation problem with constraints (see \cite{Github_SPNCS_illustrative_example} for the problem fomulation and the code), we get $P_s = \left[\begin{smallmatrix} 54.91  & -1.76\\ -1.76 & 1.81\end{smallmatrix} \right]$, $\gamma_s = 2.58$, $\lambda_s^* = 0.33$, $a_{\rho_s} = 1.16$, $P_f = \left[\begin{smallmatrix} 1.12  & 0.018\\ 0.018 & 0.65\end{smallmatrix} \right]$, $\gamma_f = 0.64$, $\lambda_f^* = 0.46$, $a_{\rho_f} = 0.41$, $T(L_s,\gamma_s, \lambda_s^*) = 360.1 \ ms$ and $T(L_f,\gamma_f, \lambda_f^*) = 1.11 \ \tfrac{s}{\epsilon}$ (in fast time scale $\sigma$). By selecting $\tau_{\text{miati}}^{s} = 324.1 \ ms$ and $\mu = 0.66 a_s \underline{a}_{U_s}$, we have $\epsilon^* = 0.0162$, see the proof of Theorem \ref{Theorem Exponential decay} and \cite{Github_SPNCS_illustrative_example} for more detail.
%
%
This implies $\mathcal{H}_1$ is UGES if $\epsilon < \epsilon^*$, $\tau_{\text{miati}}^s = 324.1 \ ms$, $\tau_{\text{mati}}^s = 360.1 \ ms$ and $\tau_{\text{mati}}^f \leq 18 \ ms$. Finally, we have $\tau_{\text{miati}}^f \leq 9\ ms$ such that \eqref{eqn: condition on miati^f} is satisfied.




% \begin{figure}[H]
%     \centering
%     \includegraphics[width = 0.8\linewidth]{Figures/Illustrative Example.png}
%     \caption{Example simulation}
%     \label{fig: Example Simulation}
% \end{figure}
















% Let $\phi_{\star} = -2L_\star \phi_\star - \gamma_\star(\phi_\star^2 + 1)$, $\phi_\star(0) = \lambda_\star^*$ and $U_\star = V_\star + \gamma_\star \phi_\star(\tau_\star)W_\star^2(e_\star)$ for $\star \in \{s, f\}$, and we let $\lambda_s^* = 0.4$ and $\lambda_f^* = 0.6$. By Assumptions \ref{Assumption reduced model}, \ref{Assumption boundary layer system} and the definition of $\phi_\star$, inequalities (\ref{eqn: Us}) and (\ref{eqn: Uf}) hold with $a_s=1$, $a_f = 0.5$, $\psi_s(s) = s$, $\psi_f(s) = s$.
% Then inequality (\ref{eqn: SPNCS interconnections}) holds with $b_1 = 293.61, b_2 = 11.25, b_3 = 4.36$.

% % \underline{Assumption \ref{Assumption U_f slow jump}}: Since $U_f$ is independent to $\xi_s$, Assumption \ref{Assumption U_f slow jump} immediately holds.

% Now that we have verified all the assumptions, we can compute $\epsilon^*   = 0.000151$, $T(L_s, \gamma_s, \lambda_s^*) = 0.0707$ and $T(L_f, \gamma_f, \lambda_f^*) = 0.6929$, and the required MATIs to stabilise the system are given by $\tau_{\text{mati}}^s \leq 0.0707$ and $\tau_{\text{mati}} \leq 0.6929\epsilon$.


