\newpage
\textbf{Proof of Corollary \ref{Corollary Exponential decay}:} The first step is to show the $\psi_s$ and $\psi_f$ in Lemma \ref{Lemma MATI} are linear. By the definition of $U_s$, \eqref{eqn: NCS Ws dot} and \eqref{eqn: NCS Vs flow}, we have
\begin{equation*}
    \begin{aligned}
        & U_s^\circ(\xi_s; F_s^y(x,0,e_s, 0)) \\
        \leq &\left< \tfrac{\partial V_s}{\partial x}, f_x(x,\overline{H}(x,e_s),e_s,0)\right> \\
            & + \gamma_d \Big( -2 L_s \phi_s(\tau_s) - \gamma_d \big(\phi_s^2(\tau_s)+1\big) \Big) W_s^2(\kappa_d, e_s) \\
            &+ 2 \gamma_d\phi_s W_s(\kappa_d,e_s) \left< \tfrac{\partial {W_s}(\kappa_d,{e_s})}{\partial {e_s}}, f_{e_s}(x,\overline{H}(x,e_s),e_s, 0)\right> \\
        \leq & - \rho_s(|x|) - \rho_s\left(W_s(\kappa_d, e_s)\right) - H_s^2(x,e_s) + \gamma_d^2 W_s^2(\kappa_d, e_s) \\
            &+ \gamma_d \Big( -2 L_s \phi_s(\tau_s) - \gamma_d \big(\phi_s^2(\tau_s)+1\big) \Big) W_s^2(\kappa_d, e_s) \\
            &+ 2 \gamma_d \phi_s(\tau_s) W_s(\kappa_d, e_s)\big(L_s {W_s}(\kappa_d, e_s)  + H_s(x,e_s) \big)  \\
        \leq & - \rho_s(|x|) - \rho_s\left(W_s(\kappa_d, e_s)\right) \\
            &- \big(H_s(x,e_s) - \gamma_d \phi_s(\tau_s)W_s(\kappa_d, e_s)\big)^2 \\
        \leq & - \rho_s(|x|) - \rho_s\left(W_s(\kappa_d, e_s)\right).
    \end{aligned}
\end{equation*}
Additionally, since $a_{\rho_s} s^2 \leq \rho_s(s)$ for all $s \in \mathbb{R}$, we have
\begin{equation}
    U_s^\circ(\xi_s; F_s^y(x,0,e_s, 0)) \leq -a_{\rho_s} |x|^2 - a_{\rho_s} W_s^2(\kappa_d, e_s)
\end{equation}
Then by \eqref{eqn: Ws exponential sandwich bound}, we have
\begin{equation*}
    \begin{aligned}
        &U_s^\circ(\xi_s; F_s^y(x,0,e_s, 0)) \\
        \leq & - \big(a_{\rho_s} |x|^2 + a_{\rho_s} W_s^2(\kappa_d,e_s)\big) \\
        \leq & - \big(a_{\rho_s} |x|^2 + a_{\rho_s} \underline{a}_{W_s}^2 |e_s|^2\big) \\
        \leq & - a_{\rho_s} \min \{ 1, \underline{a}_{W_s}^2 \} (|x|^2+|e_s|^2) \\
        \eqqcolon & - a_s \psi_s^2(|(x,e_s)|),
    \end{aligned}
\end{equation*}
which implies \eqref{eqn: Us flow} is satisfied with $a_s \coloneqq a_{\rho_s} \min \{ 1, \underline{a}_{W_s}^2 \}$ and $\psi_s(|(x,e_s)|) \coloneqq |(x,e_s)|$. 

Moreover, we have $$\underline{a}_{U_s}|(x,e_s)|^2 \leq U_s(\xi_s) \leq \overline{a}_{U_s}|(x,e_s)|^2,$$ where $\underline{a}_{U_s} \coloneqq \min\{\underline{a}_{V_s}, \gamma_s \lambda_s^* \underline{a}_{W_s}^2 \}$ and $\overline{a}_{U_s} \coloneqq \max\{\overline{a}_{V_s}, \gamma_s \tfrac{1}{\lambda_s^*} \overline{a}_{W_s}^2 \}$.

By following the same line as $U_s$, we can proof that \eqref{eqn: Uf flow} is satisfied with $a_f \coloneqq a_{\rho_f} \min \{ 1, \underline{a}_{W_f}^2 \}$ and $\psi_f(|(y,e_f)|) \coloneqq |(y,e_f)|$. Moreover, we have $$\underline{a}_{U_f}|(y,e_f)|^2 \leq U_f(\xi_s, \xi_f) \leq \overline{a}_{U_f}|(y,e_f)|^2,$$ where $\underline{a}_{U_f} \coloneqq \min\{\underline{a}_{V_f}, \gamma_f \lambda_f^* \underline{a}_{W_f}^2 \}$ and $\overline{a}_{U_f} \coloneqq \max\{\overline{a}_{V_f}, \gamma_f \tfrac{1}{\lambda_f^*} \overline{a}_{W_f}^2 \}$. Then we have 
\begin{equation}
\begin{aligned}
    \psi_s(|(x,e_s)|) &\leq a_{\psi_s}\sqrt{U_s(\xi_s)}, \\
    \psi_f(|(y,e_f)|) &\leq a_{\psi_f}\sqrt{U_f(\xi_s,\xi_f)} ,
\end{aligned}
\label{eqn: upper bound of psi}
\end{equation}
where $a_{\psi_s} = \underline{a}_{U_s}^{-\frac{1}{2}}$ and $a_{\psi_f} = \underline{a}_{U_f}^{-\frac{1}{2}}$.






Same as the proof of Theorem \ref{Theorem H_1}, we define composite Lyapunov function $U$ as $U(\xi_s, \xi_f) \coloneqq U_s(\xi) + d U_f(\xi_s,\xi_f)$, where $d \in (0,1)$. The Lyapunov function $U$ has sandwich bound 
\begin{equation}
    \underline{a}_{U} |\xi^y|_{\mathcal{E}^y}^2 \leq U(\xi^y) \leq \overline{a}_{U} |\xi^y|_{\mathcal{E}^y}^2, \label{eqn: Exponential U sandwich bound}
\end{equation}
where $\underline{a}_{U} \coloneqq \min \{\underline{a}_{U_s}, d \underline{a}_{U_f} \}$ and $\overline{a}_{U} \coloneqq \max \{\overline{a}_{U_s}, d \overline{a}_{U_f} \}$. 


We are now ready to find an exponential $\mathcal{KL}$ bound for $U$. The proof has three parts. Firstly, we will find an upper bound of $U$ during the interval between two slow transmissions. Secondly, we will find an upper bound of $U$ at each slow transmissions. Thirdly, we provide an overall upper bound in Claim $\ref{Claim U upper bound}$.



\noindent\emph{\underline{During flow}:} Since we have \eqref{eqn: Us flow} and \eqref{eqn: Uf flow}, by \cite[pp. 452]{nonlinear_systems_Khalil}, the time derivative of $U$ alone the trajectory $\xi^y$ is given by
\begin{equation*}
     U^\circ(\xi^y, F^y(\xi^y, \cyan{\epsilon})) \leq - 
     \begin{bmatrix}
         \psi_s(|(x,e_s)|) \\ \psi_f(|(y,e_f)|) 
     \end{bmatrix}^T \Lambda \begin{bmatrix}
         \psi_s(|(x,e_s)|) \\ \psi_f(|(y,e_f)|) 
     \end{bmatrix},
\end{equation*}
where $\Lambda \coloneqq \begin{bmatrix}
     a_s & -\tfrac{1}{2}(b_1 + d b_2) \\
    -\tfrac{1}{2}(b_1 + d b_2) & d (\tfrac{a_f}{\epsilon} - b_3)
\end{bmatrix}$. Then by \eqref{eqn: upper bound of psi}, we have
\begin{equation*}
    \begin{aligned}
        U^\circ(\xi^y, F^y(\xi^y, \cyan{\epsilon})) \leq - 
        \begin{bmatrix}
            \sqrt{U_s(\xi_s)} \\ \sqrt{U_f(\xi_s, \xi_f)}
        \end{bmatrix}^T
        \Lambda_1
        \begin{bmatrix}
            \sqrt{U_s(\xi_s)} \\ \sqrt{U_f(\xi_s, \xi_f)}
        \end{bmatrix},
    \end{aligned}
\end{equation*}
where $\Lambda \coloneqq 
    \begin{bmatrix}
        a_s a_{\psi_s}^2 & -\tfrac{1}{2}(b_1 + d b_2)a_{\psi_s}a_{\psi_f} \\
        -\tfrac{1}{2}(b_1 + d b_2)a_{\psi_s}a_{\psi_f} & d (\tfrac{a_f}{\epsilon} - b_3)a_{\psi_f}^2
    \end{bmatrix}$. 
Let $\mu_1 \in (0, a_s a_{\psi_s}^2)$. In order to satisfy $\Lambda_1 \geq \mu_1
    \begin{bmatrix}
        1 & 0 \\ 0 & d
    \end{bmatrix}$, we need 
    \begin{subequations}
\begin{align}
    a_s a_{\psi_s}^2 > \mu_1 \\
    (a_s a_{\psi_s}^2-\mu_1) \big( d (\tfrac{a_f}{\epsilon} - b_3)a_{\psi_f}^2 - \mu_1 d \big) &\geq \tfrac{1}{4}(b_1 + db_3)^2a_{\psi_s}^2a_{\psi_f}^2, \label{eqn: inequality of epsilon Exponential}
\end{align}
\end{subequations}
where the first inequality is satisfied by the definition of $\mu_1$, and the second inequality can be satisfied by taking $\epsilon$ sufficiently small.

Then we have 
\begin{equation}
    \begin{aligned}
        U^\circ(\xi^y, F^y(\xi^y, \cyan{\epsilon})) &\leq -\mu_1 (U_s(\xi_s) + d U_f(\xi_s,\xi_f)) \\
        & \leq - \mu_1 U(\xi^y)
    \end{aligned}
\end{equation}


\noindent\emph{\underline{During jumps}:} 

Same as the proof of Theorem \ref{Theorem H_1}, we can show at each slow transmission, we have
\begin{equation}
    U(G_s^y(\xi^y)) \leq a_d U(\xi^y),
    \label{eqn: Exponential U slow jump}
\end{equation}
where $a_d$ is defined in \eqref{eqn: U slow jump}. At each fast transmission, we have 
\begin{equation*}
    U(G_f^y(\xi^y)) \leq U(\xi^y).
\end{equation*}



By comparison principle \cite[Lemma 3.4]{nonlinear_systems_Khalil} and the fact that $U$ is non-increasing at fast transmissions, we have
\begin{equation}
    U(t,j) \leq U(t_k^s, j_k^s) \exp \! \big(-\mu_1(t-t_k^s) \big) \label{eqn: Exponential U flow}, 
\end{equation}
for all $(t_k^s, j_k^s) \preceq (t,j) \preceq (t_{k+1}^s, j_{k+1}^s - 1)$ and $(t,j)\in \text{dom}\ \xi$. We note that \eqref{eqn: Exponential U flow} corresponds to \eqref{eqn: beta 1} in the proof of Theorem \ref{Theorem H_1}.






Along the same line as deriving \eqref{eqn: flow then jump}, we have that for all $ k \in \mathbb{Z}_{\geq 1}$,
\begin{equation*}
    \begin{aligned}
        U(t^s_{k+1}, j^s_{k+1}) &\leq a_d U(t^s_{k+1},j^s_{k+1} - 1)
        \\
        &\leq a_d U(t_k^s, j_k^s) \exp (-\mu_1\tau_{\text{miati}}^s ).
    \end{aligned} 
\end{equation*}
By definition of $a_d$ (see \eqref{eqn: U slow jump}), we have that for any $\tau_{\text{miati}}^{s} \leq T(L_s, \gamma_s, \lambda_s^*)$, $\lambda \in (\exp (-\mu_1\tau_{\text{miati}}^s ), 1)$, there exist $d^* \in (0,1)$ such that if $d = (0, d^*]$, we have
\begin{equation*}
    U(t^s_{k+1}, j^s_{k+1}) \leq \lambda U(t^s_k,j^s_k)
\end{equation*}
for all $k \in \mathbb{Z}_{\geq 1}$. Let $d = d^*$.
By concatenation, we have
\begin{equation*}
    \begin{aligned}
        U(t^s_k, j^s_k) \leq & \lambda^{k-1}U(t_1^s, j_1^s),
    \end{aligned}
\end{equation*}
for all $k \in \mathbb{Z}_{\geq 1}$. 
%
Moreover, since $U$ is non-increasing during flow and upper bounded by \eqref{eqn: Exponential U slow jump} at slow transmission, we have $ U(t_1^s,j_1^s) \leq  a_d U(0,0) $. Then for all $k \in \mathbb{Z}_{\geq 0}$, we have
\begin{equation}
    U(t_k^s, j_k^s) \leq a_d \lambda^{k-1} U(0,0). \label{eqn: Exponential U slow jump decay}
\end{equation}

Now we have obtained the upper bound of trajectory during the interval between slow transmissions (i.e., \eqref{eqn: Exponential U flow}) and the upper bound at each slow transmission. We will now find an upper bound of $U$ for the whole trajectory.
\begin{claim}
    The following upper bound holds for all $(t_k^s, j_k^s) \preceq (t,j) \in \text{dom}\ \xi$
    \begin{equation*}
        U(t,j) \leq \frac{a_d}{\lambda}U(t_k^s,j_k^s)  \exp \!\left(-\tfrac{\ln{(\nicefrac{1}{\lambda})}}{\tau_{\text{mati}}^s}(t-t_k^s) \right). 
    \end{equation*}
    \label{Claim U upper bound}
\end{claim}
\textbf{Proof of Claim \ref{Claim U upper bound}:}
During flow, since $t_{k+1}^s - t_k^s \leq \tau_{\text{mati}}^s$, $a_d \geq 1$, $\lambda \in (0,1)$, $\tau_{\text{miati}}^s < \tau_{\text{mati}}^s$ and definition of $\lambda$, we have that for all $(t_k^s, j_k^s) \preceq (t,j) \preceq (t_{k+1}^s, j_{k+1}^s-1)$, we have
\begin{equation*}
    \begin{aligned}
        &\frac{a_d}{\lambda}U(t_k^s,j_k^s)  \exp \!\left(-\tfrac{\ln{(\nicefrac{1}{\lambda})}}{\tau_{\text{mati}}^s}(t-t_k^s) \right) \\
        \geq & U(t_k^s,j_k^s) \exp \!\left( -\ln{(\nicefrac{1}{\lambda})}\right)^{\tfrac{t-t_k^s}{\tau_{\text{mati}}^s}} \\
        = & U(t_k^s,j_k^s) \lambda^{\tfrac{t-t_k^s}{\tau_{\text{mati}}^s}} \\
        = &  U(t_k^s,j_k^s) \big(a_d \exp (-\mu_1 \tau_{\text{miati}}^s) \big)^{\tfrac{t-t_k^s}{\tau_{\text{mati}}^s}} \\
        = & U(t_k^s,j_k^s) {a_d}^{\tfrac{t-t_k^s}{\tau_{\text{mati}}^s}} \exp \! \big(-\mu_1 \tfrac{\tau_{\text{miati}}^s}{\tau_{\text{mati}}^s} (t - t_k^s)\big) \\
        \geq & U(t_k^s,j_k^s)\exp\!\big(-\mu_1 (t - t_k^s)\big) ,
    \end{aligned}
\end{equation*}
Then by \eqref{eqn: Exponential U flow}, we validate Claim \ref{Claim U upper bound} during the interval between slow transmissions. 

Next, we will check the upper bound at each slow transmission. Since $\tfrac{t_k^s}{\tau_{\text{mati}}^s} \leq k$, for all $k\in \mathbb{Z}_{\geq 0}$, we have 
\begin{equation*}
    \begin{aligned}
        & \frac{a_d}{\lambda}U(0,0)  \exp \!\left(-\tfrac{\ln{(\nicefrac{1}{\lambda})}}{\tau_{\text{mati}}^s}(t_k^s-0) \right) \\
        \geq & \frac{a_d}{\lambda}U(0,0)  \exp \!\left(-\ln{(\nicefrac{1}{\lambda})} k \right) \\
        = & a_d U(0,0) \lambda^{k-1}.
    \end{aligned}
\end{equation*}
 By \eqref{eqn: Exponential U slow jump decay}, we validate Claim \ref{Claim U upper bound} at slow transmissions. Then we have prove Claim \ref{Claim U upper bound}. $\hfill\square$

 By Claim \ref{Claim U upper bound}, we have 
 \begin{equation*}
     U(t,j) \leq \tfrac{a_d}{\lambda}U(0,0)  \exp \!\left(-\tfrac{\ln{(\nicefrac{1}{\lambda})}}{\tau_{\text{mati}}^s}t \right),
 \end{equation*}
 for all $(t,j) \in \text{dom} \ \xi$.
 By sandwich bound \eqref{eqn: Exponential U sandwich bound}, we have
 \begin{equation*}
     \begin{aligned}
         &|\xi^y(t,j)|_{\mathcal{E}^y}  \\
         \leq & \big(\tfrac{1}{\underline{a}_U} U(t,j)\big)^{\nicefrac{1}{2}} \\
         \leq & \left(\tfrac{a_d}{\lambda \underline{a}_U}U(0,0)  \exp \!\left(-\tfrac{\ln{(\nicefrac{1}{\lambda})}}{\tau_{\text{mati}}^s}t \right) \right)^{\nicefrac{1}{2}} \\
         \leq & \left(\tfrac{a_d}{\lambda \underline{a}_U} \overline{a}_U |\xi^y(0,0)|_{\mathcal{E}^y}^2  \exp \!\left(-\tfrac{\ln{(\nicefrac{1}{\lambda})}}{\tau_{\text{mati}}^s}t \right) \right)^{\nicefrac{1}{2}} \\    
         = & \left(\tfrac{a_d \overline{a}_U}{\lambda \underline{a}_U} \right)^{\nicefrac{1}{2}}  |\xi^y(0,0)|_{\mathcal{E}^y}  \exp \!\left(-\tfrac{\ln{(\nicefrac{1}{\lambda})}}{2 \tau_{\text{mati}}^s}t \right).
     \end{aligned}
 \end{equation*}

Since $\overline{H}$ is globally Lipschitz and $\overline{H}(0,0) = 0$, we have $\overline{H}(x,e_s) \leq L|(x,e_s)|$, where $L$ is the Lipschitz constant. 
% 
 Then by $y = z - \overline{H}(x,e_s)$, there exist $h_1 = 1 + L$ such that
 $|\xi(t,j)|_{\mathcal{E}} \leq h_1 |\xi^y(t,j)|_{\mathcal{E}^y} $ and $|\xi^y(t,j)|_{\mathcal{E}^y} \leq h_1 |\xi(t,j)|_{\mathcal{E}} $. Then the upper bound of $|\xi(t,j)|_{\mathcal{E}} $ is
 \begin{equation*}
     |\xi(t,j)|_{\mathcal{E}} \leq h_1^2 \left(\tfrac{a_d \overline{a}_U}{\lambda \underline{a}_U} \right)^{\nicefrac{1}{2}}  |\xi(0,0)|_{\mathcal{E}}  \exp \!\left(-\tfrac{\ln{(\nicefrac{1}{\lambda})}}{2 \tau_{\text{mati}}^s}t \right)
 \end{equation*}
Additionally, since $t \geq \tau_{\text{miati}} (j-1)$, we have
\begin{equation*}
    \begin{aligned}
        &\exp \!\left(-\tfrac{\ln{(\nicefrac{1}{\lambda})}}{2 \tau_{\text{mati}}^s}(t) \right) \\
        =&  \exp \!\left(-\tfrac{\ln{(\nicefrac{1}{\lambda})}}{2 \tau_{\text{mati}}^s}(\tfrac{t}{2}+\tfrac{t}{2})) \right) \\
        \leq & \exp \!\left(-\tfrac{\ln{(\nicefrac{1}{\lambda})}}{2 \tau_{\text{mati}}^s}(\tfrac{t}{2}+\tfrac{\tau_{\text{miati}}^s}{2}(j-1))) \right) \\
        =& \exp \!\left( \tfrac{\ln{(\nicefrac{1}{\lambda})}\tau_{\text{miati}}^s}{4 \tau_{\text{mati}}^s}\right)   
            \exp \!\left(-\tfrac{\ln{(\nicefrac{1}{\lambda})}}{4 \tau_{\text{mati}}^s}(t+\tau_{\text{miati}}^sj) \right) \\
        \leq & \exp \!\left( \tfrac{\ln{(\nicefrac{1}{\lambda})}\tau_{\text{miati}}^s}{4 \tau_{\text{mati}}^s}\right)   
            \exp \!\left(-\tfrac{\ln{(\nicefrac{1}{\lambda})}}{4 \tau_{\text{mati}}^s}  \min\{1,\tau_{\text{miati}}^s \} (t+j) \right).
    \end{aligned}
\end{equation*}
As a result, we have 
\begin{equation*}
    |\xi(t,j)|_{\mathcal{E}} \leq c_1 |\xi(0,0)|_{\mathcal{E}}\exp \! \big(- c_2 (t+j)\big),
\end{equation*}
where $c_1 = h_1^2 \left(\tfrac{a_d \overline{a}_U}{\lambda \underline{a}_U} \right)^{\nicefrac{1}{2}} \exp \!\left( \tfrac{\ln{(\nicefrac{1}{\lambda})}\tau_{\text{miati}}^s}{4 \tau_{\text{mati}}^s}\right)$ and $c_2 = \tfrac{\ln{(\nicefrac{1}{\lambda})}}{4 \tau_{\text{mati}}^s}  \min\{1,\tau_{\text{miati}}^s \}$.



We have shown $\mathcal{H}_2$ is uniformly globally pre-exponentially stable w.r.t $\mathcal{E}$, and we can prove $\mathcal{H}_1$ is UGES along the same line as the proof of Theorem \ref{Theorem H_1} (i.e. completeness of solution). $\hfill\blacksquare$