\section{Relation of MGD and Lipschitz Constant}\label{app:lip}


Regarding the relationship between the MGD and the Lipschitz constant of the vector field, we can consider the standard example of a linear ODE: $\dot{x}(t) = a \cdot x(t)$, for which the Lipschitz constant is precisely $a$. For simplicity, assume the initial condition $x(0) = 1$. Hence, the solution is $x(t) = e^{at}$. Then, by (4) we have $c = \frac{1}{T}(e^{aT} - 1)$, and hence:

\[
\begin{aligned}
\frac{1}{T} \int_0^T \|\dot{x}(t) - c\|^2 \, dt
&= \left( \frac{a}{2T} - \frac{1}{T^2} \right)e^{2aT} + \frac{1}{2T^2} e^{aT} - \frac{a}{2T} - \frac{1}{T^2}
\\&= \mathcal{O}\left(\frac{a}{T} e^{2aT}\right)
\\ \implies \text{MGD} &= \mathcal{O}\left(\sqrt{\frac{a}{T}} e^{aT}\right)
\end{aligned}
\]

In particular, for this example, the MGD grows super-exponentially with the Lipschitz constant. This result can be extended to an upper bound for general systems:

\begin{enumerate}
    \item By the Mean Value Theorem, there exists $\xi \in (0, T)$ such that $c = \frac{x(T) - x(0)}{T} = \dot{x}(\xi) = f(x(\xi))$.
    \item Therefore, $\|\dot{x}(t) - c\|^2 = \|\dot{x}(t) - \dot{x}(\xi)\|^2 = \|f(x(t)) - f(x(\xi))\|^2 \leq L^2 \|x(t) - x(\xi)\|^2$.
    \item We can bound the latter quantity via Grönwall's Lemma:
    \[
    \begin{aligned}
    \|x(t) - x(\xi)\|
    &= \left\|\int_{\xi}^t \dot{x}(s) \, ds \right\|
    \\&= \left\|\int_{\xi}^t f(x(s)) \, ds \right\|
    \\&\leq \int_{\xi}^t \|f(x(s))\| \, ds \quad \text{assuming } t \geq \xi
    \\&\leq \int_{\xi}^t \|f(x(s)) - f(x(\xi))\| + \|f(x(\xi))\| \, ds
    \\&\leq \underbrace{(t - \xi) \cdot \|f(x(\xi))\|}_{=\alpha(t)} + \int_{\xi}^t \underbrace{L}_{=\beta(s)} \cdot \underbrace{\|x(s) - x(\xi)\|}_{=u(s)} \, ds
    \\&\leq (t - \xi) \cdot \|f(x(\xi))\| \cdot e^{L(t - \xi)} \quad \text{via Grönwall}
    \end{aligned}
    \]

    And if $\xi \geq t$, we analogously get $\|x(t) - x(\xi)\| \leq (\xi - t) \cdot \|f(x(\xi))\| \cdot e^{L(\xi - t)}$.

    In particular, note that by the same method:
    \[
    \begin{aligned}
    \|f(x(\xi))\| = \frac{1}{T} \|x(T) - x(0)\| \leq \|f(x(0))\| e^{LT}
    \end{aligned}
    \]
\end{enumerate}

\begin{enumerate}
    \setcounter{enumi}{4}
    \item We use this result to bound the integral:
    \[
    \begin{aligned}
    \frac{1}{T} \int_0^T \|\dot{x}(t) - c\|^2 \, dt
    &\leq \frac{L^2}{T} \int_0^T \|x(t) - x(\xi)\|^2 \, dt
    \\&= \frac{L^2}{T} \left( \int_0^\xi \|x(t) - x(\xi)\|^2 \, dt + \int_\xi^T \|x(t) - x(\xi)\|^2 \, dt \right)
    \\&\leq \frac{L^2}{T} \|f(x(\xi))\|^2 \cdot \left( \int_0^\xi (\xi - t)^2 \cdot e^{2L(\xi - t)} \, dt + \int_\xi^T (t - \xi)^2 \cdot e^{2L(t - \xi)} \, dt \right)
    \\&\leq \dots
    \\&\leq \|f(x(\xi))\|^2 \left( (2LT^2 - T + \frac{1}{2L}) e^{2LT} - \frac{1}{2L} \right)
    \\&\lesssim \|f(x(0))\|^2 e^{2LT} \mathcal{O}(LT^2 e^{2LT})
    \\&= \mathcal{O}\left(\|f(x(0))\|^2 LTe^{4LT}\right)
    \end{aligned}
    \]
\end{enumerate}

\begin{enumerate}
    \setcounter{enumi}{5}
    \item Plugging this back into the definition of the MGD, we get:
    \[
    \begin{aligned}
    \text{MGD} &= \sqrt{\frac{1}{T} \int_0^T \|\dot{x}(t) - c\|^2 \, dt} = \mathcal{O}(\sqrt{LT} e^{2LT})
    \end{aligned}
    \]
\end{enumerate}
