\subsection{Proof of \cref{lem:conservative-pi}}
Suppose there exist distributions $\pi$, $f_0$, $f_1$ such that
\begin{align*}
p(y \mid x, t=0) &:= f_0(y \mid x), \text{ and } \\
p(y \mid x, t=1) &:= f_t(y \mid x) = (1-\pi(x)) f_0(y \mid x) + \pi(x) f_1(y \mid x).
\end{align*}
Pick any $x$. Observe that if $\pi(x)=0$, then the corresponding $\pi^\star(x) = 0$ and the lemma conclusion trivially holds. Thus, we may assume $\pi(x) > 0$, in which case we have by rearrangement:
\[ f_1(y \mid x) = \frac{1}{\pi(x)} \left( f_t(y \mid x) - f_0(y \mid x) \right) + f_0(y \mid x). \]
As a probability density, $f_1(y \mid x) \geq 0$, which implies
\[  \pi(x) \geq 1 - \frac{f_t(y \mid x)}{f_0(y \mid x)}. \]
Since the above holds for all $y$, we therefore must have 
\[  \pi(x) \geq 1 - \min_y \frac{f_t(y \mid x)}{f_0(y \mid x)} = \pi^\star(x). \]


To prove the second part of the lemma, let $x$ be a point and $\hat{\pi}$ be a function satisfying $1 \geq \hat{\pi}(x) \geq \pi^\star(x) > 0$. Then define
\[ f_1^{\hat{\pi}}(y \mid x) = \frac{1}{\hat{\pi}(x)} \left( f_t(y \mid x) - f_0(y \mid x) \right) + f_0(y \mid x). \]
By definition of $\pi^\star$, we have $f_1^{\hat{\pi}}(y \mid x) \geq 0$. Moreover, integrating the right hand side over $y$ shows that $f_1^{\hat{\pi}}(y \mid x)$ integrates to 1. Thus, $f_1^{\hat{\pi}}(y \mid x)$ is a proper density. Rearrangement shows that
\[ f_t(y \mid x) = (1-\hat{\pi}(x)) f_0(y \mid x) + \hat{\pi}(x) f_1^{\hat{\pi}}(y \mid x). \]
