\subsection{Proof of \cref{thm:unident}}
Consider the following densities over $[0,\infty)$: 
\begin{align*}
    f_0(y) &= \frac{3}{2} e^{-y} - e^{-2y}\\
    f^{(1)}_1(y) &= e^{-y} \\
    f^{(2)}_1(y) &= 2 e^{-2y}.
\end{align*}
It can be readily verified that these are all valid probability densities. Moreover, we can see that $f_0$ is log-concave over its domain since
\[ \frac{d^2}{d y^2} \log f_0(y) = -\frac{2e^y}{3(\frac{2}{3} - e^y)^2} < 0 \, \, \text{ for all 
 } y \geq 0. \]
$f^{(1)}_1$ and $f^{(2)}_1$ are also clearly log-concave since their log-densities are linear.


Suppose that $f_0$ is the observed null distribution. Letting $\pi_1 = \frac{3}{4}$ and $\pi_2 = \frac{1}{4}$, consider the following two observed treatment distributions:
\begin{align*}
f^{(1)}_t(y) &= (1-\pi_1) f_0(y) + \pi_1 f^{(1)}_1(y) \\
f^{(2)}_t(y) &= (1-\pi_2) f_0(y) + \pi_2 f^{(2)}_1(y).
\end{align*}
Using these definitions, we have
\begin{align*}
f^{(1)}_t(y) &= (1-\pi_1) f_0(y) + \pi_1 f^{(1)}_1(y) \\
&= \frac{1}{4} \left( \frac{3}{2} e^{-y} - e^{-2y} \right) + \frac{3}{4} e^{-y} \\
&= \frac{9}{8} e^{-y} - \frac{1}{4} e^{-2y} \\
&= \frac{3}{4} \left( \frac{3}{2} e^{-y} - e^{-2y} \right) + \frac{1}{4} \cdot 2 e^{-y} \\
&= (1-\pi_2) f_0(y) + \pi_2 f^{(2)}_1(y) \\
&= f^{(2)}_t(y).
\end{align*}
Thus, we can conclude that the C2G model is unidentifiable even when both the null distribution and the alternative distribution are restricted to being log-concave.
