\subsection{Proof of \cref{prop:confounding-npc2g}}

We need to show that $p(Y \mid X, T=1)$ can be written as a mixture model as in \cref{eqn:treatment-mixture}. This can be done by making use of the condition $Y \indep T \mid X, H$:
\begin{align*}
p(Y = y \mid X=x, T=1) &= \sum_{h=0}^1 p(H=h \mid X=x, T=1) p(Y = y \mid X=x, T=1, H=h) \\
&= \sum_{h=0}^1 p(H=h \mid X=x, T=1) p(Y = y \mid X=x, H=h) \\
&= (1-\pi(x)) f_0(y \mid x) + \pi(x) f_1(y \mid x).
\end{align*}
Here, we have simply defined $\pi(x) = p(H=1 \mid X=x, T=1)$, $f_0(y \mid x) = p(Y = y \mid X=x, H=0)$, and $f_1(y \mid x) = p(Y = y \mid X=x, H=1)$. \qed