\begin{appendices}
\section{Proofs of \Cref{theorem:rsvd_like_bound} and \Cref{theorem:fast_convergence}}\label{section:appendix}
\begin{proof}[Proof of \Cref{theorem:rsvd_like_bound}]
    First note that by a standard Chebyshev interpolation bound \cite[Lecture 20]{stewart}
    \begin{equation*}
        \inf\limits_{p \in \mathbb{P}_{2r+1}}\|\exp(x)-p(x)\|_{L^{\infty}([\lambda_{\min},\lambda_{\max}])}  \leq \frac{\gamma_{1,n}^{2r+r}}{2^{4r+3}(2r+2)!}\|\exp(\bm{A})\|_2.
    \end{equation*}
    % \begin{align*}
    %     &\inf\limits_{p \in \mathbb{P}_{2r+1}}\|\exp(x)-p(x)\|_{L^{\infty}([\lambda_{\min},\lambda_{\max}])} = \exp(\lambda_{\min}) \inf\limits_{p \in \mathbb{P}_{2r+1}}\|\exp(x)-p(x)\|_{L^{\infty}([0,\lambda_{\max}-\lambda_{\min}])} \leq \\
    %     &\exp(\lambda_{\min}) \frac{(\lambda_{\max} - \lambda_{\min})^{2r+2}}{(2r+2)!} \exp(\lambda_{\max} - \lambda_{\min}) = \frac{(\lambda_{\max} - \lambda_{\min})^{2r+2}}{(2r+2)!} \exp(\lambda_{\max})  = \\
    %     &\exp(\lambda_{\max} - \lambda_{\min}) = \frac{(\lambda_{\max} - \lambda_{\min})^{2r+2}}{(2r+2)!} \|\exp(\bm{A})\|_2.
    % \end{align*}
    Hence,
    \begin{equation*}
        4\sqrt{\ell s}  \inf\limits_{p \in \mathbb{P}_{2r+1}}\|f(x)-p(x)\|_{L^{\infty}([\lambda_{\min},\lambda_{\max}])} \leq 4\sqrt{\ell s} \frac{\gamma_{1,n}^{2r+2}}{(2r+2)!} \|\exp(\bm{A})\|_2.
    \end{equation*}
    We proceed with bounding $\mathcal{E}(s;\exp(x))$. Let $p(x) = \sum\limits_{i=1}^{s-1}\frac{(x-\lambda_{\min})^i}{i!}$. Then for $x \in [\lambda_{\min},\lambda_{\max}]$ we have $0 \leq p(x) \leq \exp(x-\lambda_{\min})$. Consequently, $\|p(\bm{\Lambda}_{n \setminus k })\|_{\F} \leq \|\exp(\bm{\Lambda}_{n \setminus k })\|_{\F} \exp(-\lambda_{\min})$. Furthermore, for $x \in [\lambda_{\min},\lambda_{\max}]$ we have
    % \begin{align*}
    %    0 &\leq  \exp(x-\lambda_{\min}) - p(x) 
    %    \\&= \sum\limits_{i=s}^{\infty} \frac{(x-\lambda_{\min})^i}{i!} = \frac{(x-\lambda_{\min})^s}{s!} \sum\limits_{i=0}^{\infty} \frac{(x-\lambda_{\min})^i}{(i+s)!} s! 
    %    \\&\leq \frac{(x-\lambda_{\min})^s}{s!} \sum\limits_{i=0}^{\infty} \frac{(x-\lambda_{\min})^i}{i!} = \frac{(x-\lambda_{\min})^s}{s!} \exp(x-\lambda_{\min}).
    % \end{align*}
    \begin{align*}
       0 \leq  \exp(x-\lambda_{\min}) - p(x) 
       \leq \frac{(x-\lambda_{\min})^s}{s!} \exp(x-\lambda_{\min}).
    \end{align*}
    Note that by the assumption on $s$ and a Stirling approximation $s! \geq \sqrt{2\pi s} \left(\frac{s}{e}\right)^s$ \cite{stirling} we have $\frac{\gamma_{1,n}^s}{s!} < 1$.
    Hence,
    \begin{align}\label{eq:bound}
        \max\limits_{i=1,\ldots,k} \left|\frac{\exp(\lambda_i)}{p(\lambda_i)}\right| &= \exp(\lambda_{\min})\max\limits_{i=1,\ldots,k} \left|\frac{\exp(\lambda_i - \lambda_{\min})}{p(\lambda_i)}\right| 
        \nonumber\\&
        = \exp(\lambda_{\min}) \left(1- \frac{(\lambda_{\max}-\lambda_{\min})^s}{s!}\right)^{-1}. 
    \end{align}
    Therefore, $\mathcal{E}(s;\exp(x))$ is bounded above by 
    \begin{equation}\label{eq:bound2}
        \mathcal{E}(s;\exp(x)) \leq \frac{1}{(1- \frac{(\lambda_{\max}-\lambda_{\min})^s}{s!})^2} \|\exp(\bm{\Lambda}_{n \setminus k})\|_{\F}^2 = \frac{1}{(1- \frac{\gamma_{1,n}^s}{s!})^2} \|\exp(\bm{\Lambda}_{n \setminus k})\|_{\F}^2.
    \end{equation}
    Plugging the inequalities  \eqref{eq:bound} and \eqref{eq:bound2} into \Cref{theorem:krylov_aware} yields the desired inequality. 
\end{proof}

\begin{proof}[Proof of \Cref{theorem:fast_convergence}]
    Bounding $4\sqrt{\ell s}\inf\limits_{p \in \mathbb{P}_{2r+1}}\|\exp(x)-p(x)\|_{L^{\infty}([\lambda_{\min},\lambda_{\max}])}$ is done identically to in \Cref{theorem:rsvd_like_bound}. We proceed with bounding $\mathcal{E}(s;\exp(x))$. Define $\delta(x) = \frac{x-\lambda_{k+1}}{\lambda_{k+1} - \lambda_n}$. Define the polynomial $p(x) = (1+x-\lambda_{n})T_{s-2}\left(1 + 2 \delta(x)\right)$, where $T_{s-2}$ is the Chebyshev polynomial of degree $s-2$. 
    Hence, recalling the definition \cref{eqn:min_ratio} of $\mathcal{E}(s;\exp(x))$, since $0\leq 1+x \leq \exp(x)$ for $x\geq 0$ and $|T_{s-2}(x)| \leq 1$ for $x \in [-1,1]$ we have,
    \[
    \|p(\bm{\Lambda}_{n \setminus k})\|_{\F}
    \leq \|\exp(\bm{\Lambda}_{n \setminus k} - \lambda_{n}\bm{I})\|_{\F}\]
    Hence, using that $\frac{\exp(x)}{1+x} \leq \exp(x)$ for $x \geq 0$ we get
    \begin{align}
        \mathcal{E}(s;\exp(x)) 
        &\leq \|p(\bm{\Lambda}_{n \setminus k})\|_{\F}^2 \max\limits_{i=1,\ldots,k} \left|\frac{\exp(\lambda_i)}{p(\lambda_i)}\right|^2 
        \nonumber\\&\leq 
        \|\exp(\bm{\Lambda}_{n \setminus k}-\lambda_{n}\bm{I})\|_{\F}^2\max\limits_{i=1,\ldots,k} e^{2\lambda_{n}} \left|\frac{\exp(\lambda_i-\lambda_{n})}{p(\lambda_i)}\right|^2 
        \nonumber\\&=\|\exp(\bm{\Lambda}_{n \setminus k})\|_{\F}^2\max\limits_{i=1,\ldots,k} \left|\frac{\exp(\lambda_i-\lambda_{n})}{p(\lambda_i)}\right|^2
        \nonumber\\&\leq\|\exp(\bm{\Lambda}_{n \setminus k})\|_{\F}^2\max\limits_{i=1,\ldots,k} \left|\frac{\exp(\lambda_i-\lambda_{n})}{T_{s-2}\left(1 + 2 \delta(\lambda_i)\right)}\right|^2.
        \label{eqn:Esexp_bd}
    \end{align}
    First note that for $|x| \geq 1$ we have
    \begin{equation*}
        T_{s-2}(x) = \frac{1}{2}\left(\left(x + \sqrt{x^2-1}\right)^{s-2} + \left(x - \sqrt{x^2-1}\right)^{s-2} \right).
    \end{equation*}
    Hence, for $\delta \geq 0$ we have $|T_{s-2}(1+2\delta)| \geq \frac{1}{2}(1+2\delta + 2\sqrt{\delta + \delta^2})^{s-2} =: \frac{1}{2}h(\delta)^{s-2}$. Therefore,
    \begin{align*}
        \max\limits_{i=1,\ldots,k} \left|\frac{e^{\lambda_i-\lambda_{n}}}{T_{s-2}\left(1 + 2 \delta(\lambda_i)\right)}\right|^2 &\leq 4 \max\limits_{i=1,\ldots,k} \left|\frac{\exp(\lambda_i-\lambda_{n})}{h(\delta(\lambda_i))^{s-2}}\right|^2\\
        &= 4 \max\limits_{i=1,\ldots,k} \left(\exp(\lambda_i - \lambda_n - (s-2)\log(h(\delta(\lambda_i))))\right)^2.
    \end{align*}
    Note that the function 
    \begin{equation*}
        g(x) := x - \lambda_n - (s-2)\log(h(\delta(x)))
    \end{equation*}
    is convex in $[\lambda_k,\lambda_1]$ because $\log(h(x))$ is concave for $x \geq 0$ and $\delta(x)$ is linear positive function for any $x \geq \lambda_{k}$. Hence, the maximum of $g$ on the interval $[\lambda_k,\lambda_1]$ is attained at either $x = \lambda_k$ or $x = \lambda_1$. The maximum of $g$ is attained at $x = \lambda_k$ whenever $g(\lambda_1) \leq g(\lambda_k)$ which happens whenever
    \begin{equation}\label{eq:scondition}
        \frac{\lambda_1 - \lambda_k}{\log\left(\frac{h(\delta(\lambda_1))}{h(\delta(\lambda_k))}\right)} + 2 \leq s.
    \end{equation}
    Note that we have whenever $x \geq y \geq 0$ we have $\frac{h(x)}{h(y)} \geq \frac{1 + x}{1+y}$, which can be seen by noting that $\frac{h(x)}{1+x}$ is an increasing function. Hence, \eqref{eq:scondition} holds whenever
    \begin{equation*}
        \frac{\lambda_1 - \lambda_k}{\log\left(\frac{\lambda_1 - \lambda_{n}}{\lambda_k - \lambda_{n}}\right)} + 2  \leq s,
    \end{equation*}
    which is our assumption on $s$. Hence, 
    \begin{equation}\label{eq:upperbound}
         \max\limits_{i=1,\ldots,k} \left|\frac{\exp(\lambda_i-\lambda_{n})}{T_{s-2}\left(1 + 2 \delta(\lambda_i)\right)}\right|^2 \leq 4 \frac{\exp(2(\lambda_k - \lambda_n))}{h(\delta(\lambda_k))^{2(s-2)}}.
    \end{equation}
    Now we use the argument from \cite[p.21]{MM15}, which shows that $h(\delta)^{(s-2)} \geq 2^{\sqrt{\min\{1,2\delta\}}(s-2) - 1}$. Plugging this inequality into \cref{eq:upperbound} and then \cref{eqn:Esexp_bd} and  using the definition for $\gamma_{i,j}$ yields
    \begin{equation*}
        \mathcal{E}(s;\exp(x)) \leq 16 \exp(2\gamma_{k,n}) 2^{-2(s-2) \sqrt{\min\left\{1,2 \frac{\gamma_{k,k+1}}{\gamma_{k+1,n}}\right\}}} \|\exp(\bm{\Lambda}_{n\setminus k})\|_\F^2.
    \end{equation*}
    % Bounding $4\sqrt{\ell s}\inf\limits_{p \in \mathbb{P}_{2r+1}}\|\exp(x)-p(x)\|_{L^{\infty}([\lambda_{\min},\lambda_{\max}])}$ is done identical to as done in \Cref{theorem:rsvd_like_bound}. We proceed with bounding $\mathcal{E}(s;\exp(x))$ by choosing the polynomial $p(x) = (1+x-\lambda_{\min})T_{s-2}\left(\frac{x-\lambda_{\min}}{\lambda_{k+1}-\lambda_{\min}}\right)$, where $T_{s-2}$ is the Chebyshev polynomial of degree $s-2$. 
    % Hence, recalling the definition \cref{eqn:min_ratio} of $\mathcal{E}(s;\exp(x))$, since $0\leq 1+x \leq e^x$ for $x\geq 0$,
    % \[
    % \|p(\bm{\Lambda}_{n \setminus k})\|_{\F}
    % \leq \|\exp(\bm{\Lambda}_{n \setminus k} - \lambda_{\min}\bm{I})\|_{\F} \left\|T_{s-2}\left(\frac{\bm{\Lambda}_{n \setminus k}-\lambda_{\min}\bm{I}}{\lambda_{k+1}-\lambda_{\min}}\right)\right\|^2.
    % \]
    % Hence, using that $|T_{s-2}(x)\leq 1$ for $x\in[0,1]$,
    % \begin{align}
    %     \mathcal{E}(s;\exp(x)) 
    %     &\leq \|p(\bm{\Lambda}_{n \setminus k})\|_{\F}^2 \max\limits_{i=1,\ldots,k} \left|\frac{e^{\lambda_i}}{p(\lambda_i)}\right|^2 
    %     \nonumber\\&\leq 
    %     \|\exp(\bm{\Lambda}_{n \setminus k}-\lambda_{\min}\bm{I})\|_{\F}^2\max\limits_{i=1,\ldots,k} e^{2\lambda_{\min}} \left|\frac{e^{\lambda_i-\lambda_{\min}}}{p(\lambda_i)}\right|^2 
    %     \nonumber\\&=\|\exp(\bm{\Lambda}_{n \setminus k})\|_{\F}^2\max\limits_{i=1,\ldots,k} \left|\frac{e^{\lambda_i-\lambda_{\min}}}{p(\lambda_i)}\right|^2.
    %     \label{eqn:Esexp_bd}
    % \end{align}
    % Finally, using that $\frac{e^x}{1+x} \leq e^x$ for $x \geq 0$,that $T_{s-2}(x)$ is increasing for $x \geq 1$, and \cite[Lemma 9.3]{tropp2023randomized} we have
    % \begin{align*}
    %     \max\limits_{i=1,\ldots,k} \left|\frac{e^{\lambda_i-\lambda_{\min}}}{p(\lambda_i)}\right|^2 
    %     &\leq 
    %     \max\limits_{i=1,\ldots,k} \left|\frac{e^{\lambda_i-\lambda_{\min}}}{T_{s-2}\big(\frac{x-\lambda_{\min}}{\lambda_{k+1}-\lambda_{\min}}\big)}\right|^2 
    %     \\&\hspace{5em}\leq \frac{e^{2\gamma}}{T_{s-2}\big(\frac{\lambda_k-\lambda_{\min}}{\lambda_{k+1}-\lambda_{\min}}\big)^2} 
    %     \leq 
    %     4 e^{2\gamma-4(s-2)\sqrt{\gamma}},
    % \end{align*}
    % Plugging this inequality into \cref{eqn:Esexp_bd} and then \cref{eqn:Esexp_bd} into \cref{theorem:krylov_aware} yields the desired inequality. 
\end{proof}
\end{appendices}