

\section{Proofs from Section~\ref{sec:gaussians-optimal}}\label{sec:ProofsGauss}




 For the analysis of the algorithm, we let $\widehat{\pte} = \cN(\widehat{\mte},\widehat{\ste}),\widehat{\ptr} = \cN(\widehat{\mtr},\widehat{\str})$ to denote approximations to the $\pte,\ptr$ respectively.  We now begin with the first part of the analysis.

\subsection*{Bound on Bias of the Estimator: Proof of Lemmas~\ref{lem:isotropic-gaussians-result} and~\ref{lem:Q_gauss_non_iso}}
\begin{lemma}
\label{cor:approx-Q}
For any $\ptr,\pte$ with corresponding approximations $\widehat{\ptr}, \widehat{\pte}$, and bounded $\ff(\xx)$ such that $\sup_{\xx}|\ff(\xx)|\leq 1$ we have
\begin{equation*}
    \left|\E_{\xx\sim \ptr} \frac{\widehat{\pte}(\xx)}{\widehat{\ptr}(\xx)} \ff(\xx) - \E_{\xx \sim \pte} \ff(\xx)\right|  \leq \Qdiv{1}{\widehat{\ptr}}{\ptr}{\widehat{\pte}} + d_{TV}(\widehat{\pte}, \pte).
\end{equation*}
\end{lemma}
\begin{proof}
First by triangle inequality we can decompose

\begin{align}\label{eq:BasicBoundGauss}
    \left|\E_{\xx\sim \ptr} \frac{\widehat{\pte}(\xx)}{\widehat{\ptr}(\xx)} \ff(\xx) - \E_{\xx \sim \pte} \ff(\xx)\right| 
    \leq &  \left|\E_{\xx\sim \ptr} \frac{\widehat{\pte}(\xx)}{\widehat{\ptr}(\xx)} \ff(\xx) - \E_{\xx \sim \widehat{\pte}} \ff(\xx)\right| \notag \\
    & + |\E_{\xx \sim \widehat{\pte}} \ff(\xx) - \E_{\xx \sim {\pte}} \ff(\xx)|
\end{align}
We now consider the two terms separately. Using the fact that $|\ff(\xx)|\leq 1$, the second term gives,
\begin{align*}
|\E_{\xx \sim \widehat{\pte}} \ff(\xx) - \E_{\xx \sim {\pte}} \ff(\xx)| &= \left|\int_{\xx} \ff(\xx) (\widehat{\pte}(\xx) -\pte(\xx)) d\xx \right|\\
& \leq \sup_{\xx}|\ff(\xx)| \int_{\xx} |\widehat{\pte} -\pte| d\xx\\
& \leq d_{TV}(\widehat{\pte},\pte).
\end{align*}

We now consider the first term.

\begin{align*}
           \left|\E_{\xx\sim \ptr} \frac{\widehat{\pte}(\xx)}{\widehat{\ptr}(\xx)} \ff(\xx) - \E_{\xx \sim \widehat{\pte}} \ff(\xx)\right| & = \left|\E_{\xx\sim \ptr} \frac{\widehat{\pte}(\xx)\ptr(\xx)}{\ptr(\xx)\widehat{\ptr}(\xx)} \ff(\xx) - \E_{\xx \sim \widehat{\pte}} \ff(\xx)\right| \\
            &  = \left|\E_{\xx\sim \widehat{\pte}} \frac{\ptr(\xx)}{\widehat{\ptr}(\xx)} \ff(\xx) - \E_{\xx \sim \widehat{\pte}} \ff(\xx)\right| \\
            &  \leq \E_{\xx\sim \widehat{\pte}} \left|\frac{\ptr(\xx)}{\widehat{\ptr}(\xx)} - 1 \right|.
    \end{align*}
    Using these bounds in Eq.~\eqref{eq:BasicBoundGauss} gives the result.

\end{proof}

From the above lemma, we see that we need to first give a bound on $\Qdiv{1}{\widehat{\ptr}}{\ptr}{\widehat{\pte}}$. Since from Definition~\ref{def:Q}, we know that $\Qdiv{1}{\cdot}{\cdot}{\cdot}\leq \Qdiv{2}{\cdot}{\cdot}{\cdot}$, in the remaining part we will show how to bound $\Qdiv{2}{\widehat{\ptr}}{\ptr}{\widehat{\pte}}$.




\begin{lemma}
    \label{lem:q_log_subexp}Let  $p,\widehat{p},$ and $q$ denote probability distributions and
    let $Z$ be a random variable defined as $Z = \ln (p(\xx)/\widehat{p}(\xx))$ for $\xx\sim q$. If $\mu := \E Z$ and $Z$ is $(\sigma, 1/2)$-subexponential for $\sigma \leq O(1)$, then $\Qdiv{2}{\widehat{p}}{p}{q} \leq O(\mu + \sigma)$.
\end{lemma}
\begin{proof}
    We have
    \begin{align*}
        \Qdiv{2}{\widehat{p}}{p}{q}^2 & = \E_{\xx\sim q} \left( \frac{p(\xx)}{\widehat{p}(\xx)} - 1\right)^2 \\
        & = \E_{\xx\sim q} (\exp(Z) - 1)^2 = \E_{\xx\sim q} [\exp(2Z) - 2\exp(Z) +1 ].
    \end{align*}
    Since $Z$ is subexponential, we have $\E_{\xx\sim q}\exp(Z-\mu) \leq \exp( \sigma)$, and therefore, $\E_{\xx\sim q} \exp(2Z) \leq \exp(2 \mu + 2\sigma)$. Now, we will use that for any $y\geq 0$, $e^y \leq 1+y+O(1)y^2$ for $y\leq O(1)$ and $e^y \geq 1+y$ which yields
    \begin{align*}
        \E_{\xx\in q}[\exp(2Z) - 2\exp(Z) + 1] & = 1 + 2 \mu + O(1)\cdot(\mu+\sigma)^2 - 2(1 + \mu) - 2 \\
        & = O(1)\cdot (\mu + \sigma)^2.
    \end{align*}
\end{proof}

We begin with the easy case and first give a bound on the bias of our estimator in the case when $\ptr$ and $\pte$ are isotropic Gaussian distributions.

\IsoGaussBias*

\begin{proof}
    We will use \cref{lem:q_log_subexp} to show $\Qdiv{2}{\widehat{\ptr}}{\ptr}{\widehat{\pte}} \leq O(\varepsilon)$ in this case. The remaining follows from \cref{cor:approx-Q}.

    Let $p = \ptr$, $\widehat{p} = \widehat{\ptr}$, and $q = \widehat{\pte}$. We need to show that $Z$, as defined in \cref{lem:q_log_subexp} is $(\varepsilon,1/2)$ subexponential and $\E_{\xx\sim q}Z \leq O(\varepsilon)$.
    
    
    Now, $Z = \ln \ptr - \ln \widehat{\ptr} = \langle \mtr - \widehat{\mtr}, \xx\rangle + \frac{1}{2}\langle \widehat{\mtr} - \mtr, \mtr + \widehat{\mtr}\rangle$ is a Gaussian with mean $ \langle \widehat{\mtr} - \mtr,\widehat{\mte}\rangle + \frac{1}{2}\langle \widehat{\mtr} - \mtr, \mtr + \widehat{\mtr}\rangle$ and variance $\|\mtr - \widehat{\mtr}\|^2_2$. From Lemma~\ref{lem:MeanGauss}, we know that that $\|\mtr - \widehat{\mtr}\|^2_2\leq \varepsilon^2$, and therefore, $\Var(Z)\leq \varepsilon^2$. Further, the mean satisfies,  
 \[
    \E Z =  \langle \widehat{\mtr} - \mtr,2\widehat{\mte} + \mtr + \widehat{\mtr}\rangle 
    \leq\| \widehat{\mtr} - \mtr\|_2 \|2\widehat{\mte} + \mtr + \widehat{\mtr}\|_2.
\]
In the above, since  $\|\mtr-\mte\|_2\leq O(1)$, and $\|\mtr\|_2\leq O(1)$, we must have $\|\widehat{\mte}\|_2\leq O(1)$. Therefore,
 \[
    \E Z 
    \leq\| \widehat{\mtr} - \mtr\|_2 \left(2\|\widehat{\mte}\|_2 + \|\mtr\|_2 + \|\widehat{\mtr}\|_2\right) \leq O(\varepsilon).
\]

We now claim that $Z$ is $(\varepsilon,1/2)$ subexponential with mean bounded by $O(\varepsilon)$. This follows since $Z$ is gaussian with std deviation $\varepsilon$, the MGF of $Z$ is bouneded by $e^{\varepsilon^2 \lambda^2}$ for all $\lambda>0$, which implies $Z$ is $(\varepsilon,1/2)$ subexponential. This concludes the proof for isotropic Gaussian distributions.
\end{proof}

\GaussBias*

\begin{proof}
    We will deduce this as a corollary from \Cref{lem:q_log_subexp}. To this end, let $Z := \ln \ptr(\xx) - \ln \widehat{\ptr}(\xx)$ for $\xx\sim \widehat{\pte}$. Note that $Z = \xx^{\top} \AA \xx + \bb^T x + c$, where 
    \begin{align*}
        \AA & = (\str^{-1} - \widehat{\str}^{-1})/2 \\
        \bb & =\str^{-1} \mtr - \widehat{\str}^{-1} \widehat{\mtr} \\
        c & = (\mtr^{\top} \str^{-1} \mtr - \widehat{\mtr}^{\top} \widehat{\str}^{-1} \widehat{\mtr})/2.
    \end{align*}
 Now, from Fact~\ref{fact:quad-gauss}, $\xx^{\top} \AA \xx$ is $(\|\AA\|_F, \|\AA\|_{op})$-subexponential, and we know that $\|\AA\|_{op} \leq \|\AA\|_F\leq \sqrt{d}\|\AA\|_{op}$. 
  \[
    \|\widehat{\str}^{-1}-\str^{-1}\|_{op} \leq \|\str^{-1/2}\|_{op}\|\str^{1/2}\widehat{\str}^{-1}\str^{1/2}-\II\|_{op}\|\str^{-1/2}\|_{op}.
    \]
    From Lemma~\ref{lem:CovGauss}, we know that $\|\str^{-1/2}\widehat{\str}\str^{-1/2}-\II\|_{op} \leq \frac{\varepsilon}{2\sqrt{d}}$. This implies that all eigenvalues of $\str^{-1/2}\widehat{\str}\str^{-1/2}$ are between $1-\varepsilon/2\sqrt{d}$ and $1+\varepsilon/2\sqrt{d}$ and as a result, $\|\str^{1/2}\widehat{\str}^{-1}\str^{1/2}-\II\|_{op} \leq \varepsilon/\sqrt{d}$. Now, from assumption, $\|\str^{-1}\|_{op} \leq O(1)$, and we get that,
    \[
    \|\widehat{\str}^{-1}-\str^{-1}\|_{F}\leq \sqrt{d} \cdot \|\widehat{\str}^{-1}-\str^{-1}\|_{op}\leq O\left(\varepsilon\right).
    \]

 Therefore, $Z$ is $(O(\varepsilon), O(\varepsilon))$-subexponential. The random variable $\bb^{\top} \xx$ is $\|\bb\|_2$-subgaussian, and we can bound,
    \begin{equation*}
        \|\bb\|_2 = \|\str^{-1} \mtr - \widehat{\str}^{-1} \widehat{\mtr}\|_2 \leq \|\str^{-1}(\mtr-\widehat{\mtr})\|_2  +  \|(\widehat{\str}^{-1}-\str^{-1})\widehat{\mtr}\|_2  \leq O(\varepsilon).
    \end{equation*}
For the first term we use Lemma~\ref{lem:MeanGauss} and for the second term we use the previous calculation along with the assumption that $\|\mtr\|_2\leq O(1).$
    The sum of $\varepsilon$-subgaussian and $(\varepsilon, \varepsilon)$-subexponential random variable is $(O(\varepsilon), O(\varepsilon))$-subexponential again.

    Finally $\E Z = \Tr \AA + \bb^{\top}\mte + c$, and since $\|\mtr-\mte\|_2\leq O(1)$, and $\|\mtr\|_2\leq O(1)$ imply that $\|\mte\|_2\leq O(1)$, $\Tr \AA \leq \|\AA\|_F$, all we need to do is bound $c$.
    \begin{align*}
        (\mtr^{\top} \str^{-1} \mtr - \widehat{\mtr}^{\top} \widehat{\str}^{-1} \widehat{\mtr}) & \leq
        \|\mtr^{\top} (\str^{-1} - \widehat{\str}^{-1}) \mtr\|_2 + \langle \str^{-1}(\mtr - \widehat{\mtr}), (\mtr+ \widehat{\mtr}) \rangle \leq O(\varepsilon) .
    \end{align*}
    The final statement of the lemma now follows from Lemma~\ref{cor:approx-Q}.
\end{proof}

\subsection*{Bound on Variance of the Estimator: Proof of Lemma~\ref{lem:Var}}
In this section, we give a bound on the variance of our estimator $ \frac{\widehat{\pte}(\xx)}{\widehat{\ptr}(\xx)}\ff(\xx)$ for $\xx \sim \ptr$.

\begin{lemma}\label{lem:BoundSquaredVariance}
Let $X$ denote the estimator $\frac{\widehat{\pte}(\xx)}{\widehat{\ptr}(\xx)}\ff(\xx)$for $\xx \sim \ptr$. If $\|\str^{-1}\|_{op}\leq O(1)$, $\|\str^{-1}-\ste^{-1}\|_F\leq O(1)$, and $\|\mtr\|_2, \|\mtr-\mte\|_2\leq O(1)$, then
\begin{equation*}
    \E_{\xx \sim \ptr}[X^2] \leq 2 + 2\Qdiv{2}{\widehat{\ptr}}{\widehat{\pte}}{\ptr} \leq O(1).
\end{equation*}
\end{lemma}
\begin{proof}
\begin{align*}
    \E_{\xx \sim \ptr}[X^2]& = \E_{\xx \sim \ptr}\left[\left(\frac{\widehat{\pte}(\xx)}{\widehat{\ptr}(\xx)}\ff(\xx) - \ff(\xx) + \ff(\xx)\right)^2\right]\\
    & \leq 2\E_{\xx \sim \ptr}\left[\left(\frac{\widehat{\pte}(\xx)}{\widehat{\ptr}(\xx)}-1\right)^2\ff(\xx)^2\right]  + 2\E_{\xx\sim \ptr}[\ff(\xx)^2]\\
    & \leq 2\cdot \Qdiv{2}{\widehat{\ptr}}{\widehat{\pte}}{\ptr} + 2.
\end{align*}
In the last line we used $|\ff(\xx)|\leq 1.$

Now, we consider the distribution of $Z := \ln \widehat{\pte}(\xx) - \ln \widehat{\ptr}(\xx)$ for $\xx\sim \ptr$. Note that $Z = \xx^{\top} \AA \xx + \bb^T x + c$, where 
    \begin{align*}
        \AA & = (\widehat{\ste}^{-1}-\widehat{\str}^{-1})/2 \\
        \bb & =\widehat{\ste}^{-1} \widehat{\mte} - \widehat{\str}^{-1} \widehat{\mtr} \\
        c & = (\widehat{\mte}^{\top} \widehat{\ste}^{-1} \widehat{\mtr} - \widehat{\mtr}^{\top} \widehat{\str}^{-1} \widehat{\mtr})/2.
    \end{align*}
    
    Now, from Fact~\ref{fact:quad-gauss}, $\xx^{\top} \AA \xx$ is $(\|\AA\|_F, \|\AA\|_{op})$-subexponential, and since $\|\AA\|_{op} \leq \|\AA\|_F\leq \sqrt{d}\|\AA\|_{op}$ we will give a bound on $\|\AA\|_{F}$.

    From triangle inequality,
    \[
    \|\AA\|_{F}\leq \|\widehat{\ste}^{-1}-\ste^{-1}\|_{F}+ \|\ste^{-1}-\str^{-1}\|_{F} + \|\widehat{\str}^{-1}-\str^{-1}\|_{F}.
    \]
    Now,
    \[
    \|\widehat{\ste}^{-1}-\ste^{-1}\|_{op} \leq \|\ste^{-1/2}\|_{op}\|\ste^{1/2}\widehat{\ste}^{-1}\ste^{1/2}-\II\|_{op}\|\ste^{-1/2}\|_{op}.
    \]
    From Lemma~\ref{lem:CovGauss}, we know that $\|\ste^{-1/2}\widehat{\ste}\ste^{-1/2}-\II\|_{op} \leq \frac{\varepsilon}{2\sqrt{d}}$. This implies that all eigenvalues of $\ste^{-1/2}\widehat{\ste}\ste^{-1/2}$ are between $1-\varepsilon/2\sqrt{d}$ and $1+\varepsilon/2\sqrt{d}$ and as a result, $\|\ste^{1/2}\widehat{\ste}^{-1}\ste^{1/2}-\II\|_{op} \leq \varepsilon/\sqrt{d}$. Now, from assumption, $\|\ste^{-1}\|_{op} \leq O(1)$, and we get that,
    \[
    \|\widehat{\ste}^{-1}-\ste^{-1}\|_{F}\leq \sqrt{d} \cdot \|\widehat{\ste}^{-1}-\ste^{-1}\|_{op}\leq O\left(\varepsilon\right).
    \]
    Similarly, we can show that 
    \[
    \|\widehat{\str}^{-1}-\str^{-1}\|_{F}\leq O(\varepsilon).
    \]
    From assumption, we know that $\|\ste^{-1}-\str^{-1}\|_{F} \leq O(1)$, and as a result we get that $\|\AA\|_{op}\leq \|\AA\|_F \leq O(1).$

    
    Therefore, $Z$ is $(O(1), O(1))$-subexponential. The random variable $\bb^{\top} \xx$ is $\|\bb\|_2$-subgaussian, and we can bound,
    \begin{align*}
        \|\bb\|_2 & = \|\widehat{\ste}^{-1} \widehat{\mte} - \widehat{\str}^{-1} \widehat{\mtr}\|_2 \\
        &\leq \|\widehat{\ste}^{-1} \widehat{\mte} - \widehat{\ste}^{-1} \widehat{\mtr}\|_2+\|\widehat{\ste}^{-1} \widehat{\mtr} - \widehat{\str}^{-1} \widehat{\mtr}\|_2\\
        & \leq\|\widehat{\ste}^{-1}\|_{op}\|\widehat{\mtr} - \widehat{\mte}\|_2  + \|\widehat{\mtr}\|_2 \|\widehat{\str}^{-1} - \widehat{\ste}^{-1}\|_{op}\leq O(1).
    \end{align*}

    The sum of $O(1)$-subgaussian and $(O(1), O(1))$-subexponential random variable is $(O(1), O(1))$-subexponential again.

    Finally $\E Z = \Tr \AA + c$, and since $\Tr \AA \leq \|\AA\|_F$, all we need to do is bound $c$.
    \begin{align*}
        (\widehat{\mte}^{\top} \widehat{\ste}^{-1} \widehat{\mte} - \widehat{\mtr}^{\top} \widehat{\str}^{-1} \widehat{\mtr}) & \leq
        \|\widehat{\mtr}^{\top} (\widehat{\ste}^{-1} - \widehat{\str}^{-1}) \widehat{\mtr}\|_2 \\
        &+ \langle \widehat{\ste}^{-1}(\widehat{\mte} - \widehat{\mtr}), (\widehat{\mte}+ \widehat{\mtr}) \rangle \leq O(1) .
    \end{align*}
    From Lemma~\ref{lem:q_log_subexp}, we can now bound $\Qdiv{2}{\widehat{\ptr}}{\widehat{\pte}}{\ptr} \leq O(1).$
\end{proof}

\VarianceGauss*

\begin{proof}
    The proof follows from the following equation: for any random variable $X$ and $\mu$,
    \[
    \E[(X-\mu)^2] = \E[X^2] -2\mu\E[X] + \mu^2 \leq \E[X^2] + 2\mu|\E[X]-\mu|.
    \]
    Now, letting $X = \frac{\widehat{\pte}(\xx)}{\widehat{\ptr}(\xx)}\ff(\xx)$ and $\mu = \E_{\xx\sim\pte}\ff(\xx)$, from \Cref{lem:BoundSquaredVariance}, $\E[X^2] \leq O(1)$ and from \Cref{lem:Q_gauss_non_iso} $|\E[X]-\mu|\leq \varepsilon$. Furthermore, since $|\ff(\xx)|\leq 1$, we can further bound $\E_{\xx\sim\pte}\ff(\xx)\leq 1.$ Therefore $\E[(X-\mu)^2]\leq O(1)$.
\end{proof}

