% \section{Proof of Claim~\ref{claim:approx-arbitrage}}\label{app:proof-arb-claim}
% Define $h_{\epsilon, p}(\delta) = \min_{g \in \partial f(\delta)} h(p, g, \delta, \epsilon)$ and $f(\delta) = F(p, w^{\star}, R, \delta)$.
% Note that since $|g|\leq B$, by assumption, we have
% \[
% h_{\epsilon, p}(\delta) = \delta^T ((gp^T) - \epsilon \ones_{n\times n})\delta \leq -\epsilon \Vert \delta\Vert_2
% \]
% This implies that $h_{\epsilon, p}$ is strongly concave~\cite[\S9.1]{boyd2004convex}.
% This implies the Polyak-Lojasiewicz condition
% \[
% \Vert \nabla h_{\epsilon}(\delta^{\star}) \Vert_2 \geq \epsilon \Vert \delta_{H, \epsilon} - \delta^{\star}\Vert_2
% \]
% On the other hand, we have 
% \[
% \Vert \nabla h_{\epsilon}(\delta^{\star})\Vert \leq \Vert \nabla h_{\epsilon}(\delta^{\star}) - \nabla f(\delta_H)\Vert + \Vert \nabla f(\delta_H)\Vert 
% \]
% Note that using the Lipschitz condition on $f$ and the definition of $h_{\epsilon, p}$, we have 
% \[
% \Vert \nabla h_{\epsilon}(\delta^{\star}) - \nabla f(\delta_H) \Vert \leq (L - B\Vert p\Vert_{\infty}-\epsilon)\Vert \delta^{\star}  - \delta_H\Vert_2 
% \]
% This implies the chain of inequalities
% \[
% \epsilon \Vert \delta_H - \delta^{\star}\Vert_2 \leq \Vert \nabla h_{\epsilon}(\delta^{\star})\Vert_2 \leq (L-B\Vert p\Vert_{\infty}-\epsilon) \Vert \delta^{\star}  - \delta_H\Vert_2  + B
% \]
% Rearranging, this implies that
% \[
% \Vert \delta_H - \delta^{\star}\Vert_2 \leq \frac{B}{2 \epsilon - L - B \Vert p\Vert_{\infty}}
% \]

% We will fix $p, w^{\star}, \pi$ and define $f(\delta) = F(p, w^{\star}, \pi, \delta) (p^T \delta)$
% Define $h(\delta) = \min_{g \in \partial f(\delta)} H(p, g, \delta)$.
% Since $h(\delta) = (p^T\delta)(1+(g-p)^T \delta)$, we have
% \begin{align*}
%     h(\delta) - h(\delta') - \nabla h(\delta)^T (\delta - \delta') &= p^T(\delta - \delta') - (p^T \delta)(g-p)^T (\delta-\delta') \\ 
%     &> \Vert p\Vert_{\infty}(\Vert g-p \Vert_{\infty}) \Vert\delta - \delta'\Vert_2^2
% \end{align*}
% which implies that $h$ is $\mu$-strongly convex with $\mu = \Vert p \Vert_{\infty}(\Vert g - p \Vert_{\infty})$.
% Moreover, since $g-p \leq 0$, $h(\delta) \leq p^T \delta$ and so $h(\delta)$ is $\Vert p \Vert_{\infty}$-Lipschitz.

% Now note that
% \begin{align*}
% \Vert \nabla f(\delta_H)\Vert_2 &= \Vert \nabla f(\delta_H) - \nabla h(\delta_H) \Vert_2 = \Vert \nabla f(\delta_H) + \nabla h(\delta^{\star}) - \nabla h(\delta^{\star})\Vert_2 \\
% &\geq \Vert \nabla h(\delta^{\star}) \Vert_2 - \Vert \nabla f(\delta_H) - \nabla h(\delta^{\star})\Vert_2 \\
% &\geq \mu \Vert \delta^{\star}-\delta_H\Vert_2 - (L + \Vert p \Vert_{\infty})\Vert \delta^{\star} - \delta^H\Vert_2
% \end{align*}
% where the first step uses the fact that $\nabla h (\delta_H) = 0$, the first inequality is the triangle inequality, and the second inequality uses the $\mu$-smoothness of $h$ and the fact that $f$ is $L$-Lipschitz and $h$ is $\Vert p \Vert_{\infty}$-Lipschitz.
% Rearranging and using the fact that $\nabla f$ is bounded gives
% \[
% \Vert \delta^{\star} - \delta^H \Vert_2 \leq \frac{\Vert \nabla f(\delta_H)\Vert_2}{\mu-(L+\Vert p \Vert_{\infty})} \leq \frac{B}{\mu-(L+\Vert p \Vert_{\infty})}  \leq \frac{B}{\Vert p \Vert_{\infty}(\Vert g -p \Vert_{\infty} -1) - L}
% \]
% as claimed.