In this decomposition we let 
\[
T = D_1 + D_2 + D_4\eqsp.
\]
Then we will do some coupling. In this case:
\[
\theta_k - \thetas = \Jnalpha{k}{0}+ \Hnalpha{k}{0} \eqsp,
\]
where the latter terms are defined by the following pair of recursions
\begin{align}
\label{eq:jn0_main}
&\Jnalpha{k}{0} =\left(\Id - \alpha_{k} \bA\right) \Jnalpha{k-1}{0} - \alpha_{k} \funcnoise{\State_{k}}\eqsp, && \Jnalpha{0}{0}=0\eqsp, \\[.1cm]
\label{eq:hn0_main}
&\Hnalpha{k}{0} =\left( \Id - \alpha_{k} \funcA{\State_{k}} \right) \Hnalpha{k-1}{0} - \alpha_{k} \zmfuncA{\State_{k}} \Jnalpha{k-1}{0}\eqsp, && \Hnalpha{0}{0}=0\eqsp.
\end{align}
Then we have:
\begin{align}
T&= \frac{1}{n}\frac{\Jnalpha{n}{0}}{\alpha_{n}} + \frac{1}{n}\frac{\Hnalpha{n}{0}}{\alpha_{n}} - \frac{1}{n}\frac{\Jnalpha{2n}{0}}{\alpha_{2n}} - \frac{1}{n}\frac{\Hnalpha{2n}{0}}{\alpha_{2n}} + \frac{1}{n}\sum_{k=n+1}^{2n}\Jnalpha{k-1}{0}\left(\frac{1}{\alpha_k} - \frac{1}{\alpha_{k-1}}\right) + \frac{1}{n}\sum_{k=n+1}^{2n}\Hnalpha{k-1}{0}\left(\frac{1}{\alpha_k} - \frac{1}{\alpha_{k-1}}\right)\eqsp.
\end{align}
Now we do:
\begin{align}
\frac{1}{n}\sum_{k=n+1}^{2n}\Jnalpha{k-1}{0}\left(\frac{1}{\alpha_k} - \frac{1}{\alpha_{k-1}}\right) 
&= \frac{1}{n}\frac{\Jnalpha{n}{0}}{\alpha_{n+1}} - \frac{1}{n}\frac{\Jnalpha{n}{0}}{\alpha_{n}} + \frac{1}{n}\frac{\Jnalpha{n+1}{0}}{\alpha_{n+2}} - \ldots \\
&= - \frac{1}{n}\frac{\Jnalpha{n}{0}}{\alpha_{n}} + \frac{1}{n}\sum_{k=n+1}^{2n-1}\frac{1}{\alpha_k}\left(\Jnalpha{k-1}{0} - \Jnalpha{k}{0}\right) + \frac{\Jnalpha{2n-1}{0}}{n \alpha_{2n}}
\end{align}
Thus, we have from \eqref{eq:jn0_main}:
\[
\Jnalpha{k-1}{0} - \Jnalpha{k}{0} = \alpha_{k} \bA \Jnalpha{k-1}{0} + \alpha_{k} \funnoisew_{k}\,.
\]

\begin{lemma}
\label{Pinsker}
Let $X \sim \mathcal{N}(0, \Sigma_1)$ and $Y \sim \mathcal{N}(0, \Sigma_2)$ belong to $\mathbb{R}^p$, and  
\[
\| \Sigma_2^{-1/2} \Sigma_1 \Sigma_2^{-1/2} - \Id_p \| \leq 1/2, \quad \text{and} \quad \trace \{ (\Sigma_2^{-1/2} \Sigma_1 \Sigma_2^{-1/2} - I_p)^2 \} \leq \delta^2,
\]
for some $\delta^2 \geq 0$. Then it holds  
\[
\kolmogorov(X, Y) \leq \delta/2.
\]
\end{lemma}
\begin{proof}
   Let $\PP_1 = \mathcal{N}(0, \Sigma_1)$ and $\PP_2 = \mathcal{N}(0, \Sigma_2)$. Denote  
\[
G = \Sigma_2^{-1/2} \Sigma_1 \Sigma_2^{-1/2},
\]
then the Kullback-Leibler divergence between $\PP_1$ and $\PP_2$ is equal to  
\[
\KLs(\mathbb{P}_1 | \mathbb{P}_2) = -0.5 \log \{\det(G)\} + 0.5 \trace \{ G - \Id_p \}
\]
\[
= 0.5 \sum_{j=1}^{p} \{\lambda_j - \log(\lambda_j) + 1\},
\]
where $\lambda_p \leq \dots \leq \lambda_1$ are the eigenvalues of the matrix $G - \Id_p$. By conditions of the lemma $|\lambda_1| \leq 1/2$, and it holds:  
\[
\KLs(\PP_1| \PP_2) \leq 0.5 \sum_{j=1}^{p} \lambda_j^2 = 0.5 \trace \{ (G - \Id_p)^2 \} \leq \delta^2 / 2
\]
which finishes the proof due to the Pinsker inequality, 
(see, e.g., \citep{Tsybakov}[pp. 88, 132]: for a measurable space $(\Omega, \mathcal{F})$ and two measures on it $\PP_1, \PP_2$:
\[
\sup_{A \in \mathcal{F}} \left| \PP_1(A) - \PP_2(A) \right| \leq \sqrt{\KLs(\PP_1 | \PP_2)/2}.
\]
\end{proof} 

%While ``co‐coercivity'' is often introduced in the operator‐theoretic literature (especially in the context of firmly nonexpansive mappings), it also appears in more classical forms in optimization textbooks whenever they discuss the Baillon–Haddad theorem or gradient‐based convergence, see e.g \cite{nesterov}.