Here are known representations for $Q_t - \bA^{-1}$, $\sum_{t=1}^n (Q_t - \bA^{-1})$ and $\Sigma_n -  \Sigma_{\infty}$ proved in \citep[pp. 26-30]{wu2024statisticalinferencetemporaldifference}:

\begin{equation}
    \label{repr:qtminusa}
    Q_t - \bA^{-1} = S_t - \bA^{-1} \prod_{k=t}^n (\Id - \alpha_k \bA),~ S_t = \sum_{j=t+1}^{n} (\alpha_t - \alpha_j) G_{t+1:j-1}^{(\alpha)}
\end{equation}

\begin{equation}
    \label{repr:sumqtminusa}
    \sum_{t=1}^n (Q_t - \bA^{-1}) = -\bA^{-1} \sum_{j=1}^n G_{1:j}^{(\alpha)}
\end{equation}

\begin{align}
    \label{repr:Lstar_minus_Ln}
    \Sigma_n - \Sigma_{\infty} = \underbrace{\frac{1}{n}\sum_{t=1}^n (Q_t - \bA^{-1})\noisecov \bA^{-\top} + \frac{1}{n} \sum_{t=1}^n \bA^{-1} \noisecov (Q_t - \bA^{-1})^\top}_{D_1} + \\ + \underbrace{\frac{1}{n} \sum_{t=1}^n (Q_t - \bA^{-1}) \noisecov (Q_t - \bA^{-1})^{\top}}_{D_2}
\end{align}
For future simplicity, we denote 
\begin{equation}
    \label{def:gnm}
    g_{n:m} = \sum_{k=n}^m k^{-\gamma},~ n \leq m
\end{equation}

We use the following proposition \cite[Proposition~1]{samsonov2024gaussian} for a Hurwitz matrix $-\bA$:

\begin{proposition}
\label{prop:hurwitz_stability}
Let $-\bA$ be a Hurwitz matrix. Then for any $P = P^{\top} \succ \Id$, there exists a unique matrix $Q = Q^{\top} \succ \Id$, satisfying the Lyapunov equation $\bA^\top Q + Q \bA = P$. Moreover, setting
\begin{equation}
\label{eq:alpha_infty_def}
\textstyle 
a = \frac{\lambda_{\min}(P)}{2\normop{Q}}\eqsp, \quad
\text{and} \quad \alpha_\infty = \frac{\lambda_{\min}(P)}{2\qcond \normop{\bA}[Q]^{2}}\wedge \frac{\normop{Q}}{\lambda_{\min}(P)} \eqsp,
\end{equation}
where $\qcond = \lambda_{\max}(Q)/\lambda_{\min}(Q)$, it holds for any $\alpha \in [0, \alpha_{\infty}]$ that $\alpha a \leq 1/2$, and
\begin{equation}
\label{eq:contractin_q_norm}
\normop{\Id - \alpha \bA}[Q]^2 \leq 1 - \alpha a\eqsp.    
\end{equation}
\end{proposition}
Hence, we arrive at a bound for the operator norm of a product $\prod_{k=1}^n (\Id - \alpha_k \bA)$:

\begin{proposition}
\label{cor:hurwitz_stability}
    Suppose the conditions of {\Cref{prop:hurwitz_stability}} hold for each $\alpha \in \{\alpha_1, \ldots, \alpha_n\}$. Therefore
    \begin{equation}
        \label{bound:id_minus_aA}
        \normopadapt{\prod_{k=1}^n (\Id - \alpha_k \bA)} \leq \sqrt{\qcond} \cdot \prod_{k=1}^n \left(1 -\frac{a}{2} \cdot \alpha_k\right) \leq \sqrt{\qcond} \cdot \exp{\left(-\frac{a}{2} \sum_{k=1}^n \alpha_k\right)}
    \end{equation}
\end{proposition}

\begin{proof}
    Applying \textbf{\Cref{prop:hurwitz_stability}} and combining inequalities $\sqrt{1 - x} \leq 1 - \frac{x}{2}$ and $1 - x \leq \exp(-x)$, we get
    \begin{align}
    \label{pf:qnorm:expbound}
    \normopadapt{\prod_{k=1}^n (\Id - \alpha_k \bA)}[Q] 
    &\leq \prod_{k=1}^n \sqrt{\normop{\Id - \alpha_k \bA)}[Q]^2} \leq \prod_{k=1}^n \sqrt{1 - a \alpha_k} \leq \prod_{k=1}^n \left(1 - \frac{a \alpha_k}{2}\right) \\ 
    &\leq \prod_{k=1}^n \exp\left(-\frac{a \alpha_k}{2}\right) = \exp\left(- \frac{a}{2}\sum_{k=1}^n \alpha_k\right)
    \end{align}
    To complete the proof it remains to note that
    
    \begin{align}
        \frac{\normop{B x}[Q]}{\normop{x}[Q]} = \frac{\normop{Q^{1/2} B x}}{\normop{Q^{1/2} x}} = \frac{\normop{Q^{-1/2}} \cdot \normop{Q^{1/2} B x}}{\normop{Q^{-1/2}} \cdot \normop{Q^{1/2} x}} \geq \frac{\normop{Q^{-1/2} Q^{1/2} B x}}{ \normop{Q^{-1/2}} \cdot \normop{Q^{1/2}} \cdot \normop{x}} \\ = \frac{1}{\Cond(Q^{1/2})} \cdot \frac{\normop{B x}}{\normop{x}}
    \end{align}
    
    Taking supremum over $x \ne 0$ and multiplying both parts by $\Cond(Q^{1/2})$ we get 
    \begin{equation}
        \label{pf:qnorm:energybound}
         \normop{B}[Q] \cdot \sqrt{\qcond} = \normop{B}[Q] \cdot \Cond(Q^{1/2}) \geq \normop{B}
    \end{equation}
    Now \eqref{pf:qnorm:expbound} and \eqref{pf:qnorm:energybound} imply the needed result:
    \begin{equation}
        \normopadapt{\prod_{k=1}^n (\Id - \alpha_k \bA)} \leq \sqrt{\qcond} \cdot \normopadapt{\prod_{k=1}^n (\Id - \alpha_k \bA)}[Q] \leq \sqrt{\qcond} \cdot \exp\left(- \frac{a}{2}\sum_{k=1}^n \alpha_k\right)
    \end{equation}
\end{proof}


\begin{proposition}
~ \\
\label{prop:gnm_lowerbound}
\begin{enumerate}
    \item  
    $g_{1:n}$ defined as \eqref{def:gnm} satisfies
    \begin{equation}
        \label{bound:gnm}
        \frac{(n+1)^{1-\gamma}}{2 - \gamma} \leq g_{1:n} \leq  \frac{n^{1-\gamma}}{1 - \gamma} 
    \end{equation}

    \item Suppose $n \leq m$. Therefore 
    \begin{equation}
        g_{n:m} \geq \frac{(m+1)^{1-\gamma} - n^{1-\gamma}}{1 - \gamma}
    \end{equation}
\end{enumerate}
\end{proposition}

\begin{proof}
    For the first part, we use Bernoulli inequality and note that
    \[
        (n+1)^{1-\gamma} \geq 1+ n(1-\gamma) \geq 2 - \gamma
    \]
    \[
        \frac{1}{2-\gamma} (n+1)^{1-\gamma} \geq 1
    \]
    Consequently, since $x^{-\gamma}$ is decreasing over positive real numbers, an integral lower and upper bound yield \begin{align}
        g_{1:n} = \sum_{k=1}^n k^{-\gamma} \geq \int_{1}^{n+1} x^{-\gamma} \, dx = \frac{(n+1)^{1-\gamma} - 1}{1 - \gamma} \geq \frac{(n+1)^{1-\gamma} (1-1/(2-\gamma))}{1-\gamma} = \frac{(n+1)^{1-\gamma}}{2-\gamma}
    \end{align}
    and 
    \begin{align}
        g_{1:n} \leq \int_{0}^n x^{-\gamma} \, d x = \frac{n^{1-\gamma}}{1-\gamma}
    \end{align}
    Similarly for $n \leq m$ we have
    \begin{equation}
        g_{n:m} \geq \int_{n}^{m+1} x^{-\gamma} \, d x = \frac{(m+1)^{1-\gamma} - n^{1-\gamma}}{1 - \gamma}
    \end{equation}
\end{proof}

For simplicity we denote
\begin{equation}
    \label{def:beta}
    \beta = \frac{a \alpha_0}{2}
\end{equation}

The following proposition controls the operator norm of $\sum_{t=1}^n G_{1:t}^{(\alpha)}$.

\begin{proposition}
    \label{prop:bound_sum_g_1t}
    Let $\alpha_0 \in (0, \alpha_{\infty}]$. Then under the assumptions of \Cref{prop:hurwitz_stability} it holds
    \begin{equation}
        \label{bound:norm:sum:G1n}
        \normopadapt{\sum_{t=1}^n G_{1:t}^{(\alpha)}} \leq \sqrt{\qcond} \cdot  C_{\gamma, \beta}^{(G)}
    \end{equation}
    where $C_{\gamma, \beta}^{(G)}$ is a constant that depends only on $\gamma$, $\beta$, $a$, $\alpha_0$.
\end{proposition}

\begin{proof}
    The triangle inequality and {\Cref{cor:hurwitz_stability}}
     immediately imply that
    \begin{align}
        \label{proof:Gnm:first:bound}
        \normopadapt{\sum_{t=1}^n G_{1:t}^{(\alpha)}} \leq \sum_{t=1}^n \normop{G_{1:t}^{(\alpha)}} = \sum_{t=1}^n \normopadapt{\prod_{k=1}^t (\Id - \alpha_k \bA)} &\leq \sqrt{\qcond} \sum_{t=1}^n \exp\left(- \frac{a}{2}\sum_{k=1}^t \alpha_k\right) \\ &= \sqrt{\qcond}
        \sum_{t=1}^n \exp\left(- \frac{a \alpha_0}{2}g_{1:t}\right)
    \end{align}
    Recall $\beta$ defined as \eqref{def:beta} and consider 
    \begin{equation}
        c_t = \frac{2^{\frac{\gamma}{1-\gamma}}}{\beta^{\frac{1}{1-\gamma}}} \cdot (\beta g_{1:t+1} - \beta g_{1:t}) \cdot (\beta g_{1:t})^{\frac{1}{1-\gamma} - 1}
    \end{equation}
    {\Cref{prop:gnm_lowerbound}} reveals that $c_t \geq 1$:
    \begin{align}
        c_t = \frac{2^{\frac{\gamma}{1-\gamma}}}{\beta^{\frac{1}{1-\gamma}}} (\beta g_{1:t+1} - \beta g_{1:t}) (\beta g_{1:t})^{\frac{1}{1-\gamma} - 1} &= \frac{2^{\frac{\gamma}{1-\gamma}}}{\beta^{\frac{1}{1-\gamma}}} \cdot\frac{\beta}{(t+1)^{\gamma}} \left(\beta g_{1:t}\right)^{\frac{\gamma}{1-\gamma}} \\ &\geq \frac{2^{\frac{\gamma}{1-\gamma}}}{\beta^{\frac{1}{1-\gamma}}} \cdot\frac{\beta}{(t+1)^{\gamma}} \left(\beta \cdot \frac{(t+1)^{1-\gamma}}{2 - \gamma}\right)^{\frac{\gamma}{1-\gamma}} \\ &\geq  \frac{2^{\frac{\gamma}{1-\gamma}}}{\beta^{\frac{1}{1-\gamma}}} \cdot \frac{\beta}{(t+1)^{\gamma}} \left(\beta \cdot \frac{(t+1)^{1-\gamma}}{2}\right)^{\frac{\gamma}{1-\gamma}}= 1
    \end{align}
    Now we expand the upper bound \eqref{proof:Gnm:first:bound} using $c_t \geq 1$:
    \begin{align}
        \label{proof:Gnm:second_bound}
        \normopadapt{\sum_{t=1}^n G_{1:t}^{(\alpha)}} &\leq \sqrt{\qcond}
        \sum_{t=1}^n \exp\left(- \beta g_{1:t}\right) \leq \sqrt{\qcond}
        \sum_{t=1}^n c_t \exp\left(- \beta g_{1:t}\right)\\ &= \frac{2^{\frac{\gamma}{1-\gamma}}}{\beta^{\frac{1}{1-\gamma}}} \cdot \sqrt{\qcond}
        \sum_{t=1}^n \underbrace{(\beta g_{1:t+1} - \beta g_{1:t}) \cdot (\beta g_{1:t})^{\frac{1}{1-\gamma} - 1} \exp\left(- \beta g_{1:t}\right)}_{\mathcal{J}_t}
    \end{align}
    The right hand side of \eqref{proof:Gnm:second_bound} is an integral sum of $\phi(x) = x^{\frac{1}{1-\gamma} - 1} \exp(-x)$ approximating $\int_{\beta g_{1:1}}^{\beta g_{1:n+1}} \phi (x) \, d x$. Consider
    \begin{equation}
        \frac{d \phi}{d x} = \exp(-x) \cdot x^{\frac{\gamma}{1-\gamma} - 1} \cdot \left(\frac{\gamma}{1-\gamma} - x\right)
    \end{equation}
    Therefore, the maximum value of $\phi(x)$ is reached at the point $x_\gamma = \frac{\gamma}{1-\gamma}$. Note that by {\Cref{prop:gnm_lowerbound}}
    \begin{align}
        \frac{\phi(\beta g_{1:t+1})}{\phi(\beta g_{1:t})} = \left(1 + \frac{(t+1)^{-\gamma}}{g_{1:t}}\right)^{\frac{\gamma}{1-\gamma}} \cdot \exp(-\beta (t+1)^{-\gamma}) &\leq \left(1+\frac{(t+1)^{-\gamma}}{(t+1)^{1-\gamma}/(2-\gamma)}\right)^{\frac{\gamma}{1 - \gamma}} \\ &= \left(1+ \frac{2 - \gamma}{t+1}\right)^{\frac{\gamma}{1-\gamma}} \leq 2^{\frac{\gamma}{1-\gamma}} 
    \end{align}

    Since $\beta g_{1:t+1} - \beta g_{1:t}$ is at most $\beta 2^{-\gamma}$ and $\phi(x)$ has a unique maximum, we conclude that $\mathcal{J}_t$ defined at \eqref{proof:Gnm:second_bound} satisfies
    \begin{equation}
        \label{proof:Gnmbound:Jtbound}
        \mathcal{J}_t \leq M_{\gamma, \beta} \cdot \int_{\beta g_{1:t}}^{\beta g_{1:t+1}} \phi(x) \, d x
    \end{equation}
    where
    \begin{equation}
        \label{def:Mgamma}
        M_{\gamma, \beta} = \max\left\{1, ~ \frac{\phi(x_\gamma)}{\phi(x_\gamma-\beta 2^{-\gamma})}, ~ \frac{\phi(x_\gamma)}{\phi(x_\gamma + \beta 2^{-\gamma})}, ~ 2^{\frac{\gamma}{1-\gamma}}\right\}
    \end{equation}

    Also set
    \begin{equation}
        \label{def:CGgammabeta}
        C_{\gamma, \beta}^{(G)} = \frac{2^{\frac{\gamma}{1-\gamma}}}{\beta^{\frac{1}{1-\gamma}}}  \cdot M_{\gamma, \beta} \cdot \Gamma\left(\frac{1}{1-\gamma}\right)
    \end{equation}
    
    The needed result follows from \eqref{proof:Gnm:second_bound} and \eqref{proof:Gnmbound:Jtbound}:
    \begin{align}
        \label{bound:norm:sum_g1t:with_integral}
        \normopadapt{\sum_{t=1}^n G_{1:t}^{(\alpha)}} \leq \frac{2^{\frac{\gamma}{1-\gamma}}}{\beta^{\frac{1}{1-\gamma}}} \cdot \sqrt{\qcond}
        \sum_{t=1}^n {\mathcal{J}_t} &\leq \frac{2^{\frac{\gamma}{1-\gamma}}}{\beta^{\frac{1}{1-\gamma}}} \cdot \sqrt{\qcond} \cdot M_{\gamma, \beta} \int_{\beta g_{1:1}}^{\beta g_{1:n+1}} \phi(x) \, d x \\ &\leq \frac{2^{\frac{\gamma}{1-\gamma}}}{\beta^{\frac{1}{1-\gamma}}} \cdot \sqrt{\qcond} \cdot M_{\gamma, \beta} \int_{0}^{+\infty} \phi(x) \, d x \\ &= \frac{2^{\frac{\gamma}{1-\gamma}}}{\beta^{\frac{1}{1-\gamma}}} \cdot \sqrt{\qcond} \cdot M_{\gamma, \beta} \cdot \Gamma\left(\frac{1}{1-\gamma}\right) \\ &= \sqrt{\qcond}\cdot C_{\gamma, \beta}^{(G)}
    \end{align}
\end{proof}

Now we provide a technical proposition.

\begin{proposition}
    \label{prop:bound_for_st_prop}
    Let $p \geq  1$, $0 < q < 1$ and $t > 0$. Then it holds
    \begin{equation}
        1 + q (1+t)^p \geq (1+qt)^p
    \end{equation}
\end{proposition}

\begin{proof}
    We introduce a function
    \[f(t) = 1 + q(1+t)^p - (1+qt)^p\]
    Note that $f(0) = q > 0$. Consider $f'(t)$:
    \[f'(t) = pq(1+t)^{p-1} - pq(1+qt)^{p-1} = pq((1+t)^{p-1} - (1 + qt)^{p-1}) \geq 0\]
    Hence, $f(t) \geq 0$ for all $t \geq 0$ which implies the needed inequality.
\end{proof}

\begin{proposition}
    \label{prop:st_bound}
    Let $\alpha_0 \in (0, \alpha_{\infty}]$. Then under the assumptions of {\Cref{prop:hurwitz_stability}} it holds
    \begin{equation}
        \label{bound:stmatrix}
        \normop{S_t} \leq \sqrt{\qcond} \cdot C_{\gamma, \beta}^{(S)} \cdot t^{\gamma-1}
    \end{equation}
    where $C_{\gamma, \beta}^{(S)}$ is a constant that depends only on $\gamma$, $\beta$, $a$, $\alpha_0$.
\end{proposition}

\begin{proof}
    Now we will apply technique similar to the one described in \citep[pp. 25-26]{wu2024statisticalinferencetemporaldifference}. Recall that
    \begin{equation}
        S_t = \sum_{j=t+1}^{n} (\alpha_t - \alpha_j) G_{t+1:j-1}^{(\alpha)}
    \end{equation}
    First we use {\Cref{cor:hurwitz_stability}} and obtain a primary bound for $\normop{S_t}$:
    \begin{align}
        \label{proof:st:primary:bound}
        \normop{S_t} \leq \sum_{j=t+1}^n (\alpha_t - \alpha_j) \normop{G_{t+1:j-1}^{\alpha}} &\leq \sqrt{\qcond} \cdot \sum_{j=t+1}^n (\alpha_t - \alpha_j) \exp\left(-\beta g_{t+1:j-1} \right) \\ &= \sqrt{\qcond} \cdot \alpha_0 \cdot \sum_{j=t+1}^{n} (t^{-\gamma} - j^{-\gamma}) \exp(-\beta g_{t+1:j-1}) \\ &= \sqrt{\qcond} \cdot \alpha_0 \cdot \sum_{j=t}^{n-1} (t^{-\gamma} - (j+1)^{-\gamma}) \exp(-\beta g_{t+1:j}) \\ &= \sqrt{\qcond} \cdot \alpha_0 \cdot \sum_{j=t}^{n-1} (j+1)^{-\gamma} \left( \left(\frac{j+1}{t}\right)^{\gamma}  - 1\right) \exp(-\beta g_{t+1:j})
    \end{align}
    The second part of {\Cref{prop:gnm_lowerbound}} directly implies that
    \begin{equation}
        \label{bound:st:fraction:jt}
        \left(\frac{j+1}{t}\right)^{1-\gamma} - 1 \leq \frac{(1 - \gamma) g_{t:j}}{t^{1-\gamma}}
    \end{equation}
    Hence we get
        \begin{equation}
        \label{bound:st:fraction:jt}
        \left(\frac{j+1}{t}\right)^{\gamma} - 1 \leq \left(\frac{(1 - \gamma) g_{t:j}}{t^{1-\gamma}}+1\right)^{\frac{\gamma}{1-\gamma}} - 1
    \end{equation}
    Since $\gamma \in (1/2; 1)$, $t^{\gamma-1} < 1$ and $\frac{\gamma}{1-\gamma} \geq 1$. Therefore, the assumptions of \Cref{prop:bound_for_st_prop} hold, so we get
    \begin{align}
        \label{corrolary:prop5:bound:for:St}
                 1 + t^{\gamma-1} \left(1 + (1-\gamma) g_{t:j}\right)^{\frac{\gamma}{1-\gamma}} \geq  \left(1+ t^{\gamma-1} (1-\gamma) g_{t:j} \right)^{\frac{\gamma}{1-\gamma}}
    \end{align}   
    Denote for simplicity $a_{t:j} = 1 + (1-\gamma) g_{t:j}$. Then $g_{t:j} = \frac{a_{t:j} -  1}{1 - \gamma}$ and $(j+1)^{-\gamma} = \frac{a_{t:j+1} - a_{t:j}}{1 - \gamma}$. Combining \eqref{corrolary:prop5:bound:for:St} with \eqref{bound:st:fraction:jt} we obtain
    \begin{equation}
        \left(\frac{j+1}{t}\right)^{\gamma} - 1 \leq t^{\gamma-1} \left(1 + (1-\gamma) g_{t:j}\right)^{\frac{\gamma}{1-\gamma}} = t^{\gamma - 1} (a_{t:j})^{\frac{\gamma}{1-\gamma}}
    \end{equation}
    Thus, we can expand the bound \eqref{proof:st:primary:bound}:
    \begin{align}
        \normop{S_t} &\leq \sqrt{\qcond} \alpha_0 \sum_{j=t}^{n-1} (j+1)^{-\gamma} \left( \left(\frac{j+1}{t}\right)^{\gamma}  - 1\right) \exp(-\beta g_{t+1:j}) \\ &\leq \sqrt{\qcond} \alpha_0 \cdot \sum_{j=t}^{n-1} \frac{a_{t:j+1} - a_{t:j}}{1-\gamma} t^{\gamma-1} (a_{t:j})^{\frac{\gamma}{1-\gamma}} \underbrace{\exp\left(\frac{\beta}{t^{\gamma}}\right) \exp\left(-\beta\frac{a_{t:j} - 1}{1-\gamma}\right)}_{=\exp(-\beta g_{t+1:j})} \\ 
        &\leq \frac{\sqrt{\qcond} \alpha_0}{1-\gamma} \exp\left(\beta+ \frac{\beta}{1-\gamma}\right) t^{\gamma-1} \sum_{j=t}^{n-1} (a_{t:j+1} - a_{t:j})  (a_{t:j})^{\frac{\gamma}{1-\gamma}} \exp\left(-\beta\frac{a_{t:j}}{1-\gamma}\right)
    \end{align}
    The right hand side can be bounded similarly to \eqref{bound:norm:sum_g1t:with_integral} using an integral for $\Gamma\left(\frac{\beta}{1-\gamma}\right)$. Therefore, there exists a constant $C_{\gamma, \beta}^{(S)}$ such that 
    \begin{align}
        \normop{S_t} \leq \sqrt{\qcond} \cdot C_{\gamma, \beta}^{(S)} \cdot t^{\gamma-1}
    \end{align}
\end{proof}

\begin{proposition}
    \label{prop:g_t:n_upperbound}
    Let $\alpha_0 \in (0, \alpha_{\infty}]$. Then under the assumptions of {\Cref{prop:hurwitz_stability}} for every $m \in \mathbb{N}$ it holds
    \begin{equation}
        \sum_{t=1}^n \normop{G_{t:n}}^m \leq \frac{\qcond^{m/2}}{1-(1-\beta n^{-\gamma})^m}
    \end{equation}
\end{proposition}

\begin{proof}
\Cref{cor:hurwitz_stability} implies that
\begin{align} 
        \sum_{t=1}^n \normop{G_{t:n}}^m &\leq \sum_{t=1}^n \prod_{k=t}^n (1 - \beta k^{-\gamma})^m \leq \qcond^{m/2} \cdot \sum_{t=1}^n \prod_{k=t+1}^n (1 - \beta k^{-\gamma})^m \\ &= \qcond^{m/2} \cdot \sum_{t=1}^n (1 - (1 - \beta t^{-\gamma})^m)^{-1} \cdot \left( \prod_{k=t+1}^n (1 - \beta k^{-\gamma})^m - \prod_{k=t}^n (1 - \beta k^{-\gamma})^m \right) \\ &\leq \qcond^{m/2} (1 - (1 - \beta n^{-\gamma})^m)^{-1} \cdot \sum_{t=1}^n \left( \prod_{k=t+1}^n (1 - \beta k^{-\gamma})^m - \prod_{k=t}^n (1 - \beta k^{-\gamma})^m \right)\\ &= 
        \qcond^{m/2} (1 - (1 - \beta n^{-\gamma})^m)^{-1} \left(1 -  \prod_{k=1}^n (1 - \beta k^{-\gamma})^m \right) \\ &\leq \frac{\qcond^{m/2}}{1 - (1 - \beta n^{-\gamma})^m}
    \end{align}
\end{proof}

\begin{lemma}
\label{lem:sigma_n_bound}
    Let $\alpha_0 \in (0, \alpha_{\infty}]$. Then under the assumptions of {\Cref{prop:hurwitz_stability}} it holds
    \begin{align}
        \label{bound:norm_of_bL_minus_Lstar}
        \normopadapt{\Sigma_n - \Sigma_{\infty}} \leq \mathcal{C}_1 n^{\gamma-1} + {\mathcal{C}}_2 n^{2(\gamma-1)}
    \end{align}
    where the constants $\mathcal{C}_1$, $\mathcal{C}_2$ are defined as follows
    \begin{align}
        \label{lemma:constants definition}
        &\mathcal{C}_1 = \frac{\qcond \normop{\Sigma_{\infty}}}{2\beta - \beta^2} 
        \\
         &\mathcal{C}_2 = 2\sqrt{\qcond} \normop{\Sigma_{\infty}} C_{\gamma, \beta}^{(G)} + \frac{\normop{\noisecov} \qcond \left(C_{\gamma, \beta}^{(S)}\right)^2}{2\gamma-1} + \frac{2 \qcond \normop{\bA \Sigma_{\infty}} C_{\gamma, \beta}^{(S)}}{\beta} 
    \end{align}
\end{lemma}
\begin{proof}
    Recall the representation \eqref{repr:Lstar_minus_Ln}. First, we will bound $D_1$. The operator norms of both terms are equal because one is a transposed version of another, so it is sufficient to bound only one of them. Note that $G_{n:m}^{(\alpha)}$, $Q_t$, $\bA$, $\bA^{-1}$, commute as polynomials in $\bA$. Now we remember the representation \eqref{repr:sumqtminusa} and obtain
    \begin{align}
        \normopadapt{\frac{1}{n}\sum_{t=1}^n (Q_t - \bA^{-1})\noisecov \bA^{-\top}} &= \normopadapt{-\frac{1}{n} \bA^{-1} \sum_{j=1}^n G_{1:j}^{(\alpha)}\noisecov \bA^{-\top}} \\ &= \normopadapt{n^{-1} \Sigma_{\infty}  \sum_{j=1}^n G_{1:j}} \leq n^{-1} \normopadapt{\Sigma_{\infty}} \cdot \normopadapt{\sum_{j=1}^n G_{1:j}}
    \end{align}
    {\Cref{prop:bound_sum_g_1t}} directly imply the bound for $D_1$:
    \begin{align}
        \normopadapt{\frac{1}{n}\sum_{t=1}^n (Q_t - \bA^{-1})\noisecov \bA^{-\top}} \leq n^{-1} \normopadapt{\Sigma_{\infty}} \cdot \normopadapt{\sum_{j=1}^n G_{1:j}} \leq n^{-1} \normopadapt{\Sigma_{\infty}} \cdot \sqrt{\qcond} \cdot C_{\gamma, \beta}^{(G)}
    \end{align}
    Hence
    \begin{align}
        \label{lemma:D1_bound}
        \normop{D_1} \leq 2 n^{-1}\normopadapt{\Sigma_{\infty}} \cdot \sqrt{\qcond} \cdot C_{\gamma, \beta}^{(G)}
    \end{align}
    Now it is time to bound the norm of $D_2$. Recall the formula \eqref{repr:qtminusa} and consider
    \begin{align}
        \label{lemma:D2_expanded_repr}
        &n^{-1}\sum_{t=1}^n(Q_t - \bA^{-1}) \noisecov (Q_t - \bA^{-1})^\top \\
        &\qquad = n^{-1}\sum_{t=1}^n\left(S_t - \bA^{-1} \prod_{k=t}^n (\Id - \alpha_k \bA)\right) \noisecov \left(S_t - \bA^{-1} \prod_{k=t}^n (\Id - \alpha_k \bA)\right)^\top \\
        &\qquad = \underbrace{n^{-1} \sum_{t=1}^n S_t \noisecov S_t^\top}_{D_{21}} + \underbrace{n^{-1}\sum_{t=1}^n\bA^{-1} \prod_{k=t}^n (\Id - \alpha_k \bA) \noisecov \bA^{-\top} \prod_{k=t}^n (\Id - \alpha_k \bA)^\top}_{D_{22}} \\ 
        &\qquad\qquad \qquad  -\underbrace{n^{-1} \sum_{t=1}^n \bA^{-1} \prod_{k=t}^n (\Id - \alpha_k \bA) \cdot \noisecov S_t^\top}_{D_{23}} - \underbrace{n^{-1}\sum_{t=1}^n S_t \noisecov \bA^{-\top} \prod_{k=t}^n (\Id - \alpha_k \bA)^{\top}}_{D_{24}}\eqsp.
    \end{align}
    {\Cref{prop:gnm_lowerbound}} and {\Cref{prop:st_bound}}  reveal an evident bound for $\normop{D_{21}}$:
    \begin{align}
        \label{lemma:D21_bound}
        \normop{D_{21}} = \normopadapt{n^{-1} \sum_{t=1}^n S_t \noisecov S_t^\top} &\leq n^{-1} \sum_{t=1}^n \normop{\noisecov} \normop{S_t}^2 \\  &\leq n^{-1} \normop{\noisecov} \sum_{t=1}^n \qcond \left(C_{\gamma, \beta}^{(S)}\right)^2 t^{2(\gamma-1)} \\ &\leq
        n^{-1} \normop{\noisecov} \qcond \left(C_{\gamma, \beta}^{(S)}\right)^2 \frac{n^{1+2(\gamma - 1)} - 1}{2\gamma - 1} \\ &\leq n^{-1} \normop{\noisecov} \qcond \left(C_{\gamma, \beta}^{(S)}\right)^2 \frac{n^{1+2(\gamma - 1)}}{2\gamma - 1} \\ &= n^{2(\gamma - 1)} \frac{\normop{\noisecov} \qcond \left(C_{\gamma, \beta}^{(S)}\right)^2}{2\gamma - 1} 
    \end{align}
    Recall that $\beta = \frac{a \alpha_0}{2}$. We use {\Cref{prop:g_t:n_upperbound}} to get a bound for $\normop{D_{22}}$:
    \begin{align} 
        \label{lemma:D22_bound}
        \normop{D_{22}} &= \normopadapt{n^{-1}\sum_{t=1}^n \prod_{k=t}^n (\Id - \alpha_k \bA) \bA^{-1} \noisecov \bA^{-\top} \prod_{k=t}^n (\Id - \alpha_k \bA)^\top} \\ &\leq n^{-1} \normop{\Sigma_\infty} \sum_{t=1}^n \normop{G_{t:n}}^2 \\ &\leq n^{-1} \cdot \frac{\qcond\cdot \normop{\Sigma_{\infty}}}{2\beta n^{-\gamma} - \beta^2 n^{-2\gamma}} \leq n^{\gamma - 1} \frac{\qcond \normop{\Sigma_\infty}}{2\beta - \beta^2}
    \end{align}
    Since $D_{23} = D_{24}^\top$, we concentrate on $\normop{D_{24}}$. {\Cref{cor:hurwitz_stability}} and {\Cref{prop:st_bound}} immediately imply 
    \begin{align}
        \normop{D_{24}} &= \normopadapt{n^{-1}\sum_{t=1}^n S_t \noisecov \bA^{-\top} \prod_{k=t}^n (\Id - \alpha_k \bA)^{\top}} \leq n^{-1} \normop{\noisecov \bA^{-\top}} \sum_{t=1}^n \normop{S_t} \normopadapt{\prod_{k=t}^n (\Id - \alpha_k \bA)^{\top}} \\ &\leq n^{-1} \normop{\bA \Sigma_{\infty}} \sum_{t=1}^n \sqrt{\qcond} t^{\gamma-1} C_{\gamma, \beta}^{(S)} \sqrt{\qcond} \prod_{k=t}^n (1- \beta k^{-\gamma}) \\ &\leq n^{-1} \qcond \normop{\bA \Sigma_{\infty}} C_{\gamma, \beta}^{(S)} \sum_{t=1}^n \frac{t^{2\gamma - 1}}{\beta} \beta t^{-\gamma} \prod_{k=t+1}^n (1 - \beta k^{-\gamma}) \\ &= n^{-1} \qcond \normop{\bA \Sigma_{\infty}} C_{\gamma, \beta}^{(S)} \sum_{t=1}^n \frac{t^{2\gamma - 1}}{\beta}  \left(\prod_{k=t+1}^n (1 - \beta k^{-\gamma}) - \prod_{k=t}^n (1 - \beta k^{-\gamma})\right) \\ &\leq n^{-1+2\gamma-1} \frac{\qcond \normop{\bA \Sigma_{\infty}} C_{\gamma, \beta}^{(S)}}{\beta} \sum_{t=1}^{n} \left(\prod_{k=t+1}^n (1 - \beta k^{-\gamma}) - \prod_{k=t}^n (1 - \beta k^{-\gamma})\right) \\ &= n^{2(\gamma-1)} \frac{\qcond \normop{\bA \Sigma_{\infty}} C_{\gamma, \beta}^{(S)}}{\beta} \left(1 - \prod_{k=1}^n (1 - \beta k^{-\gamma})\right) \\ &\leq 
        n^{2(\gamma-1)} \frac{\qcond \normop{\bA \Sigma_{\infty}} C_{\gamma, \beta}^{(S)}}{\beta}
    \end{align}

    Hence 
    \begin{equation}
        \label{lemma:proof:d23_d24_bound}
        \normop{D_{23} + D_{24}} \leq n^{2(\gamma-1)} \frac{2\qcond \normop{\bA \Sigma_{\infty}} C_{\gamma, \beta}^{(S)}}{\beta}
    \end{equation}

    The needed result follows from \eqref{lemma:D1_bound}, \eqref{lemma:D21_bound}, \eqref{lemma:D22_bound}, \eqref{lemma:proof:d23_d24_bound} using inequality $n^{-1}\leq n^{2(\gamma-1)}$ and gathering similar terms.
\end{proof}