\begin{wrapfigure}{r}{0.61\linewidth}
  \begin{mdframed}
    {\footnotesize\begin{align*}
    \text{Expressions } \texttt{e} ::= \ & \texttt{x} \mid \tt \mid \ff \mid
    \texttt{e} \land \texttt{e} \mid \texttt{e} \lor \texttt{e} \mid
    \neg \texttt{e} &\\
    \text{Statements } \texttt{s} ::= \ & \texttt{x} = e \mid x = \flip{\theta} \mid \texttt{s} ; \texttt{s}&\\
    &\mid
    \texttt{if e \{s\} else \{s\}} &\\
    &\mid (\texttt{m}_1, \hdots, \texttt{m}_n) = \texttt{mmap}(\texttt{x}_1, \hdots, \texttt{x}_n) &\\
    &\mid (\texttt{m}_1, \hdots, \texttt{m}_n) = \texttt{mmap}(\texttt{x}_1, \hdots, \texttt{x}_n) \; \texttt{with} \; \{ \texttt{e} \} &\\
    \text{Programs } P ::= \ & \texttt{s} ; \Pr(\texttt{e}) \mid \texttt{s} ; \Pr(\texttt{e}) \; \texttt{with} \; \{ \texttt{e}  \}
    \end{align*}}
  \end{mdframed}
    \caption{Full $\pineappl$ syntax.}
    \label{fig:pineappl-syntax}
\end{wrapfigure}
