\begin{figure}
\begin{mdframed}
  {\footnotesize
  \begin{align*}
    \infer[var/\top]
    {
        x[\sigma] = \top
    }
    {
        \sigma(x) = \top
    }
    \infer[var/\bot]
    {
        x[\sigma] = \bot
    }
    {
        \sigma(x) = \bot
    }
    \infer[\neg/\top]
    {
        \neg e[\sigma] = \bot
    }
    {
        e[\sigma] = \top
    }
    \infer[\neg/\bot]
    {
        \neg e[\sigma] = \top
    }
    {
        e[\sigma] = \bot
    }
  \end{align*}
  \begin{align*}
    \infer[\land/\top\top]
    {
        (e_1 \land e_2)[\sigma] = \top
    }
    {
        e_1[\sigma] = \top
        & e_2[\sigma] = \top
    }
    \infer[\land/\top\bot]
    {
        (e_1 \land e_2)[\sigma] = \bot
    }
    {
        e_1[\sigma] = \top
        & e_2[\sigma] = \bot
    }
  \end{align*}
  \begin{align*}
    \infer[\land/\bot\top]
    {
        (e_1 \land e_2)[\sigma] = \bot
    }
    {
        e_1[\sigma] = \bot
        & e_2[\sigma] = \top
    }
    \infer[\land/\bot\bot]
    {
        (e_1 \land e_2)[\sigma] = \bot
    }
    {
        e_1[\sigma] = \bot
        & e_2[\sigma] = \bot
    }
  \end{align*}
  \begin{align*}
    \infer[\lor/\top\top]
    {
        (e_1 \lor e_2)[\sigma] = \top
    }
    {
        e_1[\sigma] = \top
        & e_2[\sigma] = \top
    }
    \infer[\lor/\top\bot]
    {
        (e_1 \lor e_2)[\sigma] = \top
    }
    {
        e_1[\sigma] = \top
        & e_2[\sigma] = \bot
    }
  \end{align*}
  \begin{align*}
    \infer[\lor/\bot\top]
    {
        (e_1 \lor e_2)[\sigma] = \top
    }
    {
        e_1[\sigma] = \bot
        & e_2[\sigma] = \top
    }
    \infer[\lor/\bot\bot]
    {
        (e_1 \lor e_2)[\sigma] = \bot
    }
    {
        e_1[\sigma] = \bot
        & e_2[\sigma] = \bot
    }
  \end{align*}
  }
\end{mdframed}
\caption{Expression evaluation relation}
\label{fig:pineappl-expr-eval}
\end{figure}