%\section{Algorithm 1}
%Let
%\[
%f(\vec{w})=-\lambda_1\vec{w}^{\top}\vec{r}+\lambda_2(\vec{w}^{\top}\vec{r}-E)^2-\lambda_3(\vec{w}^{\top}\vec{r}-E)^3+\lambda_4(\vec{w}^{\top}\vec{r}-E)^4-\lambda_5(\vec{w}^{\top}\vec{r}-E)^5
%\]
%Suppose $\vec{w}=(w_1,...,w_n)$, and denote $f_i=\frac{\partial f}{\partial w_i}$, the partial derivative is calculated as:
%\[
%f_i=\frac{\partial f}{\partial w_i}=r_i\left(-\lambda_1+2\lambda_2(\vec{w}^{\top}\vec{r}-E)-3\lambda_3(\vec{w}^{\top}\vec{r}-E)^2+4\lambda_4(\vec{w}^{\top}\vec{r}-E)^3-5\lambda_5(\vec{w}^{\top}\vec{r}-E)^4\right).
%\]

 %Set $\beta=1000$, $\epsilon=0.001$ (can be changed). Initialize $\vec{w}_0\in$ simplex. 
 
 %\textbf{For}  $k=1,2,....$, 
 

 %\ \ \ \ \ Compute $S_{\vec{w}}=\sum_{j=1}^n\frac{1}{w_j}$;
 
 %\ \ \ \ \ \textbf{For} $i=\{1,...,n\}$: 
 
 %\begin{itemize}
 %\item Sample $z_i\sim\mathcal{N}(0,1)$;
 %\item Compute 
 %\[
 %V_0^i=\frac{\epsilon}{2\beta}(n+1-(1+w_i)S_{\vec{w}})+\sqrt{2\epsilon\beta^{-1}w_i}z_i;
 %\]
 \item Compute 
 \[
 f_i=r_i\left(-\lambda_1+2\lambda_2(\vec{w}^{\top}\vec{r}-E)-3\lambda_3(\vec{w}^{\top}\vec{r}-E)^2+4\lambda_4(\vec{w}^{\top}\vec{r}-E)^3-5\lambda_5(\vec{w}^{\top}\vec{r}-E)^4\right);
 \]
 \item Update
 \[
 w_i\leftarrow \frac{w_i-\epsilon w_if_i}{1-\epsilon\sum_{j=1}^nw_j f_j};
 \]
 \end{itemize}
 \textbf{Until} $k$ is large enough or $\abs{f(\vec{w}_k)-f(\vec{w}_{k-1})}<\text{Threshold}$