\section{Omitted Details in \pref{sec:alt-game}}\label{app:alt-game}
In this section, we show the proof of \pref{thm:zero-sum} and \pref{thm:general-sum}, which are proven according to the definition of NE and CCE respectively. 

\begin{proof}[Proof of \pref{thm:zero-sum}]
    Let $y_0$ be the output of $\Alg_y$ with an empty sequence of loss functions. According to \pref{alg:alternation}, the loss function for the \( x \)-player at round \( t \) is given by \( u_1(\cdot, y_t) \), while the loss function for the \( y \)-player at the same round is $ u_2(x_t, \cdot)$.
    By definition of alternating regret and using $u_2=-u_1$, we know that for any $x\in\calX$ and $y\in\calY$,
    \begin{align*}
        &\sum_{t=1}^T\left(u_1(x_t,y_t)+u_1(x_{t+1},y_t)\right) - 2\sum_{t=1}^T u_1(x,y_t)\leq \RegAlt^x,\\
        &\sum_{t=0}^{T-1}\left(u_2(x_{t+1},y_{t})+u_2(x_{t+1},y_{t+1})\right) - 2\sum_{t=0}^{T-1} u_2(x_{t+1},y)\\
        &=2\sum_{t=0}^{T-1} u_1(x_{t+1},y) - \sum_{t=0}^{T-1}\left(u_1(x_{t+1},y_{t})+u_1(x_{t+1},y_{t+1})\right)\leq \RegAlt^y.
    \end{align*}
    Taking a summation over both equations, we obtain that
    \begin{align*}
        2\sum_{t=1}^{T} u_1(x_{t},y) - 2\sum_{t=1}^T u_1(x,y_t)&\leq \RegAlt^x + \RegAlt^y+u_1(x_1,y_0)-u_1(x_{T+1},y_T)\\
        &\leq \RegAlt^x + \RegAlt^y + 2.
    \end{align*}
    Since $u_1(x,y)$ is convex in $x$ and concave in $y$, using Jensen's inequality, we know that for any $x\in\calX$ and $y\in\calY$,
    \begin{align*}
        u_1\left(\overline{x}_T,y\right) - u_1(x,\overline{y}_T) \leq \frac{\RegAlt^x + \RegAlt^y + 2}{2T} = \order\left(\frac{\RegAlt^x + \RegAlt^y}{T}\right),
    \end{align*}
    where $\overline{x}_T=\frac{1}{T}\sum_{t=1}^Tx_t$ and $\overline{y}_T=\frac{1}{T}\sum_{t=1}^Ty_t$. This further means that
    \begin{align*}
        0\leq \max_{y\in\calY}u_1(\overline{x}_T,y)-u_1(\overline{x}_T,\overline{y}_T) \leq \order\left(\frac{\RegAlt^x + \RegAlt^y}{T}\right), \\
        0\leq u_1(\overline{x}_T,\overline{y}_T) - \min_{x\in\calX}u_1(x,\overline{y}_T) \leq \order\left(\frac{\RegAlt^x + \RegAlt^y}{T}\right),
    \end{align*}
    which finishes the proof by the definition of an $\epsilon$-NE with $\epsilon=\order\left(\frac{\RegAlt^x + \RegAlt^y}{T}\right)$.
\end{proof}


\begin{proof}[Proof of \pref{thm:general-sum}]
    Similar to the proof of \pref{thm:zero-sum}, let $y_0$ be the output of $\Alg_y$ with an empty sequence of loss functions. By definition of alternating regret, we know that for any $x'\in\calX$ and $y'\in\calY$,
    \begin{align}
        &\sum_{t=1}^T\left(u_1(x_t,y_t)+u_1(x_{t+1},y_t)\right) - 2\sum_{t=1}^T u_1(x',y_t)\leq \RegAlt^x,\label{eqn:gsum-1}\\
        &\sum_{t=0}^{T-1}\left(u_2(x_{t+1},y_{t})+u_2(x_{t+1},y_{t+1})\right) - 2\sum_{t=0}^{T-1} u_2(x_{t+1},y')\leq \RegAlt^y.\label{eqn:gsum-2}
    \end{align}
    Define $\calP$ to be the uniform distribution over $\{(x_t,y_t),(x_{t+1},y_t)\}_{t\in[T]}$.
    Adding $u_2(x_{T+1},y_T)-u_2(x_1,y_0)+u_2(x_1,y')-u_2(x_{T+1},y')\in[-4,4]$ on both sides of \pref{eqn:gsum-2} and dividing $2T$ on both sides of \pref{eqn:gsum-1} and \pref{eqn:gsum-2}, we know that for any $x'\in\calX$ and $y'\in\calY$,
    \begin{align*}
    \E_{(x,y)\sim \calP}\left[u_1(x,y)\right] - \E_{(x,y)\sim \calP}\left[u_1(x',y)\right]&\leq \frac{\RegAlt^y}{2T},\\
        \E_{(x,y)\sim \calP}\left[u_2(x,y)\right] - \E_{(x,y)\sim \calP}\left[u_2(x,y')\right]&\leq \frac{\RegAlt^y + 4}{2T}.
    \end{align*}
    This finishes the proof by the definition of an $\epsilon$-CCE with $\epsilon=\order\left(\frac{\max\{\RegAlt^x, \RegAlt^y\}}{T}\right)$.
\end{proof}