\section{Omitted Details in \pref{sec: alt-oco}}\label{app:CEW}
In this section, we show the omitted proofs in \pref{sec: alt-oco}. In the following, we provide the proof of \pref{thm:hedge_simplex}.

\begin{proof}[Proof of \pref{thm:hedge_simplex}]
    We aim to show that
    \begin{align}
        \inner{p_t-u,\ell_t} &= \frac{1}{\eta}\left(\KL(u,p_t) - \KL(u,p_{t+1}) + \KL(p_t,p_{t+1})\right),\label{eqn:regular-expert}\\
        \inner{p_{t+1}-u, \ell_t} &= \frac{1}{\eta}\left(\KL(u,p_t) - \KL(u,p_{t+1}) - \KL(p_{t+1},p_{t})\right).\label{eqn:cheat-expert}
    \end{align}
    Note that the dynamic of Hedge implies that $p_{t+1,i}=\frac{p_{t,i}\exp(-\eta\ell_{t,i})}{\sum_{j=1}^dp_{t,j}\exp(-\eta\ell_{t,j})}$. Direct calculation shows that
    \begin{align*}
        &\frac{1}{\eta}\left(\KL(u,p_t) - \KL(u,p_{t+1}) + \KL(p_t,p_{t+1})\right)
        \\
        &= \frac{1}{\eta}\sum_{i=1}^d (p_{t,i}-u_i)\cdot\log\frac{p_{t,i}}{p_{t+1,i}} \\
        &= \sum_{i=1}^d (p_{t,i}-u_i)\left(\ell_{t,i} + \frac{1}{\eta}\log\left(\sum_{j=1}^dp_{t,j}\exp(-\eta\ell_{t,j})\right)\right) \\
        &=\inner{p_t-u,\ell_t},\\
        &\frac{1}{\eta}\left(\KL(u,p_t) - \KL(u,p_{t+1}) - \KL(p_{t+1},p_{t})\right)
        \\
        &= \frac{1}{\eta}\sum_{i=1}^d (p_{t+1,i}-u_i)\cdot\log\frac{p_{t,i}}{p_{t+1,i}} \\
        &= \sum_{i=1}^d (p_{t+1,i}-u_i)\left(\ell_{t,i} + \frac{1}{\eta}\log\left(\sum_{j=1}^dp_{t,j}\exp(-\eta\ell_{t,j})\right)\right) \\
        &=\inner{p_{t+1}-u,\ell_t}.
    \end{align*}
    Combining \pref{eqn:regular-expert} and \pref{eqn:cheat-expert} for all $t\in[T]$, we obtain that
    \begin{align}\label{eqn:alt-regret-simplex}
        \RegAlt(u) = \frac{2(\KL(u,p_1)-\KL(u,p_{T+1}))}{\eta} + \frac{1}{\eta}\sum_{t=1}^T\left(\KL(p_t,p_{t+1})- \KL(p_{t+1},p_t)\right).
    \end{align}
    Since $p_1$ is the uniform distribution over all $d$ experts, we can bound $\KL(u,p_1)-\KL(u,p_{T+1})\leq \log d$. To control the term $\KL(p_t,p_{t+1})- \KL(p_{t+1},p_t)$, define $G(x)=\log(\sum_{i=1}^d\exp(x_i))$ for $x\in\R^d$ and $L_t=\sum_{\tau\leq t}\ell_{\tau}$. Direct calculation shows that
    \begin{align*}
        &D_G(-\eta L_t, -\eta L_{t-1}) - D_G(-\eta L_{t-1}, -\eta L_{t}) \\
        &=2\log\left(\sum_{i=1}^d\exp(-\eta L_{t,i})\right) - 2\log\left(\sum_{i=1}^d\exp(-\eta L_{t-1,i})\right) + \sum_{i=1}^dp_{t+1,i}\cdot (\eta\ell_{t,i}) + \sum_{i=1}^dp_{t,i}\cdot(\eta\ell_{t,i}) \\
        &=\KL(p_t,p_{t+1})- \KL(p_{t+1},p_t).
    \end{align*}
    
    Applying Lemma A.2 of~\citet{wibisono2022alternating}, we know that $\KL(p_t,p_{t+1})- \KL(p_{t+1},p_t)\leq \frac{4}{3}\|\eta\ell_t\|_{\infty}^3\leq \frac{4}{3}\eta^3$, where the first inequality is because $G(x)$ is $8$-smooth of order 3 as proven in Example A.3~\citet{wibisono2022alternating}. Plugging the above to \pref{eqn:alt-regret-simplex} and picking the optimal $\eta$ finishes the proof.
\end{proof}

In the following, we show the proof for \pref{thm:hedge-cont}.
\begin{proof}[Proof of \pref{thm:hedge-cont}]
    By definition, we know that $p_t(x)=\frac{1}{Z_t}\exp(-\eta F_{t-1}(x))$ and $p_{t+1}(x)=\frac{1}{Z_{t+1}}\exp(-\eta F_{t}(x))$, where $Z_t = \int_{x\in\calX}\exp(-\eta F_{t-1}(x))dx$ and $F_t(x) = \sum_{\tau\leq t}f_{\tau}(x)$.
    Then, direct calculation shows that
    \begin{align*}
        \frac{1}{\eta}\KL(p_t,p_{t+1})        &= \frac{1}{\eta}\int_{x\in\calX}p_t(x)\log\frac{p_t(x)}{p_{t+1}(x)}dx\\
        &= \int_{x\in\calX}p_t(x)\left(f_t(x)+\frac{1}{\eta}\log\frac{Z_{t+1}}{Z_{t}}\right)dx
        \\
        &= \int_{x\in\calX}p_t(x)f_t(x)dx + \frac{1}{\eta}\left(\log Z_{t+1} - \log Z_t\right)
        \\
        \frac{1}{\eta}\KL(p_{t+1},p_{t})&= \frac{1}{\eta}\int_{x\in\calX}p_{t+1}(x)\log\frac{p_{t+1}(x)}{p_{t}(x)}dx\\
        &= \int_{x\in\calX}p_{t+1}(x)\left(-f_t(x)+\frac{1}{\eta}\log\frac{Z_{t}}{Z_{t+1}}\right)dx
        \\
        &= -\int_{x\in\calX}p_{t+1}(x)f_t(x)dx +\frac{1}{\eta}( \log Z_{t} - \log Z_{t+1})
    \end{align*}
    Combining the above two inequalities, we have
   
    \begin{align}
        \int_{x\in\calX}(p_t(x)+p_{t+1}(x))f_t(x)dx + \frac{2}{\eta}(\log Z_{T+1} - \log Z_{1}) = \frac{1}{\eta}\left(\KL(p_t,p_{t+1}) - \KL(p_{t+1},p_t)\right) .\label{eqn:alt-regret-cont}
    \end{align}
    According to the proof of Theorem 3.1 in \citet{bubeck2011introduction}, we know that 
    \begin{align*}
        \log Z_{T+1} - \log Z_{1} \geq -d\log\frac{1}{\gamma} - \eta \sum_{t=1}^Tf_t(u) - \eta T\gamma,
    \end{align*}
    for any $u\in\calX$ and $\gamma\in [0,1]$. Picking $\gamma = \frac{1}{T}$ and using the fact that $\int_{x\in\calX}p_t(x)f_t(x)dx\geq f_t(x_t)$ and $\int_{x\in\calX}p_{t+1}(x)f_t(x)dx\geq f_t(x_{t+1})$ due to convexity, we know that
\begin{align}\label{eqn:reg-cont-main}
    \RegAlt \leq \frac{d\log T}{\eta} + \frac{1}{\eta}\sum_{t=1}^T\left(\KL(p_t,p_{t+1})-\KL(p_{t+1},p_t)\right).
\end{align}
Next, we bound $\KL(p_t,p_{t+1})-\KL(p_{t+1},p_t)$. Define $H(F) = \log\int_{x\in\calX}\exp(-\eta F(x))dx$.
By definition of $\KL(p,q)$, we know that
\begin{align}\label{eqn:KL}
    \KL(p_t,p_{t+1}) = \int_{x\in\calX}p_t(x)\log\frac{p_t(x)}{p_{t+1}(x)}dx = H(F_{t+1}) - H(F_{t}) + \eta\cdot \E_{x\sim p_t}\left[f_t(x)\right].
\end{align}
Define $p_{t,s}$ to be the distribution where $p_{t,s}(x)\propto \exp(-\eta ((1-s) F_{t-1}(x) +sF_{t}(x)))$ and $Z_{t,s}=\int_{x\in\calX}\exp(-\eta ((1-s)F_{t-1}(x) +sF_{t}(x)))dx$. By definition, we have $p_{t,0}=p_t$, $p_{t,1}=p_{t+1}$, $Z_{t,0}=Z_t$ and $Z_{t,1}=Z_{t+1}$. Direct calculation shows that
\begin{align}
    \nabla_s\log Z_{t,s} &= \frac{\nabla_s Z_{t,s}}{Z_{t,s}} = \frac{1}{Z_{t,s}}\int_{x\in\calX}-\eta f_t(x)\exp(-\eta((1-s)F_{t-1}(x)+sF_t(x)))dx \nonumber \\
    &= -\E_{x\sim p_{t,s}}[\eta f_t(x)], \label{eqn:mean_exp}\\
    \nabla_s^2\log Z_{t,s} &= \frac{\int_{x\in\calX}\eta^2f_t(x)^2\exp(-\eta((1-s)F_{t-1}(x)+sF_t(x)))dx}{Z_{t,s}} \nonumber \\
    &\qquad - \left(\frac{\int_{x\in\calX}\eta f_t(x)\exp(-\eta((1-s)F_{t-1}(x)+sF_t(x)))dx}{Z_{t,s}}\right)^2 \nonumber\\
    &=\Var_{x\sim p_{t,s}}[\eta f_t(x)]. \label{eqn:var_exp}
\end{align}

According to Fundamental theorem of calculus, we know that
\begin{align*}
    \log Z_{t,1} &= \log Z_{t,0} + \int_0^1\nabla_s \log Z_{t,s}ds \\
    &=\log Z_{t,0} + [\nabla_s \log Z_{t,s}]_{s=0} +\int_0^1\int_0^\alpha \nabla_s^2 \log Z_{t,s}dsd\alpha \\
    &= \log Z_{t,0} + [\nabla_s \log Z_{t,s}]_{s=0} +\int_0^1\left(\int_s^1d\alpha\right) \nabla_s^2 \log Z_{t,s}ds \\
    &= \log Z_{t,0} + [\nabla_s \log Z_{t,s}]_{s=0} +\int_0^1(1-s)\nabla_s^2 \log Z_{t,s}ds.
\end{align*}

Then, based on \pref{eqn:KL}, we can obtain that
\begin{align*}
     \KL(p_t,p_{t+1}) &= \log Z_{t,1} - \log Z_{t,0} - \left[\nabla_s \log Z_{t,s}\right]_{s=0} \\
     &= \int_0^1 (1-s)[\nabla_{s}^2\log Z_{t,s}]ds \\
     &= \int_0^1 (1-s)\Var_{x\sim p_{t,s}}[\eta f_t(x)]ds,
\end{align*}
where the third equality is due to \pref{eqn:var_exp}. Similarly, we can obtain that
\begin{align*}
     \KL(p_{t+1},p_{t}) &= \log Z_{t,0} - \log Z_{t,1} - \left[\nabla_s \log Z_{t,s}\right]_{s=1} \\
     &= \int_0^1 (1-s)\Var_{x\sim p_{t,1-s}}[-\eta f_t(x)]ds \\
     &= \int_0^1 s'\Var_{x\sim p_{t,s'}}[\eta f_t(x)]ds', 
\end{align*}
where the last equality is by a variable replacement $s'=1-s$ and $\Var[x]=\Var[-x]$.

Combining the above two equalities, we know that
\begin{align}\label{eqn:KL-1}
    \KL(p_t,p_{t+1}) - \KL(p_{t+1},p_t) = \int_0^1(1-2s)\Var_{x\sim p_{t,s}}[\eta f_t(x)]ds.
\end{align}

To further analyze $\int_0^1(1-2s)\Var_{x\sim p_{t,s}}[\eta f_t(x)]ds$, let $v = s-\frac{1}{2}$ and $p_{t,v}\propto \exp(-(\frac{1}{2}-v)\eta F_t(x)-(\frac{1}{2}+v)\eta F_{t+1}(x))$ with an abuse of notation. Then, we have
\begin{align}
    &\frac{1}{2}\int_0^1(1-2s)\Var_{x\sim p_{t,s}}[\eta f_t(x)]ds \nonumber\\
    &= -\int_{-\frac{1}{2}}^{\frac{1}{2}}v\cdot\Var_{x\sim p_{t,v}}[\eta f_t(x)]dv \nonumber\\
    &= -\int_{0}^{\frac{1}{2}}v\cdot\Var_{x\sim p_{t,v}}[\eta f_t(x)]dv -\int_{-\frac{1}{2}}^{0}v\cdot\Var_{x\sim p_{t,v}}[\eta f_t(x)]dv \nonumber \\
    &= \int_0^{\frac{1}{2}}v\left(\Var_{x\sim p_{t,-v}}[\eta f_t(x)] - \Var_{x\sim p_{t,v}}[\eta f_t(x)]\right)dv. \label{eqn:KL-2}
\end{align}

We then show how to bound $\Var_{x\sim p_{t,-v}}[\eta f_t(x)] - \Var_{x\sim p_{t,v}}[\eta f_t(x)]$. For notational convenience, let $p_{t,-v}=q_1$ and $p_{t,v}=q_2$.

Direct calculation shows that
\begin{align}
    &\Var_{x\sim q_1}[\eta f_t(x)] - \Var_{x\sim q_2}[\eta f_t(x)] \nonumber\\
    &=\eta^2\rbr{\E_{q_1}[f_t(x)^2] - \E_{q_2}[f_t(x)^2]} - \eta^2(\E_{q_1}[f_t(x)] + \E_{q_2}[f_t(x)])(\E_{q_1}[f_t(x)] - \E_{q_2}[f_t(x)]) \nonumber\\
    &\leq \eta^2\max_{x\in\calX}f_t^2(x) \|q_1-q_2\|_{TV} + 2\eta^2\max_{x\in\calX}f_t^2(x)\|q_1-q_2\|_{TV}\nonumber\\
    &\leq 3\eta^2 \|q_1-q_2\|_{TV}, \label{eqn:KL-3}
\end{align}
where we use $f_t(x)\in[-1,1]$. To further bound $\|q_1-q_2\|_{TV}$, we define $G(x)=-\frac{1}{2}(F_t(x)+F_{t+1}(x))$ for notational convenience. By definition of $q_1$ and $q_2$, we know that for any $x\in\calX$
\begin{align*}
    \frac{q_1(x)}{q_2(x)} &= \frac{\int_{x'}\exp(G(x')+\eta vf_t(x'))dx'}{\int_{x'}\exp(G(x')-\eta vf_t(x'))dx'} \cdot \frac{\exp(G(x)-\eta vf_t(x))}{\exp(G(x)+\eta vf_t(x))} \\
    &\leq \frac{\int_{x'}\exp(G(x')-\eta vf_t(x'))dx'}{\int_{x'}\exp(G(x')-\eta vf_t(x'))dx'} \cdot \frac{\exp(G(x)+vf_t(x))}{\exp(G(x)+vf_t(x))}\exp(\eta) \\
    &= \exp(\eta),
\end{align*}
where the inequality is because $v\leq \frac{1}{2}$ and $f_t(x)\in[-1,1]$.
Similarly, we can also show that
\begin{align*}
    \frac{q_1(x)}{q_2(x)} &= \frac{\int_{x'}\exp(G(x')+\eta vf_t(x'))dx'}{\int_{x'}\exp(G(x')-\eta vf_t(x'))dx'} \cdot \frac{\exp(G(x)-\eta vf_t(x))}{\exp(G(x)+\eta vf_t(x))} \\
    &\geq \frac{\int_{x'}\exp(G(x')-\eta vf_t(x'))dx'}{\int_{x'}\exp(G(x')-\eta vf_t(x'))dx'} \cdot \frac{\exp(G(x)+vf_t(x))}{\exp(G(x)+vf_t(x))}\exp(-\eta) \\
    &= \exp(-\eta).
\end{align*}
Therefore, we know that $\|q_1-q_2\|_{TV}\leq \exp(\eta) - 1\leq 2\eta $ since $\eta\leq 1$. Combining \pref{eqn:KL-1}, \pref{eqn:KL-2}, and \pref{eqn:KL-3}, we conclude that
\begin{align}\label{eqn:KL-diff-cont}
    \KL(p_t,p_{t+1}) - \KL(p_{t+1},p_{t}) = \order(\eta^3). 
\end{align}
Combining \pref{eqn:reg-cont-main} and \pref{eqn:KL-diff-cont} and picking $\eta$ optimally finishes the proof.

\end{proof}
