\section{Judgements}
\centering
\judgement{Expression Evaluation}{$V\vDash e \rightsquigarrow v$}
    \begin{mathpar}
    \inferrule*[Right=\rulename{V-Ev-Int}]
    {~}
    {V\vDash \kwd{n}_\text{i32} \rightsquigarrow \kwd{n}_\text{i32}}
    \and
    \inferrule*[Right=\rulename{V-Ev-Op}]
    {V\vDash e_1 \rightsquigarrow \kwd{n}_1
    \\ V\vDash e_2 \rightsquigarrow \kwd{n}_2}
    {V\vDash e_1~\kwd{op}~e_2 \rightsquigarrow \kwd{n}_1~\kwd{op}~\kwd{n}_2}
    \\
    \inferrule*[Right=\rulename{V-Ev-True}]
    {~}
    {V\vDash \kwd{true} \rightsquigarrow \kwd{true}}
    \and
    \inferrule*[Right=\rulename{V-Ev-False}]
    {~}
    {V\vDash \kwd{false} \rightsquigarrow \kwd{false}}
    \\
    \inferrule*[Right=\rulename{V-Ev-Nil}]
    {~}
    {V\vDash \kwd{nil} \rightsquigarrow \kwd{nil}}
    \and
    \inferrule*[Right=\rulename{V-Ev-Box}]
    {V\vDash e \rightsquigarrow v}
    {V\vDash \kwd{box}(e) \rightsquigarrow \kwd{box}(v)}
    \\
    \inferrule*[Right=\rulename{V-Ev-Copy}]
    {V\vDash p \rightsquigarrow v}
    {V\vDash \kwd{copy}~p \rightsquigarrow v}
    \and
    \inferrule*[Right=\rulename{V-Ev-Move}]
    {V\vDash p \rightsquigarrow v}
    {V\vDash \kwd{move}~p \rightsquigarrow v}
    \and
    \inferrule*[Right=\rulename{V-Ev-Borrow}]
    {V\vDash p \rightsquigarrow v}
    {V\vDash \&^{\kwd{s}/\kwd{m}/\kwd{2}} p \rightsquigarrow \&(p, v)}
\end{mathpar}

\centering
\judgement{Statement Execution}{$V\vDash e \rightsquigarrow^\delta \Dashv V'$}
\begin{mathpar}
    \inferrule*[Right=\rulename{V-Ex-Ret}]
    {~}
    {V\vDash \kwd{return} \rightsquigarrow^0 \Dashv V}
    \and
    \inferrule*[Right=\rulename{V-Ex-Seq}]
    {V\vDash s_1\rightsquigarrow^{\delta_1}\Dashv V'
    \\ V'\vDash s_2\rightsquigarrow^{\delta_2}\Dashv V''}
    {V\vDash s_1; s_2\rightsquigarrow^{\delta_1+\delta_2}\Dashv V''}
    \\
    \inferrule*[Right=\rulename{V-Ex-Tick}]
    {~}
    {V\vDash \kwd{tick}(\delta)\rightsquigarrow^\delta \Dashv V}
    \and
    \inferrule*[Right=\rulename{V-Ex-Drop}]
    {~}
    {V\vDash \kwd{drop}~p\rightsquigarrow^0\Dashv V}
    \\
    \inferrule*[Right=\rulename{V-Ex-Assign}]
    {V\vDash e \rightsquigarrow v'
    \\ \VWt{V}{p}{v'}{V'}}
    {V\vDash p\from e\rightsquigarrow^0 \Dashv V'}
    \\
    \inferrule*[Right=\rulename{V-Ex-Cons}]
    {V\vDash e_1 \rightsquigarrow v_1
    \\ V\vDash e_2 \rightsquigarrow v_2
    \\ \VWt{V}{p}{\kwd{cons}(v_1, v_2)}{V'} }
    {V\vDash p\from \kwd{cons}(e_1, e_2)\rightsquigarrow^0 \Dashv V'}
    \\
    \inferrule*[Right=\rulename{V-Ex-IfT}]
    {V\vDash p\rightsquigarrow \kwd{true}
    \\ V\vDash s_1\rightsquigarrow^\delta \Dashv V'}
    {V\vDash \kwd{if}~ p ~\kwd{then}~ s_1 ~\kwd{else}~ s_2 ~\kwd{end} \rightsquigarrow^\delta \Dashv V'}
    \and
    \inferrule*[Right=\rulename{V-Ex-IfF}]
    {V\vDash p\rightsquigarrow \kwd{false}
    \\ V\vDash s_2\rightsquigarrow^\delta \Dashv V'}
    {V\vDash \kwd{if}~ p ~\kwd{then}~ s_1 ~\kwd{else}~ s_2 ~\kwd{end} \rightsquigarrow^\delta \Dashv V'}
    \\
    \inferrule*[Right=\rulename{V-Ex-Mat-Nil}]
    {V\vDash p\rightsquigarrow \kwd{nil}
    \\ V\vDash s_1\rightsquigarrow^\delta \Dashv V'}
    {V\vDash \kwd{match}~ p ~ \{\kwd{nil}\mapsto s_1, \kwd{cons}(x_\text{hd}, x_\text{tl})\mapsto s_2\} \rightsquigarrow^\delta \Dashv V'}

    \inferrule*[Right=\rulename{V-Ex-Mat-Cons}]
    {V\vDash p\rightsquigarrow \kwd{cons}(hd, tl)
    \\ \VWt{V}{p}{\bot}{V_1}
    \\ \VWt{V_1}{x_\text{hd}}{hd}{V_2}
    \\ \VWt{V_2}{x_\text{tl}}{tl}{V_\text{b}}
    \\\\ V_\text{b}\vDash s_2\rightsquigarrow^\delta \Dashv V'_\text{b}
    \\ V'_\text{b}\vDash x_\text{hd}\rightsquigarrow hd'
    \\ V'_\text{b}\vDash x_\text{tl}\rightsquigarrow tl'
    \\\\ \VWt{V'_\text{b}}{x_\text{hd}}{\bot}{V'_1}
    \\ \VWt{V'_1}{x_\text{tl}}{\bot}{V'_2}
    \\ \VWt{V'_2}{p}{\kwd{cons}(hd', tl')}{V'} 
    }
    {V\vDash \kwd{match}~ p ~ \{\kwd{nil}\mapsto s_1, \kwd{cons}(x_\text{hd}, x_\text{tl})\mapsto s_2\} \rightsquigarrow^\delta \Dashv V'}
    \\
    
    \inferrule*[Right=\rulename{V-Ex-App}]
    {\kwd{fn}~ f ~(\vec{x}_\text{param}:\vec{t}_\text{param}, \vec{x}_\text{local}:\vec{t}_\text{local}, x_\text{ret}:t_\text{ret}) \{~ s ~\}
    \\ V\vDash \vec{e}\rightsquigarrow \vec{v}
    \\\\ \VWt{V}{\vec{x}_\text{param}}{\vec{v}}{V_1}
    \\ \VWt{V_1}{\vec{x}_\text{local}}{\bot}{V_2}
    \\ \VWt{V_2}{x_\text{ret}}{\bot}{V_\text{b}}
    \\\\ V_\text{b}\vDash s\rightsquigarrow^\delta \Dashv V'_\text{b}
    \\ V'_\text{b}\vDash x_\text{ret} \rightsquigarrow v_\text{ret}
    \\\\ \VWt{V'_\text{b}}{\vec{x}_\text{param}}{\bot}{V'_1}
    \\ \VWt{V'_1}{\vec{x}_\text{local}}{\bot}{V'_2}
    \\ \VWt{V'_2}{x_\text{ret}}{\bot}{V'_3}
    \\ \VWt{V'_3}{p}{v_\text{ret}}{V'}
    } 
    {V\vDash p\from f(\vec{e})\rightsquigarrow^\delta \Dashv V'}
\end{mathpar}

\centering
\judgement{Enrich}{$\textit{enrich}~ t ~\textit{as}~ \tau$}
\begin{mathpar}
    \inferrule*[Right=\rulename{Enrich-Int}]
    {~}
    {\textit{enrich}~ \kwd{i32} ~\textit{as}~\kwd{i32}}
    \and
    \inferrule*[Right=\rulename{Enrich-Bool}]
    {~}
    {\textit{enrich}~ \kwd{bool} ~\textit{as}~ \kwd{bool}}
    \\

    \inferrule*[Right=\rulename{Enrich-List}]
    {\alpha~\text{fresh}}
    {\textit{enrich}~ \kwd{list} ~\textit{as}~  \kwd{list}(\alpha)}
    \and
    \inferrule*[Right=\rulename{Enrich-Box}]
    {\alpha~\text{fresh}}
    {\textit{enrich}~ \kwd{box}(\kwd{list}) ~\textit{as}~ \kwd{box}(\kwd{list}(\alpha))}
    \\
    
    \inferrule*[Right=\rulename{Enrich-Shared}]
    {\textit{enrich}~ t ~\textit{as}~ \tau}
    {\textit{enrich}~ \&^\kwd{s}(t) ~\textit{as}~ \&^\kwd{s}(\tau)}
    \\
    \inferrule*[Right=\rulename{Enrich-Mutable}]
    {\textit{enrich}~ t ~\textit{as}~ \tau_\text{c}
    \\ \textit{enrich}~ t ~\textit{as}~ \tau_\text{p}
    }
    {\textit{enrich}~ \&^\kwd{m}(t) ~\textit{as}~ \&^\kwd{m}(\tau_\text{c}, \tau_\text{p})}
\end{mathpar}

\centering
\judgement{Sharing}{$\textit{share}~ \tau ~\textit{as}~\tau_1, \tau_2$}
\begin{mathpar}
    \inferrule*[Right=\rulename{Share-Int}]
    {~}
    {\textit{share}~ \kwd{i32} ~\textit{as}~\kwd{i32}, \kwd{i32}}
    \and
    \inferrule*[Right=\rulename{Share-Bool}]
    {~}
    {\textit{share}~ \kwd{bool} ~\textit{as}~\kwd{bool}, \kwd{bool}}
    \\
    \inferrule*[Right=\rulename{Share-List}]
    {\alpha_1, \alpha_2 ~\text{fresh}
    \\\alpha = \alpha_1 + \alpha_2}
    {\textit{share}~ \kwd{list}(\alpha) ~\textit{as}~\kwd{list}(\alpha_1), \kwd{list}(\alpha_2)}
    \\
    \inferrule*[Right=\rulename{Share-Box}]
    {\textit{share}~ \tau ~\textit{as}~\tau_1, \tau_2}
    {\textit{share}~ \kwd{box}(\tau) ~\textit{as}~\kwd{box}(\tau_1), \kwd{box}(\tau_2)}
    \\
    \inferrule*[Right=\rulename{Share-Shared}]
    {\textit{share}~ \tau ~\textit{as}~\tau_1, \tau_2}
    {\textit{share}~ \&^\kwd{s}(\tau) ~\textit{as}~ \&^\kwd{s}(\tau_1), \&^\kwd{s}(\tau_2)}
\end{mathpar}

\centering
\judgement{Prophesying}{$\textit{prophesy}~ \tau_\text{c} ~\textit{as}~\tau_\text{p}$}
\begin{mathpar}
    \inferrule*[Right=\rulename{Prophesy-Int}]
    {~}
    {\textit{prophesy}~ \kwd{i32} ~\textit{as}~ \kwd{i32}}
    \and
    \inferrule*[Right=\rulename{Prophesy-Bool}]
    {~}
    {\textit{prophesy}~ \kwd{bool} ~\textit{as}~ \kwd{bool}}
    \\
    \inferrule*[Right=\rulename{Prophesy-List}]
    {\alpha_\text{p}~\text{fresh}}
    {\textit{prophesy}~ \kwd{list}(\alpha) ~\textit{as}~ \kwd{list}(\alpha_\text{p})}
    \\
    \inferrule*[Right=\rulename{Prophesy-Box}]
    {\textit{prophesy}~ \tau ~\textit{as}~ \tau_\text{p} }
    {\textit{prophesy}~ \kwd{box}(\tau) ~\textit{as}~ \kwd{box}(\tau_\text{p})}
    \\
    \inferrule*[Right=\rulename{Prophesy-Shared}]
    {\textit{prophesy}~ \tau ~\textit{as}~ \tau_\text{p}}
    {\textit{prophesy}~ \&^\kwd{s}(\tau) ~\textit{as}~ \&^\kwd{s}(\tau_\text{p})}
    \\
    \inferrule*[Right=\rulename{Prophesy-Mutable}]
    {\textit{prophesy}~ \tau_\text{c} ~\textit{as}~ \tau_\text{cp}
    \\ \textit{prophesy}~ \tau_\text{p} ~\textit{as}~ \tau_\text{pp}
    }
    {\textit{prophesy}~ \&^\kwd{m}(\tau_\text{c}, \tau_\text{p}) ~\textit{as}~ \&^\kwd{m}(\tau_\text{cp}, \tau_\text{pp})}
\end{mathpar}

\centering
\judgement{Meet/Join}{$\tau_1\cap\tau_2 / \tau_1\cup\tau_2$}
\begin{mathpar}    
    \inferrule*[Right=Meet-Int]
    {~}
    {\kwd{i32}\cap\kwd{i32}=\kwd{i32}}
    \and
    \inferrule*[Right=Join-Int]
    {~}
    {\kwd{i32}\cup\kwd{i32}=\kwd{i32}}
    \\
    \inferrule*[Right=Meet-Bool]
    {~}
    {\kwd{bool}\cap\kwd{bool}=\kwd{bool}}
    \and
    \inferrule*[Right=Join-Bool]
    {~}
    {\kwd{bool}\cup\kwd{bool}=\kwd{bool}}
    \\
    
    \inferrule*[Right=Meet-List]
    {\min(\alpha_1, \alpha_2)=\alpha}
    {\kwd{list}(\alpha_1)\cap\kwd{list}(\alpha_2)=\kwd{list}(\alpha)}
    \and
    \inferrule*[Right=Join-List]
    {\max(\alpha_1, \alpha_2)=\alpha}
    {\kwd{list}(\alpha_1)\cup\kwd{list}(\alpha_2)=\kwd{list}(\alpha)}
    \\
    
    \inferrule*[Right=Meet-Box]
    {\tau_1 \cap \tau_2=\tau}
    {\kwd{box}(\tau_1)\cap\kwd{box}(\tau_2)=\kwd{box}(\tau)}
    \and
    \inferrule*[Right=Join-Box]
    {\tau_1 \cup \tau_2=\tau}
    {\kwd{box}(\tau_1)\cup\kwd{box}(\tau_2)=\kwd{box}(\tau)}
    \\
    
    \inferrule*[Right=Meet-Shared]
    {\tau_1 \cap \tau_2=\tau}
    {\&^\kwd{s}(\tau_1)\cap\&^\kwd{s}(\tau_2)=\&^\kwd{s}(\tau)}
    \and
    \inferrule*[Right=Join-Shared]
    {\tau_1 \cup \tau_2=\tau}
    {\&^\kwd{s}(\tau_1)\cup\&^\kwd{s}(\tau_2)=\&^\kwd{s}(\tau)}
    \\

    \inferrule*[Right=Meet-Mutable]
    {\tau_{\text{c}, 1} \cap \tau_{\text{c}, 2}=\tau_\text{c}
    \\ \tau_{\text{p}, 1} \cup \tau_{\text{p}, 2}=\tau_\text{p}
    \\ \vdash \&^\kwd{m}(\tau_{\text{c}, 1}, \tau_{\text{p}, 1})
    \\ \vdash \&^\kwd{m}(\tau_{\text{c}, 2}, \tau_{\text{p}, 2})
    }
    {\&^\kwd{m}(\tau_{\text{c}, 1}, \tau_{\text{p}, 1})\cap\&^\kwd{m}(\tau_{\text{c}, 2}, \tau_{\text{p}, 2})=\&^\kwd{m}(\tau_\text{c}, \tau_\text{p})}
    \\
    \inferrule*[Right=Join-Mutable]
    {\tau_{\text{c}, 1} \cup \tau_{\text{c}, 2}=\tau_\text{c}
    \\ \tau_{\text{p}, 1} \cap \tau_{\text{p}, 2}=\tau_\text{p}
    \\ \vdash \&^\kwd{m}(\tau_{\text{c}, 1}, \tau_{\text{p}, 1})
    \\ \vdash \&^\kwd{m}(\tau_{\text{c}, 2}, \tau_{\text{p}, 2})
    }
    {\&^\kwd{m}(\tau_{\text{c}, 1}, \tau_{\text{p}, 1})\cup\&^\kwd{m}(\tau_{\text{c}, 2}, \tau_{\text{p}, 2})=\&^\kwd{m}(\tau_\text{c}, \tau_\text{p})}
\end{mathpar}

\centering
\judgement{Typing Expression}{$\Gamma\vdash e \hookrightarrow \tau\dashv\Gamma'$}
\begin{mathpar}
    \inferrule*[Right=\rulename{$\Gamma$-Ev-Int}]
    {~}
    {\Gamma\vdash \kwd{n}_\text{i32} \hookrightarrow \kwd{i32}\dashv\Gamma}
    \and
    \inferrule*[Right=\rulename{$\Gamma$-Ev-Op}]
    {\Gamma\vdash e_1\hookrightarrow \kwd{i32}\dashv\Gamma
    \\ \Gamma\vdash e_2\hookrightarrow \kwd{i32}\dashv\Gamma}
    {\Gamma\vdash e_1~\kwd{op}~e_2 \hookrightarrow \kwd{i32}\dashv\Gamma}
    \\
    
    \inferrule*[Right=\rulename{$\Gamma$-Ev-True}]
    {~}
    {\Gamma\vdash \kwd{true} \hookrightarrow \kwd{bool}\dashv\Gamma}
    \and
    \inferrule*[Right=\rulename{$\Gamma$-Ev-False}]
    {~}
    {\Gamma\vdash \kwd{false} \hookrightarrow \kwd{bool}\dashv\Gamma}
    \\
    \inferrule*[Right=\rulename{$\Gamma$-Ev-Copy}]
    {\Gamma\vdash p \hookrightarrow \tau
    \\ \tau = \kwd{i32} ~\text{or}~ \tau = \kwd{bool} }
    {\Gamma\vdash \kwd{copy}~p \hookrightarrow \tau\dashv\Gamma}
    \and
    \inferrule*[Right=\rulename{$\Gamma$-Ev-Box}]
    {\Gamma\vdash e \hookrightarrow \tau\vdash\Gamma'}
    {\Gamma\vdash \kwd{box}(e) \hookrightarrow \kwd{box}(\tau)\vdash\Gamma'}
    \\

    \inferrule*[Right=\rulename{$\Gamma$-Ev-Nil}]
    {\alpha ~\text{fresh}}
    {\Gamma\vdash \kwd{nil} \hookrightarrow \kwd{list}(\alpha)\vdash\Gamma}
    \and
    \inferrule*[Right=\rulename{$\Gamma$-Ev-Move}]
    {\Gamma\vdash p \hookrightarrow \tau
    \\ \GWt{\Gamma}{p}{\bot}{\Gamma'}}
    {\Gamma\vdash \kwd{move}~p \hookrightarrow \tau\dashv\Gamma'}
    \\
    
    \inferrule*[Right=\rulename{$\Gamma$-Ev-Shared}]
    {\Gamma\vdash p \hookrightarrow \tau
    \\ \textit{share}~ \tau ~\textit{as}~\tau_1, \tau_2
    \\ \GWt{\Gamma}{p}{\tau_1}{\Gamma'}
    }
    {\Gamma\vdash \&^\kwd{s}~p \hookrightarrow \&^\kwd{s}(\tau_2)\dashv\Gamma'}
    \\
    
    \inferrule*[Right=\rulename{$\Gamma$-Ev-Mutable}]
    {\Gamma\vdash p \hookrightarrow \tau
    \\ \textit{prophesy}~ \tau ~\textit{as}~ \tau_\text{p} 
    \\ \GWt{\Gamma}{p}{\tau_\text{p}}{\Gamma'}
    }
    {\Gamma\vdash \&^\kwd{m}~p \hookrightarrow \&^\kwd{m}(\tau, \tau_\text{p})\dashv\Gamma'}
\end{mathpar}

\centering
\judgement{Typing Statements}{$\Gamma\vdash s \hookrightarrow^\delta \dashv\Gamma'$}
\begin{mathpar}
    \inferrule*[Right=\rulename{$\Gamma$-Ex-Ret}]
    {~}
    {\Gamma\vdash \kwd{return} \hookrightarrow^0\vdash\Gamma}
    \and
    \inferrule*[Right=\rulename{$\Gamma$-Ex-Seq}]
    {\Gamma_1\vdash s_1\hookrightarrow^{\delta_1}\dashv\Gamma_2
    \\ \Gamma_2\vdash s_2\hookrightarrow^{\delta_2}\dashv\Gamma_3}
    {\Gamma_1\vdash s_1; s_2\hookrightarrow^{\delta_1+\delta_2}\dashv\Gamma_3}
    \\
    
    \inferrule*[Right=\rulename{$\Gamma$-Ex-Tick}]
    {~}
    {\Gamma\vdash\kwd{tick}(\delta)\hookrightarrow^\delta\vdash\Gamma}
    \and
    \inferrule*[Right=\rulename{$\Gamma$-Ex-Drop}]
    {\Gamma\vdash p\hookrightarrow \tau
    \\ \vdash \tau
    \\ \GWt{\Gamma}{p}{\bot}{\Gamma'}
    }
    {\Gamma\vdash \kwd{drop}~p \hookrightarrow^0\dashv \Gamma'}
    \\

    \inferrule*[Right=\rulename{$\Gamma$-Ex-Assign}]
    {\Gamma\vdash e\hookrightarrow \tau'\dashv\Gamma_1
    \\ \Gamma_1\vdash p \hookrightarrow \tau
    \\ \vdash \tau
    \\ \GWt{\Gamma_1}{p}{\tau'}{\Gamma'}}
    {\Gamma\vdash p\from e \hookrightarrow^0\dashv\Gamma'}
    \\

    \inferrule*[Right=\rulename{$\Gamma$-Ex-Cons}]
    {\Gamma\vdash e_1\hookrightarrow \kwd{i32} \dashv \Gamma_1
    \\ \Gamma_1\vdash e_2\hookrightarrow \kwd{box}(\kwd{list}(\alpha'))\dashv\Gamma_2
    \\ \GWt{\Gamma_2}{p}{\kwd{list}(\alpha')}{\Gamma'}}
    {\Gamma\vdash p\from \kwd{cons}(e_1, e_2)\hookrightarrow^{\alpha'}\dashv\Gamma'}
    \\

    \inferrule*[Right=\rulename{$\Gamma$-Ex-If}]
    {\Gamma\vdash p\hookrightarrow \kwd{bool}
    \\ \Gamma\vdash s_1\hookrightarrow^{\delta_1}\dashv\Gamma_1
    \\ \Gamma\vdash s_2\hookrightarrow^{\delta_2}\dashv\Gamma_2
    \\ \max(\delta_1, \delta_2)=\delta
    \\ \Gamma_1\sqcap\Gamma_2=\Gamma' }
    {\Gamma\vdash \kwd{if}~ p ~\kwd{then}~ s_1 ~\kwd{else}~ s_2 ~\kwd{end} \hookrightarrow^\delta \dashv\Gamma'}
    \\
    \inferrule*[Right=\rulename{$\Gamma$-Ex-Mat}]
    {\Gamma\vdash p\hookrightarrow \kwd{list}(\alpha)
    \\ \Gamma\vdash s_1\hookrightarrow^{\delta_1}\dashv\Gamma_1
    \\\\ \GWt{\Gamma}{p}{\bot}{\Gamma_{\text{b}, 1}}
    \\ \GWt{\Gamma_{\text{b}, 1}}{x_\text{hd}}{\kwd{i32}}{\Gamma_{\text{b}, 2}}
    \\ \GWt{\Gamma_{\text{b}, 2}}{x_\text{tl}}{\kwd{box}(\kwd{list}(\alpha))}{\Gamma_\text{b}}
    \\ \Gamma_\text{b}\vdash s_2\hookrightarrow^{\delta_2}\dashv\Gamma'_\text{b}
    \\\\ \Gamma'_\text{b}\vdash x_\text{tl}\hookrightarrow \kwd{list}(\beta)
    \\ \GWt{\Gamma'_\text{b}}{x_\text{hd}}{\bot}{\Gamma'_{\text{b}, 1}}
    \\ \GWt{\Gamma'_{\text{b}, 1}}{x_\text{tl}}{\bot}{\Gamma'_{\text{b}, 2}}
    \\ \GWt{\Gamma'_{\text{b}, 2}}{p}{\kwd{list}(\beta)}{\Gamma_2}
    \\\\ \max(\delta_1, \delta_2-(\alpha-\beta))=\delta
    \\ \Gamma_1\sqcap\Gamma_2=\Gamma'}
    {\Gamma\vdash \kwd{match}~ p ~ \{\kwd{nil}\mapsto s_1, \kwd{cons}(x_\text{hd}, x_\text{tl})\mapsto s_2\} \hookrightarrow^\delta \dashv\Gamma'}
    \\

    \inferrule*[Right=\rulename{$\Gamma$-Ex-App}]
    {\text{fn}~ f ~(\vec{x}_\text{param}:\vec{t}_\text{param}, \vec{x}_\text{local}:\vec{t}_\text{local}, x_\text{ret}:t_\text{ret}) \{~ s ~\}
    \\\\ \vdash f \Leftarrow (\Gamma_f, \delta_f)
    \\ \Gamma_f\vdash x_\text{ret} \hookrightarrow \tau_\text{ret}, (\forall x_i\in\vec{x}_\text{param}, i=1, ..., n) \Gamma_f \vdash x_i \hookrightarrow \tau_{\text{param}, i}
    \\\\ \Gamma_0=\Gamma, (\forall e_i\in \vec{e}, i=1, ..., n) \Gamma_{i-1}\vdash e_i\hookrightarrow\tau_{\text{arg}, i}\dashv\Gamma_i
    \\ (\forall i=1,..,n)~ \tau_{\text{param}, i} = \tau_{\text{arg}, i}
    \\ \Gamma_n \vdash p \hookrightarrow \tau
    \\ \vdash \tau
    \\ \GWt{\Gamma_n}{p}{\tau_\text{ret}}{\Gamma'}
    }
    {\Gamma\vdash p\from f(\vec{e})\hookrightarrow^{\delta_f}\dashv\Gamma'}
\end{mathpar}

\centering
\judgement{Function Analysis}{$\vdash f \Leftarrow (\Gamma_f, \delta_f)$}
\begin{mathpar}
    \inferrule
    {\text{fn}~ f ~(\vec{x}_\text{param}:\vec{t}_\text{param}, \vec{x}_\text{local}:\vec{t}_\text{local}, x_\text{ret}:t_\text{ret}) \{~ s ~\}
    \\  \vdash f \Rightarrow (\Gamma_f, \delta_f)
    \\ \Gamma_f\vdash s\hookrightarrow^\delta\dashv\Gamma'_f
    \\\\ \forall x \in \textbf{dom}(\Gamma'_f), \vdash \Gamma'_f(x)
    \\ \Gamma'_f \vdash x_\text{ret} \hookrightarrow \tau'_\text{ret}
    \\ \Gamma_f \vdash x_\text{ret} \hookrightarrow \tau_\text{ret}
    \\ \tau'_\text{ret} = \tau_\text{ret}
    \\ \delta = \delta_f}
    {\vdash f \Leftarrow (\Gamma_f, \delta_f)}
\end{mathpar}
    

\centering
\judgement{Potential Function}{$\phi(v:\tau)$}
\begin{mathpar}
    \inferrule*[Right=$\phi$-Bot]
    {~}
    {\phi(\_:\bot)=0}
    \and
    \inferrule*[Right=$\phi$-Int]
    {~}
    {\phi(\kwd{n}_\text{i32}:\kwd{i32})=0}
    \\
    \inferrule*[Right=$\phi$-True]
    {~}
    {\phi(\kwd{true}:\kwd{bool})=0}
    \and
    \inferrule*[Right=$\phi$-False]
    {~}
    {\phi(\kwd{false}:\kwd{bool})=0}
    \\
    
    \inferrule*[Right=$\phi$-Nil]
    {~}
    {\phi(\kwd{nil}:\kwd{list}(\alpha))=0}
    \\
    \inferrule*[Right=$\phi$-Cons]
    {~}
    {\phi(\kwd{cons}(\kwd{n}_\text{i32}, \kwd{box}(lv)):\kwd{list}(\alpha))=\alpha+\phi(\kwd{box}(lv):\kwd{box}(\kwd{list}(\alpha)))}
    \\
    \inferrule*[Right=$\phi$-Box]
    {~}
    {\phi(\kwd{box}(lv):\kwd{box}(\kwd{list}(\alpha)))=\phi(lv:\kwd{list}(\alpha))}
    \\
    \inferrule*[Right=$\phi$-Shared]
    {~}
    {\phi(\&(\_, v):\&^\kwd{s}(\tau))=\phi(v:\tau)}
    \\
    \inferrule*[Right=$\phi$-Mutable]
    {~}
    {\phi(\&(\_, v):\&^\kwd{m}(\tau_\text{c}, \tau_\text{p}))=\phi(v:\tau_\text{c})-\phi(v:\tau_\text{p})}
\end{mathpar}