\begin{proof}
\label{prf:thm:SW:BRD}
\emph{Case 1:}
We first consider the case that one of the conditions holds. If $c_i(x_i)$ is $c_0$-convex, then we know that $\SW(\bmx)$ is $c_0$-convex on $x_i$. Similarly, if $f_i(k_i)$ is $c_0$-concave, since $k_i$ depends linearly on $x_i$, we also know that $\SW(\bmx)$ is $c_0$-convex on $x_i$. Also if $\SW(\bmx)$ is $c_0$-concave on $x_i$ for all $i$, then $\SW(\bmx)$ is $c_0$-concave on $\bmx$. 

As a property of $c_0$-concave function $f(\bmx)$ and maximum point $\bmx^*$, we have
\begin{equation}
\label{eq:convex:ineq}
    f(\bmx^*) - f(\bmx) \le \frac{1}{2c_0} \|\nabla f(\bmx)\|^2.
\end{equation}

Define the energy function $E(t) = \SW(\bmx^*) - \SW(\bmx(t))$, then 
\begin{align*}
    \frac{\dd E(t)}{\dd t} =-\sum_\iinn \frac{\partial \SW}{\partial x_i}(\bmx(t)) \frac{\dd x_i}{\dd t}(t)
    = -\sum_\iinn \left(\frac{\partial \SW}{\partial x_i}(\bmx(t))\right)^2 = -\|\nabla \SW(\bmx(t))\|^2.
\end{align*}
Since $\SW(\bmx)$ is $c_0$-concave, by \cref*{eq:convex:ineq} we have $\|\nabla \SW(\bmx(t))\|^2 \ge 2c_0 (\SW(\bmx^*) - \SW(\bmx)) = 2c_0 E(t)$. Therefore, we have
\begin{align*}
    \frac{\dd E(t)}{\dd t} \le -2c_0 E(t).
\end{align*}
By standard differential equation analysis, we have $E(t) \le \exp(-2c_0 t)E(0)$. Taking $c = -2c_0$ completes the proof.

\emph{Case 2:}
Next, we consider the general case. Define $J(t) = t(\SW(\bmx^*) - \SW(\bmx(t))) + \frac{1}{2}\| \bmx^* - \bmx(t) \|^2$. We have
\begin{align*}
    \frac{\dd J(t)}{\dd t} =& \SW(\bmx^*) - \SW(\bmx(t))  - t \langle \frac{\pp \SW}{\pp \bmx}(\bmx(t)), \frac{\dd \bmx}{\dd t}\rangle - \langle \bmx^* - \bmx(t), \frac{\dd \bmx}{\dd t}\rangle
    \\
    =& \SW(\bmx^*) - \SW(\bmx(t)) - \langle \bmx^* - \bmx(t), \nabla \SW(\bmx(t))\rangle - t \|\nabla \SW(\bmx(t))\|^2
\end{align*}
By concavity of $\SW(\bmx)$ we have $\SW(\bmx^*) - \SW(\bmx(t)) \le \langle \bmx^* - \bmx(t), \nabla \SW(\bmx(t))\rangle$, then we have $\frac{\dd J(t)}{\dd t} \le 0$. This indicates that
\begin{align*}
    J(t) \le J(0) = \frac{1}{2}\| \bmx^* - \bmx(0) \|^2
\end{align*}
where $J(t) \ge t(\SW(\bmx^*) - \SW(\bmx(t)))$, and therefore
\begin{align*}
    \SW(\bmx^*) - \SW(\bmx(t)) \le \frac{1}{2t}\| \bmx^* - \bmx(0) \|^2
\end{align*}
Taking $c = \frac{\| \bmx^* - \bmx(0) \|^2}{2}$ completes the proof.

\end{proof}