\begin{proof}
\label{prf:thm:comparative:money}
$\bmx^*(t)$ should satisfy,
\begin{equation}
\label{eq:comparative:money:NE}
    x^*_i(t) = \argmax_{x_i} f_i(x_i + \sum_\jnei w_{ij} x^*_j(t) + \delta_i t) - c_i(x_i),
\end{equation}

By \cref{eq:comparative:money:NE}, we have
\begin{align*}
    c'_i(x^*_i(t)) - f'_i(k^*_i(t) + \delta_i t) = 0,
\end{align*}
which carves out an implicit function
\begin{align*}
    F_i(\bmx^*(t), t) = 0,\quad \forall \iinn
\end{align*}
with $F_i(\bmx,t) = c'_i(x_i) - f'_i(k_i + \delta_i t)$. Take $E_i(t) = F_i(\bmx^*(t), t)$, by implicit function theorem, we have

\begin{equation}
\label{eq:comparative:money:implicit}
    \frac{\dd E_i}{\dd t}(t) = \frac{\pp F_i}{\pp \bmx}(\bmx^*(t),t) \frac{\dd \bmx^*}{\dd t}(t) + \frac{\pp F_i}{\pp t}(\bmx^*(t),t) = 0
\end{equation}

Together \cref{eq:comparative:money:implicit} with all $i$, we have 
\begin{align*}
    \frac{\dd \bmx^*}{\dd t}(t) = - \left( \frac{\pp F}{\pp \bmx} \right)^{-1} \frac{\pp F}{\pp t}(\bmx^*(t),t)
\end{align*}
where $F(\bmx^*(t),t) = (F_1(\bmx^*(t),t), F_2(\bmx^*(t),t), \dots, F_n(\bmx^*(t),t))$, by computation we have,
\begin{align*}
    & \frac{\pp F}{\pp t}(\bmx^*(t),t) = -\diag(\bmf''(\bmk^*(t) + t\bmdd)) \bmdd
    \\
    & \frac{\pp F}{\pp \bmx}(\bmx^*(t),t) = \diag(\bmc''(\bmx^*(t))) - \diag(\bmf''(\bmk^*(t) + t\bmdd))W
\end{align*}

By $\bmu(t) = \bmu(x^*(t);t)$, we derive that,
\begin{align*}
    \bmu'(0) = \frac{\pp \bmu}{\pp t}(\bmx^*;0) + \frac{\pp \bmu}{\pp \bmx}(\bmx^*;0) \frac{\dd \bmx^*}{\dd t}(0)
\end{align*}
where
\begin{align*}
    & \frac{\pp \bmu}{\pp t}(\bmx^*;0) = \diag(\bmf'(\bmk^*)) \bmdd
    \\
    & \frac{\pp \bmu}{\pp \bmx}(\bmx^*;0) = \diag(\bmf'(\bmk^*)) W - \diag(\bmc'(\bmx^*))
    \\
    & \frac{\dd \bmx^*}{\dd t}(0) = \left( \diag(\bmc''(\bmx^*)) - \diag(\bmf''(\bmk^*))W \right)^{-1} \diag(\bmf''(\bmk^*)) \bmdd
\end{align*}

By equilibrium condition, we have
\begin{align*}
    \diag(\bmc'(\bmx^*)) = \diag(\bmf'(\bmk^*))
\end{align*}
and thus
\begin{align*}
    \frac{\pp \bmu}{\pp \bmx}(\bmx^*;0) = \diag(\bmf'(\bmk^*))(W - I)
\end{align*}

Above all,
\begin{align*}
    \bmu'(0) =& \diag(\bmf'(\bmk^*)) \left( \bmdd + (W-I) \left( \diag(\bmc''(\bmx^*)) - \diag(\bmf''(\bmk^*))W \right)^{-1} \diag(\bmf''(\bmk^*)) \bmdd \right)
    \\
    =& \diag(\bmf'(\bmk^*)) \left( I + (W-I) \left( \diag(\bmc''(\bmx^*)) - \diag(\bmf''(\bmk^*))W \right)^{-1} \diag(\bmf''(\bmk^*)) \right) \bmdd
    \\
    =& \diag(\bmf'(\bmk^*)) \left( I + (W-I) \left( \diag(\bmc''(\bmx^*)/\bmf''(\bmk^*)) - W \right)^{-1} \right) \bmdd
    \\
    =& \diag(\bmf'(\bmk^*)) \left( \left( \diag(\bmc''(\bmx^*)/\bmf''(\bmk^*)) - W \right)\cdot \left( \diag(\bmc''(\bmx^*)/\bmf''(\bmk^*)) - W \right)^{-1}
    \right.
    \\
    +& \left. (W-I) \left( \diag(\bmc''(\bmx^*)/\bmf''(\bmk^*)) - W \right)^{-1} \right) \bmdd
    \\
    =& \diag(\bmf'(\bmk^*)) \left( (\diag(\bmc''(\bmx^*)/\bmf''(\bmk^*))-I) \left( \diag(\bmc''(\bmx^*)/\bmf''(\bmk^*)) - W \right)^{-1} \right) \bmdd
    \\
    =& \diag(\bmf'(\bmk^*)) \cdot \diag(\bmc''(\bmx^*) - \bmf''(\bmk^*)) \cdot \left[ \diag(\bmc''(\bmx^*)) - W \diag(\bmf''(\bmk^*)) \right]^{-1} \bmdd
\end{align*}
which completes the proof.

\end{proof}