\subsection{Proof of \cref{thm:revdif}}
\label{app:prf:revdif}
\begin{proof}
By Nelson's relation (\cref{lem:nelson}), $\Q$ is equivalent to the path measure of the following SDE: 
$$\d X_t=X_t\d t+\sqrt{2}\d\Bl_t,~t\in[0,T-\delta];~X_{T-\delta}\sim\piu_\delta.$$

Leveraging Girsanov theorem (\cref{lem:rn_path_measure_contd}), we know that for a.s. $X\sim\Qd$:
\begin{align*}
    &\log\de{\Qd}{\Q}(X)\\
    &=\log\frac{\phi(X_0)}{\piu_\delta(X_{T-\delta})}+(T-\delta)d+\int_0^{T-\delta}\ro{\|s_{T-t_-}(X_{t_-})\|^2\d t+\sqrt{2}\inn{s_{T-t_-}(X_{t_-}),\d B_t}}\\
    &=\log Z+W(X)+\log\de{\pi}{\piu_\delta}(X_{T-\delta}).
\end{align*}
Thus, the equation $\E_{\Qd}\de{\Q}{\Qd}=1$ implies 
$$Z=\E_{\Qd(X)}\e^{-W(X)}\de{\piu_\delta}{\pi}(X_{T-\delta}).$$

Since $\frac{\Zh}{Z}=\de{\Q}{\Qd}(X)\de{\pi}{\piu_\delta}(X_{T-\delta})$, we have
\begin{align*}
    \prob\ro{\abs{\frac{\Zh}{Z}-1}\ge\varepsilon}&=\prob_{X\sim\Qd}\ro{\abs{\de{\Q}{\Qd}(X)\de{\pi}{\piu_\delta}(X_{T-\delta})-1}\ge\varepsilon}\\
    &\le\prob_{X\sim\Qd}\ro{\abs{\de{\Q}{\Qd}(X)-1}\gtrsim\varepsilon}+\prob_{X\sim\Qd}\ro{\abs{\de{\pi}{\piu_\delta}(X_{T-\delta})-1}\gtrsim\varepsilon}.
\end{align*}
The inequality is due to the fact that $|ab-1|\ge\varepsilon$ implies $|a-1|\ge\frac{\varepsilon}{3}$ or $|b-1|\ge\frac{\varepsilon}{3}$ for $\varepsilon\in[0,1]$. It suffices to make both terms above $O(1)$. To bound the first term, we use the similar approach as in the proof of \cref{eq:jar_acc_bound} in \cref{thm:jar_complexity}:
$$\prob_{X\sim\Qd}\ro{\abs{\de{\Q}{\Qd}(X)-1}\gtrsim\varepsilon}=\Qd\ro{\abs{\de{\Q}{\Qd}-1}\gtrsim\varepsilon}\lesssim\frac{\tv(\Q,\Qd)}{\varepsilon}\lesssim\frac{\sqrt{\kl(\Q\|\Qd)}}{\varepsilon}.$$
Hence, it suffices to let $\tv(\Q,\Qd)^2\lesssim\kl(\Q\|\Qd)\lesssim\varepsilon^2$. To bound the second term, we have
\begin{align*}
    \prob_{X\sim\Qd}\ro{\abs{\de{\pi}{\piu_\delta}(X_{T-\delta})-1}\gtrsim\varepsilon}&\le\prob_{X\sim\Q}\ro{\abs{\de{\pi}{\piu_\delta}(X_{T-\delta})-1}\gtrsim\varepsilon}+\tv(\Q,\Qd)\\
    &\le \piu_\delta\ro{\abs{\de{\pi}{\piu_\delta}-1}\gtrsim\varepsilon}+\tv(\Q,\Qd)\\
    &\lesssim\frac{\tv(\piu_\delta,\pi)}{\varepsilon}+\varepsilon.
\end{align*}
Therefore, it suffices to make $\tv(\piu_\delta,\pi)\lesssim\varepsilon$.
\end{proof}