\section{Proofs}\label{appendix:proofs}
\subsection{Missing proofs from Section~\ref{sec:alg}}\label{proof:sec:alg}
\begin{proof}[Proof of Corollary~\ref{thm:alg_bcs}]
We need to compute a lower bound $L$ on  $\frac{\bbE\insq{g'(\vecA_i^T\bx)}}{\normi{{y_i}}_{\psi_2}}$.  Instead of computing $\bbE\insq{g'(\vecA_i^T\bx)}$, we will compute $\bbE\insq{y_iA_{i,j}}$ for  any $j$ in the support of $\bx$. From \eqref{eq:log_expt11} and \eqref{eq:log_expt1_avg11}, we note that $\bbE\insq{y_iA_{i,j}} = \bbE\insq{g'(\vecA_i^T\bx)}$.
Also note that
$\bbE\insq{y_i A_{i,j}}= \bbE\insq{ A_{i,j}\bbE\insq{y_i| A_{i,j}}}$.


For any $\cU\subseteq[1:n]$, we denote $\sum_{l \in \cU}A_{i,l}$ by $A_{i,\cU}$.  For any $A_{i,j} = a$, 
\begin{align*}
\bbP&\inp{y_i = 1|A_{i,j} = a} \\
&= \bbP\inp{A_{i,\cS\setminus\inb{j}}+z_i\geq -a} \\
& = \bbP\inp{\frac{A_{i,\cS\setminus\inb{j}}+z_i}{\sqrt{k-1+\sigma^2}}\geq -\frac{a}{\sqrt{k-1+\sigma^2}}}\\
& = 1-\Phi\inp{-\frac{a}{\sqrt{k-1+\sigma^2}}}
\end{align*} where $\Phi(x) = \frac{1}{2\pi}\int_{-\infty}^{x}e^{-\frac{t^2}{2}}dt$ is the cumulative distribution function of the standard Gaussian distribution. Thus, 
$\bbP\inp{y_i = -1|A_{i,j} = a}  = \Phi\inp{-\frac{a}{\sqrt{k-1+\sigma^2}}}$ and 
$$\bbE\insq{y_i| A_{i,j}=a} = 1-2\Phi\inp{-\frac{a}{\sqrt{k-1+\sigma^2}}}.$$ We are now ready to compute $\bbE\insq{ A_{i,j}\bbE\insq{y_i| A_{i,j}}}$.
\begin{align}
\bbE&\insq{ A_{i,j}\bbE\insq{y_i| A_{i,j}}} \nonumber\\
&= \bbE\insq{ A_{i,j}\inp{1-2\Phi\inp{-\frac{A_{i,j}}{\sqrt{k-1+\sigma^2}}}}}\nonumber\\
&= \bbE\insq{ A_{i,j}}-2\bbE\insq{A_{i,j}\Phi\inp{-\frac{A_{i,j}}{\sqrt{k-1+\sigma^2}}}}\nonumber\\
&= 0-2\bbE\insq{A_{i,j}\Phi\inp{-\frac{A_{i,j}}{\sqrt{k-1+\sigma^2}}}}\label{eq:expt2}
\end{align}
\begin{align}
\bbE&\insq{A_{i,j}\Phi\inp{-\frac{A_{i,j}}{\sqrt{k-1+\sigma^2}}}}\nonumber\\
& = \int_{-\infty}^{\infty}a\frac{1}{\sqrt{2\pi}}e^{-\frac{a^2}{2}}\inp{\frac{1}{\sqrt{2\pi}}\int_{-\infty}^{-\frac{a}{\sqrt{k-1+\sigma^2}}}e^{-\frac{t^2}{2}}dt}da\nonumber\\
& = \frac{1}{2\pi}\int_{-\infty}^{\infty}\int_{-\infty}^{-\frac{a}{\sqrt{k-1+\sigma^2}}}ae^{-\frac{a^2}{2}}e^{-\frac{t^2}{2}}dt\,da\nonumber\\
& \stackrel{(a)}{=} \frac{1}{2\pi}\int_{-\infty}^{\infty}\int_{-\infty}^{-{t}{\sqrt{k-1+\sigma^2}}}ae^{-\frac{a^2}{2}}e^{-\frac{t^2}{2}}da\,dt\nonumber\\
& =\frac{1}{2\pi}\int_{-\infty}^{\infty}\inp{\int_{-\infty}^{-{t}{\sqrt{k-1+\sigma^2}}}ae^{-\frac{a^2}{2}}da}e^{-\frac{t^2}{2}}dt\nonumber\\
& = \frac{1}{2\pi}\int_{-\infty}^{\infty}\inp{-e^{-\frac{t^2(k-1+\sigma^2)}{2}}}e^{-\frac{t^2}{2}}dt\nonumber\\
& = -\frac{1}{\sqrt{2\pi\inp{k+\sigma^2}}}\int_{-\infty}^{\infty}\frac{\sqrt{k+\sigma^2}}{\sqrt{2\pi}}e^{-\frac{t^2(k+\sigma^2)}{2}}dt\nonumber\\
& = -\frac{1}{\sqrt{2\pi\inp{k+\sigma^2}}}\label{eq:expt3}
\end{align} where $(a)$ follows for change of variable formula for integration. From \eqref{eq:expt2} and \eqref{eq:expt3}, we have 
\begin{align}
\bbE\insq{y_i A_{i,j}} = \sqrt{\frac{2}{\pi}}\times\frac{1}{\sqrt{\inp{k+\sigma^2}}}.\label{eq:expt4}
\end{align} From [Example 2.5.8]\cite{vershynin}, we also note that $\normi{{y_i}}_{\psi_2} = 1$. Thus, $L = \sqrt{\frac{2}{\pi}}\times\frac{1}{\sqrt{\inp{k+\sigma^2}}}$ and $\min\inb{L, L^2} = L^2$, which when substituted in \eqref{eq: alg_bound}  gives the desired bound.
\end{proof}

\begin{proof}[Proof of Corollary~\ref{thm:alg_spl}]
We first note that  $\frac{\bbE\insq{g'(\vecA_i^T\bx)}}{\normi{{y_i}}_{\psi_2}} = \frac{\bbE\insq{y_iA_{i,j}}}{\normi{{y_i}}_{\psi_2}}$ for  any $j$ in the support of $\bx$. This follows from \eqref{eq:log_expt11} and \eqref{eq:log_expt1_avg11}. We first compute $\bbE\insq{y_iA_{i,j}}$, which is the same as $\bbE\insq{\inp{\vecA_i^T\bx+z_i}A_{i,j}}$ for \spl. 
Note that $\bbE\insq{\inp{\vecA_i^T\bx+z_i}\inp{A_{i, j}}} = \bbE\insq{A_{i, j}^2} = 1$.
Also, from [Example 2.5.8]\cite{vershynin} 
\begin{align*}
\normi{\inp{\vecA_i^T\bx+z_i}}_{\psi_2}\leq C\sqrt{k+\sigma^2}\\
\end{align*} for some constants $C$. With this,
\begin{align*}
\frac{\bbE\insq{g'(\vecA_i^T\bx)}}{\normi{{y_i}}_{\psi_2}}\geq \frac{1}{C\sqrt{k+\sigma^2}}: =L.
\end{align*}Note that $\min\inb{L, L^2} = L^2$, which when substituted in \eqref{eq: alg_bound} gives the desired bound.
\end{proof}

\begin{proof}[Proof of Corollary~\ref{thm:alg_logreg}]
We will first compute $g(\vecA_i^T\bx) = \bbE\insq{y_i|\vecA_i^T\bx}$ for \logreg.
\begin{align*}
g(\vecA_i^T\bx)&=\bbE\insq{y_i|\vecA_i^T\bx}\\
&= \frac{1}{1+e^{-\beta \vecA_i^T\bx}}-\frac{e^{-\beta \vecA_i^T\bx}}{1+e^{-\beta \vecA_i^T\bx}}\\
&=\frac{1-e^{-\beta \vecA_i^T\bx}}{1+e^{-\beta \vecA_i^T\bx}}\\
& \stackrel{(a)}{=} {\tanh\inp{\frac{\beta \vecA_i^T\bx}{2}}}
\end{align*}where $(a)$ uses the definition of $\tanh$. Then
\begin{align*}
\bbE\insq{g'(\vecA_i^T\bx)} &= \frac{\beta}{2}\bbE\insq{\frac{1}{{\text{cosh}}^2\inp{\frac{\beta \vecA_i^T\bx}{2}}}}\\
& \stackrel{(c)}{\geq}\frac{\beta}{2}\bbE\insq{e^{-\frac{\inp{\beta\vecA_i^T\bx}^2}{4}}}
\end{align*} where $(c)$ follows from the inequality $\text{cosh}(t)\leq e^{t^2/2}$ (see [Exercise 2.2.3]\cite{vershynin}). 

% \begin{align*}
% \bbE\insq{y_i\vecA_i^T\bx} &= \bbE\insq{\vecA_i^T\bx\bbE\insq{y_i|\vecA_i^T\bx}}\\
% & = \bbE\insq{\vecA_i^T\bx\inp{\frac{1}{1+e^{-\beta \vecA_i^T\bx}}-\frac{e^{-\beta \vecA_i^T\bx}}{1+e^{-\beta \vecA_i^T\bx}}}}\\
% & = \bbE\insq{\vecA_i^T\bx\inp{\frac{1-e^{-\beta \vecA_i^T\bx}}{1+e^{-\beta \vecA_i^T\bx}}}}\\
% & = \bbE\insq{\vecA_i^T\bx\inp{\frac{e^{\beta \vecA_i^T\bx}-1}{e^{\beta \vecA_i^T\bx}+1}}}\\
% & \stackrel{(a)}{=} \bbE\insq{\vecA_i^T\bx\inp{\tanh\inp{\frac{\beta \vecA_i^T\bx}{2}}}}\\
% & \stackrel{(b)}{=} \frac{k\beta}{2}\bbE\insq{\frac{1}{{\text{cosh}}^2\inp{\frac{\beta \vecA_i^T\bx}{2}}}}\\
% & \stackrel{(c)}{\geq}\frac{k\beta}{2}\bbE\insq{e^{-\frac{\beta^2\vecA_i^T\bx^2}{2}}}\\
% \end{align*} , $(b)$ follows by noting that $\vecA_i^T\bx\sim N(0, k)$ and using Stein's lemma and $(c)$ follows from the inequality $\text{cosh}(t)\leq e^{t^2/2}$ (see \cite[Exercise 2.2.3]{vershynin}). 

Now, we need to compute $\bbE\insq{e^{-\frac{\inp{\beta\vecA_i^T\bx}^2}{4}}}$ where $\vecA_i^T\bx\sim N(0,k)$. Let $\sigma_1 := \frac{1}{\frac{\beta^2}{2}+\frac{1}{k}}$. Then

\begin{align}
\bbE\insq{e^{-\frac{\inp{\beta\vecA_i^T\bx}^2}{4}}} &= \int_{-\infty}^{\infty}\frac{1}{\sqrt{2\pi k}}e^{-\beta^2a^2/4}e^{-a^2/2k} da\nonumber\\
& = \sqrt{\frac{\sigma_1}{k}}\int_{-\infty}^{\infty}\frac{1}{\sqrt{2\pi \sigma_1}}e^{-x^2/2\sigma_1} da\nonumber\\
& = \sqrt{\frac{\sigma_1}{k}}\nonumber\\
& = \sqrt{\frac{2}{2+\beta^2 k}}\label{eq:expectation_log}
\end{align}

Thus,
\begin{align*}
\bbE\insq{g'(\vecA_i^T\bx)}&\geq \frac{\beta}{2}\sqrt{\frac{2}{2+\beta^2 k}}\\
& = \frac{1}{2}\sqrt{\frac{2}{2/\beta^2+ k}}.
\end{align*}
From [Example 2.5.8]\cite{vershynin}, we also note that $\normi{{y_i}}_{\psi_2} = 1$. Thus, $L = \frac{1}{2}\sqrt{\frac{2}{2/\beta^2+ k}}$ and $\min\inp{L, L^2} = L^2$, which gives the desired bound.

\end{proof}

