
\section{Basic Inequalities}\label{app:basic_inequalities}

In our proofs, we will need to repeatedly bound certain recurrences and sums.
In this section, we present useful inequalities to this end.

\begin{lemma}[Harmonic partial sum bound]\label{lemma:harmonic}
For any integers $s,\bar{s}$, constant $c\in\mathbb{R}$ such that $1 \leq \bar{s} < s$, $p \neq -1$, and $a \geq 0$, it holds that
\begin{align*}
   \log (s + a) - \log (\bar{s} + a ) + \frac{1}{s + a} &\leq \sum_{n = \bar{s}}^{s} \frac{1}{n + a} \leq \frac{1}{\bar{s} + a} + \log ( s + a) - \log (\bar{s} + a), \\
   \frac{(s + a)^{p+1}}{p+1} - \frac{(\bar{s} + a)^{p+1}}{(p+1)} + (\bar{s} + a)^p &\leq \sum_{n = \bar{s}}^{s} (n + a)^p \leq \frac{(s + a)^{p+1}}{p+1} - \frac{(\bar{s} + a)^{p+1}}{p+1} + (s + a)^p, \text{ if } p \geq 0 \\
   \frac{(s + a)^{p+1}}{p+1} - \frac{(\bar{s} + a)^{p+1}}{p+1} + (s + a)^p &\leq \sum_{n = \bar{s}}^{s} (n + a)^p \leq \frac{(s + a)^{p+1}}{p+1} - \frac{(\bar{s} + a)^{p+1}}{p+1} + (\bar{s} + a)^p, \text{ if } p \leq 0
\end{align*}
\end{lemma}
\begin{proof}
Let $f_1:\mathbb{R}_{\geq 0} \rightarrow \mathbb{R}_{\geq 0}$ be a non-decreasing positive function and $f_2:\mathbb{R}_{\geq 0} \rightarrow \mathbb{R}_{\geq 0}$ be a non-increasing positive function.
Then it holds that
\begin{align*}
    \int_{x = \bar{s}}^s f_1(x) dx + f_1(\bar{s}) \leq \sum_{n=\bar{s}}^s f_1(n) \leq \int_{x = \bar{s}}^s f_1(x) dx  + f_1(s), \\
    \int_{x = \bar{s}}^s f_2(x) dx + f_2(s) \leq \sum_{n=\bar{s}}^s f_2(n) \leq \int_{x = \bar{s}}^s f_2(x) dx + f_2(\bar{s}).
\end{align*}
The result follows from a simple integral bound with $\int \frac{1}{x} dx = \log x$ and $\int x^p dx = \frac{x^{p+1}}{p+1}$.
\end{proof}

We state a certain recurrence inequality that appears several times in our analysis as a lemma, in order to shorten some proofs.

\begin{lemma}[General error recurrence]\label{lemma:general_recurrence}
Let $c_0 \geq 0, c_1 \geq 0, \gamma > 1, a \geq 0$ be arbitrary constants such that $a \geq \gamma$.
Furthermore, let $\{u_t\}_{t=0}^\infty$ be a sequence of non-negative numbers such that for all $t \geq 0$, it holds that
\begin{align*}
    u_{t+1} \leq \frac{c_0}{t+a} + \frac{c_1}{(t+a)^2} + \left( 1 - \frac{\gamma}{t+a}\right) u_t.
\end{align*}
Then, for all values of $t\geq 0$, it holds that:
\begin{align*}
u_{t+1} \leq &\frac{u_0 a ^ \gamma + c_1 (a^{\gamma-2} + 1) (1+a^{-1})^\gamma + c_0 (1+a^{-1})^\gamma a^{\gamma-1}}{\left(t+a\right)^\gamma}  \\
    &\quad + \frac{c_0 + c_1 (1+a^{-1})^\gamma (\gamma - 1)^{-1}}{t+a} + \frac{c_1}{(t+a)^2} + \gamma^{-1}(1+a^{-1})^\gamma c_0 
\end{align*}
    
\end{lemma}
\begin{proof}
We note that inductively, we have
\begin{align*}
u_{t+1} \leq &\frac{c_0}{t+a} + \frac{c_1}{(t+a)^2} + u_0 \prod_{s=0}^{t} \left( 1 - \frac{\gamma}{s+a} \right) 
     + \sum_{s=0}^{t-1} \left( \frac{c_0}{s+a} + \frac{c_1}{(s+a)^2} \right) \prod_{s'=s+1}^{t} \left(1 - \frac{\gamma}{s'+a} \right).
\end{align*}
Using the inequality $1 + x \leq e^{x}$, we obtain
\begin{align*}
u_{t+1} \leq &\frac{c_0}{t+a} + \frac{c_1}{(t+a)^2} + u_0 \prod_{s=0}^{t} \exp\left\{- \frac{\gamma}{s+a}\right\} + \sum_{s=0}^{t-1} \left( \frac{c_0}{s+a} + \frac{c_1}{(s+a)^2} \right) \prod_{s'=s+1}^{t} \exp\left\{ - \frac{\gamma}{s'+a}\right\} \\
\leq &\frac{c_0}{t+a} + \frac{c_1}{(t+a)^2} + u_0 \exp\left\{- \sum_{s=0}^{t}\frac{\gamma}{s+a}\right\} + \sum_{s=0}^{t-1} \left( \frac{c_0}{s+a} + \frac{c_1}{(s+a)^2} \right)  \exp\left\{ -\sum_{s'=s+1}^{t} \frac{\gamma}{s'+a}\right\}. 
\end{align*}
Here, using Lemma~\ref{lemma:harmonic}, since $a - 1 > 0$, it holds that
\begin{align*}
  \sum_{s=0}^{t}\frac{\gamma}{s+a} &\geq \sum_{s = 1}^{t+1} \frac{\gamma}{s+(a - 1)} \geq \gamma \log(t+a) - \gamma \log a = \log \left(\frac{(t+1)^\gamma}{a^\gamma}\right) \\
  \sum_{s'=s+1}^{t} \frac{\gamma}{s'+a} &\geq \gamma \log(t + a) - \gamma \log(s + a + 1) \geq \log \left\{ \frac{(t+a)^\gamma}{(s+a+1)^\gamma} \right\},
\end{align*}
therefore $u_{t+1}$ can be further upper bounded by
\begin{align*}
u_{t+1} \leq &\frac{c_0}{t+a} + \frac{c_1}{(t+a)^2} + u_0 \frac{a^\gamma}{ \left(t+a\right)^\gamma} + \sum_{s=0}^{t-1} \left( \frac{c_0}{s+a}  + \frac{c_1}{(s+a)^2} \right) \left(\frac{s + a + 1}{t+a}\right)^\gamma \\
\leq &\frac{c_0}{t+a} + \frac{c_1}{(t+a)^2} + \frac{u_0 a ^ \gamma}{\left(t+a\right)^\gamma} + (t+a)^{-\gamma} \sum_{s=0}^{t-1} \left( \frac{c_0}{s+a} + \frac{c_1}{(s+a)^2} \right) \left(s+a+1\right)^\gamma \\
\leq &\frac{c_0}{t+a} + \frac{c_1}{(t+a)^2} + \frac{u_0 a ^ \gamma}{\left(t+a\right)^\gamma} + (t+a)^{-\gamma} (1 + a^{-1})^\gamma \sum_{s=0}^{t-1} \left( c_0 \left(s+a\right)^{\gamma-1} + c_1\left(s+a\right)^{\gamma-2} \right) .
\end{align*}
The last term can be bound with the corresponding integral (see Lemma~\ref{lemma:harmonic}), yielding (since $\gamma-1 > 0$):
\begin{align*}
    \sum_{s=0}^{t-1}(s+a)^{\gamma - 1} &\leq \frac{(t+a)^\gamma}{\gamma} + a ^ {\gamma - 1}.
\end{align*}
For the term $\sum_{s=0}^{t-1}(s+1)^{\gamma - 2}$, we analyzing the two cases $1 < \gamma \leq 2$ and $\gamma > 2$ using Lemma~\ref{lemma:harmonic} we obtain
\begin{align*}
    \sum_{s=0}^{t-1}(s+a)^{\gamma - 2} &\leq \frac{(t+a)^{\gamma-1}}{\gamma - 1} + a^{\gamma - 2} + 1.
\end{align*}
The two inequalities combined yield the stated bound,
\begin{align*}
    u_{t+1} \leq & \frac{c_0}{t+a} + \frac{c_1}{(t+a)^2} + \frac{u_0 a ^ \gamma}{\left(t+a\right)^\gamma} + (t+a)^{-\gamma} (1 + a^{-1})^\gamma \sum_{s=0}^{t-1} \left( c_0(s+a)^{\gamma-1} + c_1(s+a)^{\gamma - 2} \right) \\
    \leq & \frac{c_0}{t+a} + \frac{c_1}{(t+a)^2} + \frac{u_0 a ^ \gamma}{\left(t+a\right)^\gamma} + \gamma^{-1}(1+a^{-1})^\gamma c_0 + \frac{c_0 (1+a^{-1})^\gamma a^{\gamma-1}}{(t+a)^\gamma} \\ 
    &\quad +\frac{c_1 (1+a^{-1})^\gamma}{(t+a)(\gamma - 1)} + \frac{c_1 (a^{\gamma-2} + 1) (1+a^{-1})^\gamma}{(t+a)^\gamma} \\
    \leq & \frac{u_0 a ^ \gamma + c_1 (a^{\gamma-2} + 1) (1+a^{-1})^\gamma + c_0 (1+a^{-1})^\gamma a^{\gamma-1}}{\left(t+a\right)^\gamma}  \\
    &\quad + \frac{c_0 + c_1 (1+a^{-1})^\gamma (\gamma - 1)^{-1}}{t+a} + \frac{c_1}{(t+a)^2} + \gamma^{-1}(1+a^{-1})^\gamma c_0 .
\end{align*}
\end{proof}
