
\section{Utility analysis}\label{sec:appendix_utility}
In this section, we establish the utility guarantees for our algorithm. Initially, we calculate the accuracy for the query of the standard Bloom filter in Section~\ref{sec:acc_bloom}. We then assess the utility loss caused by introducing the random response technique by comparing the output of the DPBloomfilter with the output of the standard Bloom filter in Section~\ref{sec:acc_dpbloom_bloom}. Ultimately, we present the assessment of our algorithm's utility in Section~\ref{sec:acc_dpbloom_true}.

We begin by defining the notation we will use in this section.
\begin{definition}\label{def:three_z}
    Let $z \in \{0,1\}$ denote the true answer for whether $x \in A$. Let $\wh{z} \in \{0,1\}$ denote the answer outputs by \textsc{Bloom filter}. Let $\wt{z} \in \{0,1\}$ denote the answer output by \textsc{DPBloomFilter} (Algorithm~\ref{alg:init}).
\end{definition}

\subsection{Accuracy for query of Standard Bloom Filter}\label{sec:acc_bloom}

We first present the accuracy of the query of the standard bloom filter, as follows.

\begin{lemma}[Accuracy for query of Standard Bloom Filter
]\label{lem:bloom_true_accuracy:formal}
If the following conditions hold
\begin{itemize}
    \item Assume that a hash function selects each array position with equal probability. 
    \item Let $\wh{z}$ be defined as Definition~\ref{def:three_z}.
    \item Let $z$ be defined as Definition~\ref{def:three_z}.
    \item Let $\alpha := \Pr[z=0]$
\end{itemize}
Then, we can show
\begin{align*}
    \Pr [ \wh{z} = z ] \geq 1 - (1 - e^{-2|A| k / m})^k \cdot \alpha.
\end{align*}
Further if $m = \Omega(|A| k)$ and $k = \Theta(\log(1/\delta_{err}))$, we have
\begin{align*}
     \Pr [ \wh{z} = z ] \geq 1 - \delta_{err} \cdot \alpha.
\end{align*}
\end{lemma}

\begin{proof}
Recall that we have defined Bloom filter in Definition~\ref{def:bloom_filter}, it only has false positive error. Therefore, we only need to calculate the following
\begin{align*}
    \Pr[\wh{z} = 1 | z = 0]
\end{align*}

Recall that $A \subset [n]$ denotes the set of elements inserted into the Bloom filter. And $h_i : [n] \rightarrow [m]$ for each $i \in [k]$ denotes $k$ hash functions used in the Bloom filter. 

For a query $y \notin A$, we denotes event $E_1$ happens if the following happens:
\begin{align*}
    h_i[y] = 1, \forall i \in [k]
\end{align*}

Recall that we have defined Bloom filter in Definition~\ref{def:bloom_filter}, we have 
\begin{align}\label{eq:def_E_1}
    \Pr[\wh{z} = 1 | z = 0] = \Pr[E_1].
\end{align}

Now, we start calculating $\Pr[E_1]$.

Recall that we assume a hash function selects each array position with equal probability in the lemma statement. 

During one inserting operation, the probability of a certain bit is not set to $1$ is 
\begin{align*}
    (1 - \frac{1}{m})^k
\end{align*}



If we have inserted $|A|$ elements, the probability that a certain bit is still $0$ is
\begin{align*}
    (1 - \frac{1}{m})^{|A| k} = ( (1-\frac{1}{m})^{m} )^ {|A| k/m } \geq e^{-2 |A| k / m}
\end{align*}
where the last step follows from $(1-1/m)^m \geq e^{-2}$ for all $m \geq 2$.

Thus the probability that a certain bit is $1$ is
\begin{align*}
    1 - (1 - \frac{1}{m})^{ |A| k} \leq 1 - e^{-2 |A| k / m}.
\end{align*}

Combining the above fact, we have
\begin{align}\label{eq:pr_e}
    \Pr[E_1] = & ~ (1 - (1 - \frac{1}{m})^{|A|k})^k \notag \\
    \leq & ~ (1 - e^{-2 |A| k / m})^k.
\end{align}
where the first step follows from the definition of event $E_1$, the second step follows from $(1-1/m)^m \geq e^{-2}$ for all $m \geq 2$. 

Therefore, the accuracy of Bloom filter is
\begin{align*}
    \Pr[\wh{z} = z] 
    = & ~ 1 - \Pr[\wh{z} = 1 | z = 0] \Pr[z=0] \\
    = & ~ 1 - \Pr[E_1] \alpha \\
    \geq & ~ 1 - (1 - e^{-2 |A| k / m})^k \alpha.
\end{align*}
where the first step follows from Bloom filter only has false positive error, the second step follows from the definition of event $E_1$ and the definition of $\alpha$, the third step follows from Eq.~\eqref{eq:pr_e}. 

\end{proof}

\subsection{Accuracy (compare DPBloomFilter with Standard BloomFilter) for Query}\label{sec:acc_dpbloom_bloom}
We then assess the accuracy loss caused by the introduction of the random response technique by comparing the outputs of the DPBloomfilter with those of the standard Bloom filter.

\begin{lemma}[Accuracy (compare DPBloomFilter with Standard BloomFilter) for Query
]\label{lem:dpbloom_bloom_accuracy:formal}

If the following conditions hold
\begin{itemize}
    \item Let $\wh{z}$ be defined as Definition~\ref{def:three_z}.
    \item Let $\wt{z}$ be defined as Definition~\ref{def:three_z}.
    \item Let $\alpha: = \Pr[ z = 0 ] \in [0,1]$
    \item Let $t := \frac{ e^{\epsilon_0} }{ e^{\epsilon_0} + 1 }$. 
    \item Let $\delta_{\mathrm{err}}$ be defined as in Lemma~\ref{lem:bloom_true_accuracy:formal}. 
\end{itemize}

Then, we can show
\begin{align*}
\Pr[ \wt{z} = \wh{z}] \geq t \cdot (\alpha - \delta_{\mathrm{err}}).
\end{align*}

\end{lemma}
\begin{proof}
We denote the query as $q$. 

We define
\begin{align}\label{def:Q}
    Q := \{j \in [m] ~:~ h_i(q) = j,~ i \in [k]\}
\end{align}



We denote $Q[i]$ as the $i$-th element in $Q$. 

Using basic probability rules, we have
\begin{align*}
    & ~ \Pr[\wt{z} = \wh{z}] \\
    = & ~ \Pr[\wt{z} = 1 | \wh{z} = 1] \Pr[\wh{z} = 1] \\
    + & ~ \Pr[\wt{z} = 0 | \wh{z} = 0] \Pr[\wh{z} = 0].
\end{align*}

{\bf Step 1}. Calculate $\Pr[\wt{z} = 1 | \wh{z} = 1]$


We denote event $E_2$ happens as the following happens:
\begin{align*}
    \wt{g}[j] = g[j], \forall j \in Q.
\end{align*}

Recall that we have defined Bloom filter in Definition~\ref{def:bloom_filter}, we have 

\begin{align*}
    \Pr[\wt{z} = 1 | \wh{z} = 1] = \Pr[E_2].
\end{align*}

 
Now, we calculate the probability that $E_2$ happens. 
\begin{align*}
    \Pr [E_2] = & ~ \prod_{i = 1}^k \Pr [\wt{g}[Q[i]] = g[Q[i]]] \notag \\
    = & ~ (\frac{e^{\epsilon_0}}{e^{\epsilon_0} + 1})^k.
\end{align*}
where the first step follows from each entry of $g$ is independent, the second steps follows from the definition of $\wt{g}$. 

Therefore, we have
\begin{align}\label{eq:pr_wtz1_z1}
    \Pr[\wt{z} = 1 | \wh{z} = 1] 
    = & ~ (\frac{e^{\epsilon_0}}{e^{\epsilon_0} + 1})^k.
\end{align}

{\bf Step 2}. Calculate $\Pr[\wt{z} = 0 | \wh{z} = 0]$

Recall we have defined $Q \subset [m]$ in Eq.~\eqref{def:Q}. We further define
\begin{align*}
    Z := \{j \in Q ~:~ g[j] = 0\}.
\end{align*}

We denote $Z[i]$ as the $i$-th element in $Z$. 

We further define
\begin{align*}
    \ov{Q} := Q \backslash Z.
\end{align*}


By basic probability rules, we have
\begin{align*}
    \Pr[\wt{z} = 0 | \wh{z} = 0] = & ~ 1 - \Pr[\wt{z} = 1 | \wh{z} = 0].
\end{align*}

Now, let's calculate $\Pr[\wt{z} = 1 | \wh{z} = 0]$

$[\wt{z} = 1 | \wh{z} = 0]$ happens only if the following conditions hold:
\begin{enumerate}
    \item All elements in $Z$ flip from $0$ to $1$.
    \item All elements in $\ov{Q}$ remain $1$.
\end{enumerate}

Then, we have
\begin{align*}
    \Pr[\wt{z} = 1 | \wh{z} = 0]  = & ~ \prod_{i = 1}^{|Z|} \Pr [\wt{g}[Z[i]] = 1] \prod_{i = 1}^{|\ov{Q}|} \Pr [\wt{g}[\ov{Q}[i]] = 1] \notag \\
    = & ~ (\frac{1}{e^{\epsilon_0} + 1})^{|Z|} (\frac{e^{\epsilon_0}}{e^{\epsilon_0} + 1})^{|\ov{Q}|} \notag \\
    \leq & ~ (\frac{1}{e^{\epsilon_0} + 1})^{|Z|} \notag \\
    \leq & ~ \frac{1}{e^{\epsilon_0} + 1}.
\end{align*}
where the first step follows from the above analysis, the second step follows from the definition of $\wt{g}$, the third step follows from $|\ov{Q}| \geq 0$ and $\frac{e^{\epsilon_0}}{e^{\epsilon_0} + 1} < 1$, the fourth step follows from $|Z| \geq 1$ and $\frac{1}{e^{\epsilon_0} + 1} < 1$. 

Therefore, we have
\begin{align}\label{eq:pr_wtz0_z0}
    \Pr[\wt{z} = 0 | \wh{z} = 0] = & ~ 1 - \Pr[\wt{z} = 1 | \wh{z} = 0] \notag \\
    \geq & ~ 1 -  \frac{1}{e^{\epsilon_0} + 1} \notag \\
    = & ~ \frac{ e^{\epsilon_0} }{ e^{\epsilon_0} + 1 }.
\end{align}
Let $\hat \alpha := \Pr[ \wh{z} = 0 ]$, then we have $1- \wh{\alpha} = \Pr[ \wh{z} = 1 ]$. 
Let $\alpha := \Pr[ z = 0 ]$.
Note that $ \wh{\alpha} = \alpha (1 - \delta_{\mathrm{err}}) $.

Let $t := \frac{e^{\epsilon_0}}{e^{\epsilon_0} + 1}$. 

The final accuracy is 
\begin{align*}
& ~ \Pr[\wt{z} = 0 | \wh{z} = 0]  \cdot \Pr[ \wh{z} = 0 ] + \Pr[\wt{z} = 1 | \wh{z} = 1]  \cdot \Pr[ \wh{z} = 1 ] \\
= & ~ \Pr[\wt{z} = 0 | \wh{z} = 0]  \cdot \wh{\alpha} + \Pr[\wt{z} = 1 | \wh{z} = 1]  \cdot (1- \wh{\alpha}) \\
= & ~ \Pr[\wt{z} = 0 | \wh{z} = 0]  \cdot \alpha (1 - \delta_{err}) \\
+ & ~ \Pr[\wt{z} = 1 | \wh{z} = 1]  \cdot (1- \alpha + \alpha \cdot \delta_{err}) \\
\geq & ~ \frac{ e^{\epsilon_0} }{ e^{\epsilon_0} + 1 }  \cdot \alpha (1 - \delta_{err}) + (\frac{ e^{\epsilon_0} }{ e^{\epsilon_0} + 1 })^k  \cdot (1- \alpha + \alpha \cdot \delta_{err}) \notag \\ 
= & ~ t \cdot (\alpha - \alpha \cdot \delta_{err}) + t^k  \cdot (1- \alpha + \alpha \cdot \delta_{err}) \\
\geq & ~ t \cdot \alpha \cdot (1 - \delta_{err}).
\end{align*}



where the first step follows from the definition of $\wh{\alpha}$, the second step follows from $ \wh{\alpha} = \alpha (1 - \delta) $, the third step follows from  Eq.~\eqref{eq:pr_wtz1_z1} Eq.~\eqref{eq:pr_wtz0_z0}, the fourth step follows from basic algebra rules, the fifth step follows from $(1 - \alpha + \alpha \cdot \delta_{\mathrm{err}}) \geq 0$. 

Therefore, the final accuracy is $t \cdot (\alpha - \delta_{err})$. 
\end{proof}

\subsection{Accuracy (compare DPBloomfilter with true-answer) for Query}\label{sec:acc_dpbloom_true}
Now we can examine the utility guarantees of DPBloomfilter by calculating the error between the ground truth for query and the output of DPBloomfilter.

\begin{theorem}[Accuracy (compare DPBloomfilter with true-answer) for Query, formal version of Lemma~\ref{thm:dpbloom_true_accuracy:informal}]\label{thm:dpbloom_true_accuracy:formal}

If the following conditions hold
\begin{itemize}
    \item Let $\wh{z}$ be defined as Definition~\ref{def:three_z}.
    \item Let $z$ be defined as Definition~\ref{def:three_z}.
    \item Let $\alpha: = \Pr[ z = 0 ] \in [0,1]$
    \item Let $t := e^{\epsilon_0} / (e^{\epsilon_0} + 1)$. 
    \item Let $\delta_{\mathrm{err}}$ be defined as in Lemma~\ref{lem:bloom_true_accuracy:formal}. 
\end{itemize}

Then, we can show 
\begin{align*}
\Pr[ \wt{z} = z ] \geq \alpha (1-t-t^k) \delta_{\mathrm{err}} + \alpha t .
\end{align*}
\end{theorem}

\begin{proof}

We have
\begin{align*}
    & ~ \Pr[ \wt{z} = z ] \\
    = & ~ \Pr [\wt{z} = 0 | \wh{z} = 0] \Pr [\wh{z} = 0 | z = 0] \Pr[z=0] \\
    + & ~ \Pr [\wt{z} = 0 | \wh{z} = 1] \Pr [\wh{z} = 1 | z = 0] \Pr[z=0] \\
    + & ~ \Pr [\wt{z} = 1 | \wh{z} = 1] \Pr [\wh{z} = 1 | z = 1] \Pr[z=1] \\
    + & ~ \Pr [\wt{z} = 1 | \wh{z} = 0] \Pr [\wh{z} = 0 | z = 1] \Pr[z=1]\\
    \geq & ~ t \cdot (1 - \Pr[E_1]) \cdot \alpha + (1- t^k) \cdot \Pr[E_1]\cdot \alpha + t^k \cdot 1 \cdot (1-\alpha)\\
     = & ~ \alpha (1-t-t^k) \delta_{\mathrm{err}} + \alpha t + t^k(1-\alpha)\\
     \geq & ~ \alpha (1-t-t^k) \delta_{\mathrm{err}} + \alpha t.
\end{align*}
where the first step from basic probability rules, the secod step follows from Equation~\ref{eq:def_E_1}, Equation \ref{eq:pr_wtz0_z0} and definition of $\alpha$ and $t$, the third step follows from basic algebra,  the fourth step follows from the fact that $t,\alpha \in [0,1]$.

\end{proof}

To make it easier to understand, we also provide the utility analysis of the Bloom filter under the case of random guess.  

\begin{lemma}[Accuracy for Query under Random Guess]\label{lem:random_guess}
If the following conditions hold
\begin{itemize}
    \item Let $\wh{z}$ be defined as Definition~\ref{def:three_z}.
    \item $\epsilon_0 = 0$. Namely, each bit in the bit-array of the DP Bloom has $\frac{1}{2}$ probability to be set to $0$, and  $\frac{1}{2}$ probability to be set to $1$. 
\end{itemize}

Then, we can show 
\begin{align*}
    \Pr[\wt{z} = 0] = & ~ 1 - \frac{1}{2^k}, \notag \\
    \Pr[\wt{z} = 1] = & ~ \frac{1}{2^k}.
\end{align*}
\end{lemma}

\begin{proof}
    By the definition of Bloom filter~\ref{def:bloom_filter}, the answer $\wt{z} = 1$ requires $k$ corresponding positions in the bit-array of the query are all set to $1$. 

    Note that each bit has $\frac{1}{2}$ probability to be set to $1$. Therefore, we have
    \begin{align*}
        \Pr[\wt{z} = 1] = \frac{1}{2^k} .
    \end{align*}

    Then, we have $\Pr[\wt{z} = 0] = 1 - \Pr[\wt{z} = 1] = 1 - \frac{1}{2^k}.$
\end{proof}




