
\section{Proof of Theorem~\ref{thm:binary} and Theorem~\ref{thm:multi}}

\subsection{Proof of Theorem~\ref{thm:binary}}
\label{sec:proof-thm-binary}

 We begin by analyzing the $\rein$ based gradient estimator.
With $N$ samples, we have: 
\begin{align*}
\mse(\hat{\nabla}^{\mathsf{RF}}_{N})
= \V(\hat{\nabla}^{\mathsf{RF}}_{N})
=\frac{1}{N} \V_{A \sim \pi_\theta} \bigg(A \nabla_\theta \log(\pi_\theta(A)) \bigg).
\end{align*}

Using the definition of $A$, we derive the following:
\begin{align*}
\V_{A \sim \pi_\theta} \left(A \nabla_\theta \log(\pi_\theta(A)) \right) = \frac{1}{(1-\theta) \theta} - 4.
\end{align*}
As a result, we have:
\begin{align}
\mse(\hat{\nabla}^{\mathsf{RF}}_{N}) =  \frac{1}{N
}\left(\frac{1}{(1-\theta) \theta} - 4\right). \label{eqn:mse-rf-bin}
\end{align}

 
Next, we analyze the pathwise gradient estimator $\hat{\nabla}^{\mathsf{grad}}_{\tilde{\tau},N}$.
Let $h_{\tau}(U,\theta) = \frac{\exp\left(\frac{U-\theta}{\tau}\right)-1}{\exp\left(\frac{U-\theta}{\tau}\right)+1}$ 
be a random variable,
where $U \sim \mathsf{Uni}[0,1]$, so that:
\begin{align}
\mse(\hat{\nabla}^{\mathsf{grad}}_{\tau,N}) = \left[
\bias(\nabla_\theta h_{\tau}(U,\theta))\right]^2 + \frac{1}{N} \V(\nabla_\theta h_{\tau}(U,\theta)).
\label{eqn:mse-decompo-bin}
\end{align}


To compute the bias term in~\eqref{eqn:mse-decompo-bin}, we note that
\begin{align*}
\E(h_{\tau}(U,\theta)) & = \E \left(\frac{1}{1+\exp\left( -\frac{U-\theta}{\tau}\right)}\right) - \E\left(\frac{1}{\exp\left(\frac{U-\theta}{\tau}\right)+1} \right) =2 \tau \log \left( \frac{\exp (\frac{1-\theta}{\tau})+1}{\exp (\frac{-\theta}{\tau})+1}\right)-1, \end{align*}
\begin{align*}
\nabla_\theta \E(h_{\tau}(U,\theta)) & = 2 \left(\frac{1}{1+\exp\left(\frac{1-\theta}{\tau} \right)} - \frac{1}{1+\exp\left(\frac{-\theta}{\tau} \right)}\right).
\end{align*} 
Therefore,
\begin{align}
\left[\bias(\nabla_\theta h_{\tau}(U,\theta))\right]^2 = 4 \left(1+\frac{1}{1+\exp\left(\frac{1-\theta}{\tau} \right)} - \frac{1}{1+\exp\left(\frac{-\theta}{\tau} \right)}\right)^2.
\label{eqn:mse-bias-bin}
\end{align}
Note that the above term goes to 4 as $\tau \to \infty$. The other part contributing to the mse~\eqref{eqn:mse-decompo-bin} is  the variance term and it satisfies
\begin{align*}
\V(\nabla_\theta h_{\tau}(U,\theta)) \le 
\E\left[\nabla_\theta (h_{\tau}(U,\theta))\right]^2 =
\frac{4}{\tau} \left[ \frac{3 \exp\left(\frac{-\theta}{\tau}\right) +1}{6 \left(\exp\left(\frac{-\theta}{\tau}\right)+1\right)^3 } - \frac{3 \exp\left(\frac{1-\theta}{\tau}\right) +1}{6 \left(\exp\left(\frac{1-\theta}{\tau}\right)+1\right)^3 }  \right].
\end{align*}
Combining the above equation with~\eqref{eqn:mse-bias-bin},
we arrive at $\mse(\hat{\nabla}^{\mathsf{grad}}_{\tilde{\tau},N}) 
\le 
v_N(\tau)$, where
\begin{align*}
v_N(\tau) \defeq 
4
\left(1+\frac{1}{1+\exp\left(\frac{1-\theta}{\tau} \right)} - \frac{1}{1+\exp\left(\frac{-\theta}{\tau} \right)}\right)^2 + \frac{1}{N}
\frac{4}{\tau} \left[ \frac{3 \exp\left(\frac{-\theta}{\tau}\right) +1}{6 \left(\exp\left(\frac{-\theta}{\tau}\right)+1\right)^3 } - \frac{3 \exp\left(\frac{1-\theta}{\tau}\right) +1}{6 \left(\exp\left(\frac{1-\theta}{\tau}\right)+1\right)^3 }  \right]
\end{align*}

 

For all $N \ge 1$, 
we can verify that $\lim_{\tau \to \infty} v_N(\tau) = 4$
and for large enough $\tau$, $v_N(\tau)$ is increasing in $\tau$. Thus, there exists some 
$\Tilde{\tau} > 0$ such that $\mse(\hat{\nabla}^{\mathsf{grad}}_{\tilde{\tau},N}) < 4$.
Comparing this with~\eqref{eqn:mse-rf-bin} for $\mse(\hat{\nabla}^{\mathsf{RF}}_{N}) $  completes the proof.
 

\subsection{Proof of Theorem~\ref{thm:multi}}
\label{sec:proof-thm-multi}



 For every $j$,
$G(A) \nabla_{\theta_i} \log(\pi_\theta(A)) = \frac{G(a_j)}{\pi_\theta(a_j)}\nabla_{\theta_i} (\pi_\theta(a_j))$
with probability $\frac{\theta_j}{\sum_{j=1}^m \theta_j}$
and
\begin{align*}
\frac{G(a_j)}{\pi_\theta(a_j)}\nabla_{\theta_i} (\pi_\theta(a_j))
&= \begin{cases}
\frac{-G(a_j)}{\sum_{j=1}^m\theta_j}, & j \ne i \\ 
\frac{G(a_i)}{\theta_i} - \frac{G(a_i)}{\sum_{j=1}^m\theta_j},  & j =i.
\end{cases}
\end{align*}

Therefore,
\begin{align}
\mse(\hat{\nabla}^{\mathsf{RF}}_{N,\theta_i})
 & =   \V_{A \sim \pi_\theta} \bigg(G(A) \nabla_{\theta_i} \log(\pi_\theta(A)) \bigg) \nonumber \\
  & = \sum_{j\neq i} \frac{\theta_j}{\sum_{j=1}^m \theta_j} \frac{(G(a_j))^2}{(\sum_{j=1}^m\theta_j)^2} +  \frac{\theta_i}{\sum_{j=1}^m \theta_j} \left( \frac{G(a_i)}{\theta_i} - \frac{G(a_i)}{\sum_{j=1}^m\theta_j} \right)^2 - \left(\nabla_{\theta_i} \E_{A\sim \pi_\theta}(G(A))\right)^2  \nonumber  
\\ &= \frac{\sum_{j=1}^m\theta_j(G(a_j))^2}{(\sum_{j=1}^m\theta_j)^3} + \frac{(G(a_i))^2}{\theta_i\sum_{j=1}^m \theta_j} - 2 \frac{(G(a_i))^2}{(\sum_{j=1}^m \theta_j)^2}  - \left(\nabla_{\theta_i} \E_{A\sim \pi_\theta}(G(A))\right)^2.
\label{eqn:mse-reinforce}
\end{align}




% \[\sum_{i=1}^mG(a_i) (\tilde{h}_\tau(Z,\theta))_i = \sum_{i=1}^m f\left( a_i \right) \left( \frac{\exp((\log (\theta_i)+Z_i)/\tau)}{\sum_{j=1}^{m}\exp((\log (\theta_j)+Z_j)/\tau)}\right)  \]


% \[ \nabla_{\theta_k}\sum_{i=1}^mG(a_i) (\tilde{h}_\tau(Z,\theta))_i  = \sum_{i=1}^mG(a_i) \nabla_{\theta_k}(\tilde{h}_\tau(Z,\theta))_i \]
We also note that
\begin{align*}
    \nabla_{\theta_k}{G\left(\sum_{i=1}^ma_i (\tilde{h}_\tau(Z,\theta))_i\right)} &= {G'\left(\sum_{i=1}^ma_i (\tilde{h}_\tau(Z,\theta))_i\right)}\left(\frac{\exp\left(\frac{Z_k}{\tau}\right) {\theta_k}^{\frac{1}{\tau}}}{\tau \theta_k}\right) \\& \left( \frac{a_k}{\sum_{j=1}^m{\exp\left(\frac{Z_j}{\tau}\right)}{\theta_j}^{\frac{1}{\tau}}} - \sum_{i=1}^m\frac{a_i\exp\left(\frac{Z_i}{\tau}\right){\theta_i}^{\frac{1}{\tau}}}{(\sum_{j=1}^m{\exp\left(\frac{Z_j}{\tau}\right)}{\theta_j}^{\frac{1}{\tau}})^2}\right),
\end{align*}
and therefore, 
$\lim_{\tau \to \infty} \nabla_{\theta_k}{G\left(\sum_{i=1}^ma_i (\tilde{h}_\tau(Z,\theta))_i\right)} = 0 $ for all $Z$.

Noting that $|G'(\cdot)| \le \bar{G}$, we have 
\begin{align*}
    \lim_{\tau \to \infty} \nabla_{\theta_k}
    G\left(\sum_{i=1}^m a_i (\tilde{h}_\tau(Z,\theta))_i \right) = 0.
\end{align*}

As a result,  
\begin{align*}
    \lim_{\tau \to \infty}\V_Z \left(\nabla_{\theta_k}
    G
    \left(\sum_{i=1}^m a_i (\tilde{h}_\tau(Z,\theta))_i \right)
    \right) =0,
\end{align*} and
\begin{align*}
    \lim_{\tau \to \infty} \left[\bias(\hat{\nabla}^{\mathsf{grad}}_{\tau,N, \theta_i})\right]^2 = \left(\nabla_{\theta_i} \E_{A\sim \pi_\theta}(G(A))\right)^2.
\end{align*} 
Theorem~\ref{thm:multi} follows directly from the above.

% We can also show that for $\tau$ large enough, 
% $\left[\bias_i(\hat{\nabla}^{\mathsf{grad}}_{\tau,N})\right]^2$ is increasing in $\tau$.
% Therefore, there exists $\tilde{\tau}$ such that 
% \begin{align*}
% \mse_i(\hat{\nabla}^{\mathsf{grad}}_{\Tilde{\tau},N}) \leq \left(\nabla_{\theta_i} \E_{A\sim \pi_\theta}(G(A))\right)^2
% \end{align*}
% and we finish the proof.





 