

\begin{table*}[ht]
\caption{LLM alignment objectives of \Ours. In the table, $\gamma(y \mid x) = \beta \log \frac{\pi_\theta(y \mid x)}{\pi_{\mathrm{ref}}(y \mid x)}$. All the proofs can be found in Appendix \ref{apx:proofs}.}
  \label{tb:all-llm-objective}
  \centering
  \scalebox{0.77}{
  \begin{tabular}{lccc}
    \toprule
    Method & Assumption of $r(x,y)$  & Objective       \\
    \midrule
   DPO & $ \mathbb{P}\text{r}(y_w \succeq y_l) = \sigma(r(x,y_w) - r(x,y_l))$     & $\mathcal{L}_{\text{pair}}=-\mathbb{E}\;\biggl[
   \log \sigma\Bigl(
     \beta \log\!\tfrac{\pi_\theta(y_w \mid x)}{\pi_{\mathrm{ref}}(y_w \mid x)}-
     \beta \log\!\tfrac{\pi_\theta(y_l \mid x)}{\pi_{\mathrm{ref}}(y_l \mid x)}
   \Bigr)
\biggr]$   \\
    \midrule
    \Ours (Contrastive) & $\mathbb{P}\text{r}(y_w \succeq y^{(1)}_l, ..., y_w \succeq y^{(m)}_l) 
= \text{softmax}(r(x, y_w))$ & $\mathcal{L}_{\text{con}} = -\mathbb{E} \biggl[
    \log \frac{\exp\bigl(\gamma(y_w \mid x)\bigr)}{
       \exp\bigl(\gamma(y_w \mid x)\bigr) + \sum_{i=1}^m \exp\bigl(\gamma(y_l^{(i)} \mid x)\bigr)}
    \biggr]$  \\
    \midrule
    \Ours (LambdaRank) & $\mathbb{P}\text{r}(y_1 \succeq ... \succeq y_m) = \prod_{1<i<j<m} \sigma(r(x,y_i) - r(x,y_j))$ & $\mathcal{L}_{\text{lamb}}=-\mathbb{E}\;\biggl[ \sum_{1<i<j<m}
   \log \sigma\Bigl(
     \gamma(y_i \mid x)-
     \gamma(y_j \mid x)
   \Bigr)
\biggr]$  \\
    \midrule
    \Ours (ListMLE) & $\mathbb{P}\text{r}(y_1 \succeq ... \succeq y_m) = \prod^m_{i=1} \text{softmax}^m_i(r(x, y_i))$ & $ \mathcal{L}_{\text{lmle}} = -\mathbb{E} \biggl[
    \sum^m_{i=1} \log \frac{\exp\bigl(\gamma(y_i \mid x)\bigr)}{
        \exp\bigl(\gamma(y_i \mid x)\bigr) + \sum_{j=i}^m \exp\bigl(\gamma(y_j \mid x)\bigr)}
    \biggr]$  \\
    \bottomrule
  \end{tabular}}
%   \vspace{-0.2in}
\end{table*}
