\begin{tcolorbox}[enhanced, colback=black!5!white, colframe=black!75!white, title=A Failed Case of \name]

\textbf{Problem (USAMO 2004):} 
Let $a, b, c$ be positive reals. Prove that
\begin{equation*}
(a + b + c) ^ 3 \leq (a ^ 5 - a ^ 2 + 3) * (b ^ 5 - b ^ 2 + 3) * (c ^ 5 - c ^ 2 + 3)
\end{equation*}
\tcbline


\textbf{Formal solution:}
\begin{lstlisting}
theorem Problem_3dP5 {a b c : ℝ} (ha : a > 0) (hb : b > 0) (hc : c > 0) : (a + b + c) ^ 3 ≤ (a ^ 5 - a ^ 2 + 3) * (b ^ 5 - b ^ 2 + 3) * (c ^ 5 - c ^ 2 + 3) := by 
  scale NEQ_Cauchy_Schwarz_left_sqrt_3vars (u1 := 1) (u2 := 1) (u3 := 1) (v1 := a) (v2 := b) (v3 := c) ...
  scale NEQ_weighted_AM_GM_left_3vars (u := a + b + c) (v := 3) (w := a^2 + b^2 + c^2) (i1 := 1) (i2 := 1/2) (i3 := 1/2) ...
  llm_frac_reduce ...
  llm_cancel_denom ...
  scale NEQ_Cauchy_Schwarz_sqrt_left_2vars (u1 := 1) (u2 := 1) (v1 := a) (v2 := a) ...
  llm_simplify ...
  llm_rearrange ...
  llm_simplify ...
  llm_rearrange ...
  llm_simplify ...
  llm_rearrange ...
  llm_frac_apart ...
  llm_simplify ...
  llm_rearrange ...
  llm_frac_apart ...
  llm_simplify ...
  llm_simplify ...
  llm_rearrange ...
  llm_simplify ...
  llm_rearrange ...
  llm_simplify ...
  llm_factor ... = 4*sqrt (2)*sqrt (b^2 + c^2)*(3 + a^2 + b^2 + c^2 + 2*a + 2*b + 2*c)^2 + (1 + a)^2*(3 + a^2 + b^2 + c^2 + 2*a + 2*b + 2*c)^2 - (64*(3 + a^5 - a^2)*(3 + b^5 - b^2)*(3 + c^5 - c^2))
  FAIL(TIMEOUT)! 
\end{lstlisting}

\end{tcolorbox}

\begin{tcolorbox}[enhanced, colback=black!5!white, colframe=black!75!white, title=A Successful Case of \name]

\textbf{Problem (Evan Chen):} 
If $a, b, c$ are positive reals and $a ^ 2 + b ^ 2 + c ^ 2 = 1$, then
\begin{equation*}
\frac{1}{a^2+2}+\frac{1}{b^2+2}+\frac{1}{c^2+2} \leq \frac{1}{6 a b+c^2}+\frac{1}{6 b c+a^2}+\frac{1}{6 c a+b^2}.
\end{equation*}
\tcbline


\textbf{Formal solution:}
\begin{lstlisting}
theorem Problem_2d4e1 {a b c : ℝ} (ha : a > 0) (hb : b > 0) (hc : c > 0) (h : a ^ 2 + b ^ 2 + c ^ 2 = 1) : 1 / (a ^ 2 + 2) + 1 / (b ^ 2 + 2) + 1 / (c ^ 2 + 2) ≤ 1 / (6 * a * b + c ^ 2) + 1 / (6 * b * c + a ^ 2) + 1 / (6 * c * a + b ^ 2) := by
  scale NEQ_AM_GM_div_square_right_2vars (u := b) (v := c) ...
  scale NEQ_AM_GM_div_square_right_2vars (u := b) (v := a) ...
  scale NEQ_AM_GM_div_square_right_2vars (u := a) (v := c) ...
  llm_simplify ...
  llm_simplify ...
  llm_rearrange ...
  sym_tangent_line ...
  llm_simplify ... = 27/49 - (27*a^2/49) - (27*b^2/49) - (27*c^2/49)
  try close
  SUCCESS!
\end{lstlisting}
\end{tcolorbox}


\section{Some more cases of \name} \label{app:case_study}

\input{answers/more_cases}

% %
% %\url{https://artofproblemsolving.com/community/c5h476722p2669114}

% https://math.stackexchange.com/questions/1589186/prove-that-fracaba5b5ab-fracbcb5c5bc-fraccac5a5ca-l

