\begin{tcolorbox}[breakable, enhanced, colback=black!5!white, colframe=black!75!white, title=A Different Proof Generated by \name (1)]

\textbf{Problem:} 
Let $a, b, c$ be three positive reals. Prove that if $abc = 1$, then
\begin{equation*}
a ^ 2 + b ^ 2 + c ^ 2 \ge a + b + c
\end{equation*}

Source: {\small\url{https://web.evanchen.cc/handouts/Ineq/en.pdf}}

\tcbline

\textbf{Formal solution:}
\begin{lstlisting}
theorem Example_1d7 {a b c : ℝ} (h : a * b * c = 1) : a + b + c ≤ a ^ 2 + b ^ 2 + c ^ 2 := by
  scale NEQ_AM_GM_left_square_2vars (u := 1) (v := a) ...
  scale NEQ_AM_GM_left_square_2vars (u := 1) (v := c) ...
  scale NEQ_AM_GM_left_square_2vars (u := 1) (v := b) ...
  llm_rearrange ...
  llm_simplify ...  = 3/2 - a^2/2 - b^2/2 - c^2/2
  llm_rearrange (left := 3/2) (right := a^2/2 + b^2/2 + c^2/2)
  scale NEQ_AM_GM_right_normal_3vars (u := a^2/2) (v := b^2/2) ...
  llm_simplify ...  = (a*b*c)^2 / 8
  llm_simplify ...  = 1 / 8
  try close
\end{lstlisting}

{Note: At first glance, ``AM-GM alone is hopeless here, because whenever we apply AM-GM, the left and right hand sides of the inequality all have the same degree''. However, \name find a proof by using $1 \times a \leq \frac{a^2+1}{2}$, $1 \times b \leq \frac{b^2+1}{2}$, $1 \times c \leq \frac{c^2+1}{2}$}.
\end{tcolorbox}

\vspace{2em}

\begin{tcolorbox}[breakable, enhanced, colback=black!5!white, colframe=black!75!white, title=A Different Proof Generated by \name (2)]

\textbf{Problem (JMO 2012):} 
Let $a, b, c$ be positive reals. Prove that
\begin{equation*}
\frac{a^3+5b^3}{3a+b}+\frac{b^3+5c^3}{3b+c}+\frac{c^3+5a^3}{3c+a} \geq \frac{3}{2}(a^2+b^2+c^2).
\end{equation*}

Source: {\small\url{https://artofproblemsolving.com/community/c5h476722p2669114}}

\tcbline

\textbf{Formal solution:}
\begin{lstlisting}
theorem Problem_3de6'' {a b c : ℝ} (ha : a > 0) (hb : b > 0) (hc : c > 0) : (3 / 2) * (a ^ 2 + b ^ 2 + c ^ 2) ≤ (a ^ 3 + 5 * b ^ 3) / (3 * a + b) + (b ^ 3 + 5 * c ^ 3) / (3 * b + c) + (c ^ 3 + 5 * a ^ 3) / (3 * c + a) := by
  llm_cancel_factor ...
  scale NEQ_Muirhead2_onestep_right_3vars (u := a) (v := b) ...
  scale NEQ_Muirhead1_left_3vars (u := c) (v := a) (w := b) ...
  scale NEQ_Muirhead1_left_3vars (u := a) (v := b) (w := c) ...
  scale NEQ_Muirhead2_onestep_left_3vars (u := a) (v := b) ...
  llm_cancel_factor ...
  scale NEQ_Muirhead2_onestep_right_3vars (u := a) (v := b) ...
  llm_simplify ...
  scale NEQ_Muirhead2_left_3vars (u := c) (v := b) (w := a) ...
\end{lstlisting}

{Note: A completely mechanical proof, achieved by iteratively applying Muirhead inequality six times after canceling the denominator}

\end{tcolorbox}

\vskip 2em

\begin{tcolorbox} [breakable, enhanced, colback=black!5!white, colframe=black!75!white, title=\name Checks Existing Answers (1)]

\textbf{Problem (Japan 1997):} 
Prove that
\begin{equation*}
\frac{\left(b+c-a\right)^{2}}{\left(b+c\right)^{2}+a^{2}}+\frac{\left(c+a-b\right)^{2}}{\left(c+a\right)^{2}+b^{2}}+\frac{\left(a+b-c\right)^{2}}{\left(a+b\right)^{2}+c^{2}}\geq\frac{3}{5}
\end{equation*}

Source: {\small\url{https://artofproblemsolving.com/community/c6h146p537}}

\tcbline

\textbf{Informal solution No.1 (provided by AoPS community):}

Solution: 

Let :

$ P = \frac {\left(b + c - a\right)^{2}}{\left(b + c\right)^{2} + a^{2}} + \frac {\left(c + a - b\right)^{2}}{\left(c + a\right)^{2} + b^{2}} + \frac {\left(a + b - c\right)^{2}}{\left(a + b\right)^{2} + c^{2}}$

{\color{red} By Cauchy Swarchz inequality, we have
$$
\begin{aligned}
 & (a^2 + b^2 + c^2 + (a + b)^2 + (b + c)^2 + (c + a)^2)(P) \geq (a + b + c)^2 \\
 & (3(a^2 + b^2 + c^2) + 2(ab + bc + ca))(P) \geq (a + b + c)^2 \\
 & (3(a + b + c)^2 - 4(ab + bc + ca))(P) \geq (a + b + c)^2 \\
\end{aligned}
$$
}

Hence, 

$ P \geq \frac {(a + b + c)^2}{3(a + b + c)^2 - 4(ab + bc + ca)^2}$

but we know that $ (a + b + c)^2 \geq 3(ab + bc + ca)$,

$ P\geq \frac {3(ab + bc + ca)}{9(ab + bc + ca) - 4(ab + bc + ca)} = \frac{3}{5}$

...

\vskip 2pt

Note: the proof is correct if all variables are assumed to be positive. However, without this assumption, applying Cauchy-Schwarz is incorrect, and a counterexample is successfully found by our symbolic solver $[c := 8.0, a := 1/8, b := (-1.0)]$.

This problem is proved by \name using llm\_simplification and tangent\_line trick tactics.


\end{tcolorbox}

\vskip 2em

\begin{tcolorbox} [breakable, enhanced, colback=black!5!white, colframe=black!75!white, title=\name Checks Existing Answers (2)]

\textbf{Problem (Japan 1997):} 
Prove that
\begin{equation*}
\frac{\left(b+c-a\right)^{2}}{\left(b+c\right)^{2}+a^{2}}+\frac{\left(c+a-b\right)^{2}}{\left(c+a\right)^{2}+b^{2}}+\frac{\left(a+b-c\right)^{2}}{\left(a+b\right)^{2}+c^{2}}\geq\frac{3}{5}
\end{equation*}

Source: {\small\url{https://artofproblemsolving.com/community/c6h146p537}}

\tcbline

\textbf{Informal solution No.2 (provided by AoPS community):}

....

don't use so much of mathematics on that simple problem.. 

:P :D
here's the solution using TITU's lemma..

The lemma-

if $x,y,a,b$ are reals and $x,y>0$ then
$ \frac {a^2}{x} + \frac {b^2}{y}\ge\frac {{(a + b}^2}{(x + y)}$

simply applying the lemma on the lhs twice

we get

$ LHS\ge\frac {{(a + b + c)}^2}{3(a^2 + b^2 + c^2) + 2(ab + bc + ca)}$

{\color{red} by AM-GM

$ {(a + b + c)}^2\ge3(ab + bc + ca) ~\text{and}~ 3(a^2 + b^2 + c^2) + 2(ab + bc + ca)\ge5(ab + bc + ca)$
}

...

\vskip 2pt

{Note: it appears that the issue arises from the inequality being in the wrong direction. Actually, the problem is unprovable when applying the Titu's lemma (a counterexample found by our symbolic solver: $[b=1.0, a = 1.0, c=0.5]$)}

\end{tcolorbox}

% %
% %\url{https://artofproblemsolving.com/community/c5h476722p2669114}

% https://math.stackexchange.com/questions/1589186/prove-that-fracaba5b5ab-fracbcb5c5bc-fraccac5a5ca-l

