\newpage
\begin{tcolorbox}[breakable, enhanced, colback=black!5!white, colframe=black!75!white,  title=A Failed Case of OpenAI o1-preview]
{\small
\textbf{Prompt:} 
Please solve the following problem:
For $a > 0, b > 0, c > 0, d > 0$ such that $a \cdot b + b \cdot c + c \cdot d + d \cdot a = 1$, show that:
\begin{equation*}
\frac{a^3}{b+c+d} + \frac{b^3}{c+d+a} + \frac{c^3}{d+a+b} + \frac{d^3}{a+b+c} \geq \frac{1}{3}
\end{equation*}
\tcbline

\textbf{Informal solution:}

To solve this problem, we aim to show that for positive real numbers \(a\), \(b\), \(c\), \(d\) satisfying \(ab + bc + cd + da = 1\), the inequality
\[
\frac{a^3}{b+c+d} + \frac{b^3}{c+d+a} + \frac{c^3}{d+a+b} + \frac{d^3}{a+b+c} \geq \frac{1}{3}
\]
holds true.

\emph{Step 1: Simplify the Inequality}.
First, note that 
\[
b + c + d = (a + b + c + d) - a = S - a,
\]
where \(S = a + b + c + d\). Thus, the inequality can be rewritten as:
\[
\sum_{\text{cyclic}} \frac{a^3}{S - a} \geq \frac{1}{3}.
\]

\emph{Step 2: Analyze the Function}.
Consider the function 
\[
f(x) = \frac{x^3}{S - x} \quad \text{for} \quad x \in (0, S).
\]
We will investigate the convexity of this function to apply Jensen's inequality.

Compute the second derivative:
\[
f''(x) = \frac{2S^2 + 2Sx + x^2}{(S - x)^3} > 0 \quad \text{for} \quad x \in (0, S).
\]
This shows that \(f(x)\) is convex on \((0, S)\).

\emph{Step 3: Apply Jensen's Inequality}.
Since \(f(x)\) is convex, Jensen's inequality states that:
\[
\frac{1}{4} \sum_{i=1}^{4} f(a_i) \geq f\left( \frac{1}{4} \sum_{i=1}^{4} a_i \right) = f\left(\frac{S}{4}\right)
\]

Compute \(f\left(\frac{S}{4}\right)\):
\[
f\left(\frac{S}{4}\right) = \frac{\left(\frac{S}{4}\right)^3}{S - \frac{S}{4}} = \frac{\left(\frac{S}{4}\right)^3}{\frac{3S}{4}} = \frac{S^2}{48}
\]

Therefore, the sum becomes:
\[
\sum_{\text{cyclic}} \frac{a^3}{S - a} \geq 4 \cdot \frac{S^2}{48} = \frac{S^2}{12}
\]

\emph{Step 4: Relate \(S\) to the Given Condition}.
From the given condition \(ab + bc + cd + da = 1\), and using the Cauchy-Schwarz inequality:
\[
(ab + bc + cd + da) \leq \frac{1}{2}\left(a^2 + b^2 + c^2 + d^2\right)
\]

But since \(ab + bc + cd + da = 1\), we get:
\[
a^2 + b^2 + c^2 + d^2 \geq 2
\]

{\color{red} Also, note that 
\[
S^2 = (a + b + c + d)^2 \geq 4(a^2 + b^2 + c^2 + d^2) \geq 8, \quad \text{so} \ S^2 \geq 8.
\]

Therefore:
\[
\sum_{\text{cyclic}} \frac{a^3}{S - a} \geq \frac{S^2}{12} \geq \frac{8}{12} = \frac{2}{3}
\]
But this contradicts the desired inequality, suggesting a miscalculation.}

\emph{Step 5: Test the Equality Case}.
Consider \(a = b = c = d = \frac{1}{2}\). Then:
\[
ab + bc + cd + da = 4\left(\frac{1}{2} \cdot \frac{1}{2}\right) = 1
\]

Compute the left-hand side:
\[
\sum_{\text{cyclic}} \frac{a^3}{b+c+d} = 4 \cdot \frac{\left(\frac{1}{2}\right)^3}{\frac{3}{2}} = 4 \cdot \frac{\frac{1}{8}}{\frac{3}{2}} = 4 \cdot \frac{1}{8} \cdot \frac{2}{3} = \frac{1}{3}
\]
This shows that equality holds when \(a = b = c = d = \frac{1}{2}\).

\emph{Step 6: Conclude the Proof}
Since the function \(f(x) = \frac{x^3}{S - x}\) is convex, the minimum of the sum occurs when all variables are equal, i.e., \(a = b = c = d\). Therefore, the inequality holds true:
\[
\frac{a^3}{b+c+d} + \frac{b^3}{c+d+a} + \frac{c^3}{d+a+b} + \frac{d^3}{a+b+c} \geq \frac{1}{3}.
\]

}
\end{tcolorbox}