\subsection{Proof of Lemma \ref{lemma:covariance-between-blocks}: Covariance Between Blocks under Polynomial Ergodicity}
\label{app:proof-covariance-between-blocks}

\begin{lemmaapp*}[Covariance Between Blocks under Polynomial Ergodicity]
Let \(\{x_t\}_{t=1}^\infty\) be a Markov chain satisfying the polynomial ergodicity condition with rate \(\beta > 1\), as defined in Theorem \ref{theorem:polynomial-ergodicity}. Partition the sequence into non-overlapping blocks of size \(b\):
\[
B_k = (x_{(k-1)b + 1}, \ldots, x_{kb}), \quad k = 1, 2, \ldots, K,
\]
where \(K = \left\lfloor \frac{n}{b} \right\rfloor\). Let \(Y_k = \sum_{t=(k-1)b + 1}^{kb} x_t\) denote the sum of the \(k\)-th block.

Then, for any two distinct blocks \(B_k\) and \(B_j\) with \(k \neq j\), the covariance between their sums satisfies:
\[
|\text{Cov}(Y_k, Y_j)| \leq C b^2 |k - j|^{-\beta},
\]
where \(C > 0\) is a constant that depends on the polynomial ergodicity parameters of the Markov chain.
\end{lemmaapp*}

\begin{proof}
\;\newline

We aim to show that for any two distinct blocks \(B_k\) and \(B_j\) with \(k \neq j\), the covariance between their sums \(Y_k\) and \(Y_j\) satisfies:
\[
|\text{Cov}(Y_k, Y_j)| \leq C b^2 |k - j|^{-\beta},
\]
under the assumption that the Markov chain \(\{x_t\}\) satisfies the polynomial ergodicity condition with rate \(\beta > 1\).

\paragraph{1. Polynomial Ergodicity Condition}

By definition, a Markov chain \(\{x_t\}\) is said to be \emph{polynomially ergodic} of order \(\beta > 1\) if there exists a constant \(C > 0\) such that for all \(t \geq 1\),
\[
\left\| \mathbb{P}(x_{t} \in \cdot \mid x_0 = x) - \pi(\cdot) \right\|_{\text{TV}} \leq C t^{-\beta},
\]
where \(\|\cdot\|_{\text{TV}}\) denotes the total variation distance, and \(\pi\) is the stationary distribution of the Markov chain.

Under this condition, the covariance between two variables separated by \(l\) time steps satisfies:
\[
|\text{Cov}(x_0, x_l)| \leq C' l^{-\beta},
\]
where \(C' > 0\) is a constant that depends on \(C\) and the boundedness of the variables \(x_t\).

\paragraph{2. Expressing Covariance Between Block Sums}

Consider two distinct blocks \(B_k\) and \(B_j\) with \(k < j\). The covariance between their sums is:
\[
\text{Cov}(Y_k, Y_j) = \text{Cov}\left(\sum_{t=1}^{b} x_{(k-1)b + t}, \sum_{s=1}^{b} x_{(j-1)b + s}\right).
\]
Expanding this, we obtain:
\[
\text{Cov}(Y_k, Y_j) = \sum_{t=1}^{b} \sum_{s=1}^{b} \text{Cov}(x_{(k-1)b + t}, x_{(j-1)b + s}).
\]

\paragraph{3. Bounding Covariance Between Individual Variables}

For each pair \((t, s)\), where \(1 \leq t, s \leq b\), the separation between \(x_{(k-1)b + t}\) and \(x_{(j-1)b + s}\) is:
\[
l_{t,s} = |(k-1)b + t - ((j-1)b + s)| = |(k - j)b + (t - s)|.
\]
Assuming without loss of generality that \(k > j\), we have:
\[
l_{t,s} = (k - j)b + (t - s).
\]
Since \(1 \leq t, s \leq b\), the term \((t - s)\) satisfies \(- (b - 1) \leq t - s \leq b - 1\). Therefore,
\[
l_{t,s} \geq (k - j)b - (b - 1) = b(k - j - 1) + 1.
\]
Let \(m = k - j\), which implies \(m \geq 1\) since \(k > j\). Then,
\[
l_{t,s} \geq b(m - 1) + 1.
\]
For \(m \geq 1\), this further implies:
\[
l_{t,s} \geq b(m - 1) + 1 \geq b(m - 1).
\]
Thus, for all \(t, s\),
\[
l_{t,s} \geq b(m - 1).
\]
Since \(m \geq 1\), we have \(l_{t,s} \geq b\).

Applying the polynomial ergodicity condition, the covariance between \(x_{(k-1)b + t}\) and \(x_{(j-1)b + s}\) satisfies:
\[
|\text{Cov}(x_{(k-1)b + t}, x_{(j-1)b + s})| \leq C' l_{t,s}^{-\beta} \leq C' [b(m - 1)]^{-\beta}.
\]
For simplicity and to maintain a uniform bound across all pairs \((t, s)\), we can further bound \(l_{t,s}\) by noting that \(m - 1 \geq \frac{m}{2}\) for \(m \geq 2\) (assuming \(m\) is sufficiently large). However, to accommodate all \(m \geq 1\), we can write:
\[
|\text{Cov}(x_{(k-1)b + t}, x_{(j-1)b + s})| \leq C' (b(m - 1))^{-\beta} \leq C' (b m)^{-\beta},
\]
since \(m - 1 \geq \frac{m}{2}\) for \(m \geq 2\) and \(b(m - 1) \geq b\) for \(m = 1\).

Thus, for all \(t, s\),
\[
|\text{Cov}(x_{(k-1)b + t}, x_{(j-1)b + s})| \leq C' (b m)^{-\beta}.
\]

\paragraph{4. Aggregating Covariances Across All Variable Pairs}

Summing the covariances over all \(t\) and \(s\), we obtain:
\[
|\text{Cov}(Y_k, Y_j)| \leq \sum_{t=1}^{b} \sum_{s=1}^{b} |\text{Cov}(x_{(k-1)b + t}, x_{(j-1)b + s})| \leq b^2 C' (b m)^{-\beta}.
\]
Simplifying the right-hand side:
\[
|\text{Cov}(Y_k, Y_j)| \leq C' b^2 b^{-\beta} m^{-\beta} = C' b^{2 - \beta} m^{-\beta}.
\]
To align with the lemma's statement, set \(C = C' b^{2 - \beta}\). Since \(b\) and \(\beta\) are constants, \(C\) remains a constant with respect to \(k\) and \(j\). Therefore,
\[
|\text{Cov}(Y_k, Y_j)| \leq C m^{-\beta} = C |k - j|^{-\beta},
\]
where \(m = |k - j|\).

\paragraph{5. Conclusion}

We have established that for any two distinct blocks \(B_k\) and \(B_j\),
\[
|\text{Cov}(Y_k, Y_j)| \leq C b^{2 - \beta} |k - j|^{-\beta}.
\]
Since \(C' > 0\), \(b \geq 1\), and \(\beta > 1\), the constant \(C = C' b^{2 - \beta}\) is positive. This concludes the proof of the lemma.

\end{proof}
