\begin{lstlisting}[language=json,numbers=none]
Original Answer:

To find the probability of the spinner landing on $C$, I need to subtract the probabilities of the spinner landing on $A$ and $B$ from $1$, since the sum of the probabilities of all possible outcomes is $1$. I can write this as an equation: $P(C) = 1 - P(A) - P(B)$. I know that $P(A) = \frac{1}{3}$ and $P(B) = \frac{5}{12}$, so I can plug those values into the equation and simplify. I get: $P(C) = 1 - \frac{1}{3} - \frac{5}{12} = \frac{12}{12} - \frac{4}{12} - \frac{5}{12} = \frac{3}{12}$. I can reduce this fraction by dividing the numerator and denominator by $3$, and I get: $P(C) = \frac{1}{4}$. 





















  
Scores:
SkyworkLlama:4.5312
SkyworkGemma:-1.2187
URM:9.8431
QRM:27.9685
Internlm2:2.0429
\end{lstlisting}