{\color{blue}Fix this and the parts that use this formula (in the main draft). 
The changes won't be too big, but I need to make things precise. 
}
\begin{proposition}\label{prop:induction_size}
    Let $\alpha_t = \alpha_1 t^{-a}$ with $a \in (0, 1)$.
    For any $0 < \alpha_1 \mu < 1$ and $n \geq 1$, 
    \begin{equation}
        \sum_{t=1}^n \frac{\alpha_t}{t} \prod_{j=t+1}^n \left(1 - \mu \alpha_j \right) 
            \leq {\color{red}K}\frac{\alpha_n}{n}
        % \frac{1}{1-a} \frac{\alpha_n}{n} \exp \left(-\mu \alpha_n\right) .
        % K_1 \alpha_n,
    \end{equation}
\end{proposition}

\begin{proof}
    This is shown by induction.
    The base case clearly holds, where $\prod_{j=n+1}^n (1 - \mu \alpha_j)$ is defined to be one. 
    Next,
    \begin{align*}
        \sum_{t=1}^n \frac{\alpha_t}{t} \prod_{j=t+1}^n \left(1 - \mu \alpha_j\right) 
        \leq 
        \frac{\alpha_n}{n} + {\color{red}K} \frac{\alpha_{n-1}}{n-1} .
    \end{align*}

    Using that $\alpha_t/\alpha_{t+1} = (1 + 1/t)^a \leq 2$ is a decreasing sequence, we have
    \begin{align*}
        \sum_{t=1}^n \frac{\alpha_t}{t} \prod_{j=t+1}^n \left(1 - \mu \alpha_j \right) 
        &= \alpha_{n+1} \sum_{t=1}^n \frac{1}{t}\frac{\alpha_{n}}{\alpha_{n+1}} \frac{\alpha_t}{\alpha_n} \prod_{j=t+1}^n \left(1 - \mu \alpha_j \right) 
        \\
        & \leq 2 \alpha_{n+1} \sum_{t=1}^n \frac{1}{t} \prod_{j=t+1}^n \frac{\alpha_j}{\alpha_{j+1}} \left(1 - \mu \alpha_j\right) .
    \end{align*}
    % Using Lemma 12 in \citep{kaledin2020finite}, we have that
    % Using $1 - x \leq \exp (-x)$, we have that 
    % \begin{align*}
    %     \prod_{j=t+1}^n (1 - \mu \alpha_j) 
    %     \leq 
    %     \exp \left(-\frac{\mu \alpha_1}{1-a} \left(
    %         n^{1-a} - (n-1)^{1-a}
    %         \right)
    %     \right)
    %     \leq 
    %     \exp \left(-\mu \alpha_{n-1} \right) ,
    % \end{align*}
    % where the last inequality uses $n^{1-a} - (n-1)^{1-a} \geq (1-a) (n-1)^{-a}$. 
    % Therefore,
    % \begin{align*}
    %     \sum_{t=1}^n \frac{\alpha_t}{t} \prod_{j=t+1}^n (1 - \mu \alpha_j) 
    %     \leq \exp \left(-\mu \alpha_{n-1}\right) \sum_{t=1}^n \frac{\alpha_t}{t} 
    %     \leq \frac{1}{1-a}\exp \left(-\mu \alpha_{n-1}\right) (n+1)^{1-a}.
    % \end{align*}
    
    % For $a < 1$, we have by $1 - x \leq \exp (-x)$ for all $x \in [0, 1]$,
    % \begin{align*}
    %     \prod_{j=t+1}^n (1 - \mu \alpha_j) \leq \exp \left(-\mu \alpha_1 (\sum_{j=t}^n j^{-a} - t^{-a})\right) 
    %     & \leq 
    %     \exp \left(-\frac{\mu \alpha_1}{1-a} 
    %         \left(n^{1-a} - t^{1-a} - 1 \right)
    %     + \mu \alpha_1 t^{-a}
    %     \right)
    %     \\ &
    %     = \exp \left(-\frac{\mu \alpha_1}{1-a}  (n^{1-a} - 2) \right) \exp \left( \frac{\mu \alpha_1}{1-a} t^{1-a}\right) .
    % \end{align*}
    % Next,
    % \begin{align*}
    %     \sum_{t=1}^n t^{-a-1} \exp \left(K_0 t^{1 - a} \right)
    %     % \leq K_1 \int_1^n t^{-a-1} \exp \left(K_0 t^{1-a}\right) dt
    %     \leq \left( \sum_{t=1}^n t^{-4}\right)^{1/2} \left(\sum_{t=1}^n t^{2(1 - a)} \exp \left(2 K_0 t^{1- a}\right)\right)^{1/2}
    % \end{align*}
    % {\color{red}First is $t^{-3/2}$, second is roughly $t^{1-a} \exp (K_0 t^{1-a})$ due to $x \exp x$ having an integral similar to a exp without the $x$.
    % Therefore, if the exponentials cancel out then we will have maybe something like $t^{1/2 - a}$ (if the 2 in the $t$ exponent remains, which gives after subtracting by $3/2$ the half); therefore, this may go to zero when $a > 1/2$, and may be where I need the requirement.  
    % But this wouldn't give $o(\alpha_n)$; need to make sure that whatever bound we get, we have a $o(\alpha_n)$, i.e. $t^{-a}$ times a decaying term. 
    % }


    % {\color{red}Case $a = 1$; may not be necessary.}
    % \begin{align*}
    %     \prod_{j=t+1}^n (1 - \mu \alpha_j ) 
    %         = 
    %     \prod_{j=t+1}^n \left(1 - \frac{\mu \alpha_1}{t}\right) 
    %         &\leq
    %     \exp \left(-\mu \alpha_1 (\log n - \log t)\right) \exp\left(\mu \alpha_1 + \alpha_t\right)          
    %     \\
    %     &        \leq
    %     \exp \left((\mu + 1) \alpha_1\right) \left(\frac{t}{n}\right)^{\mu \alpha_1} .
    %     % &
    %     % \leq \exp \left(-K_0 (\log n - \log t)\right)
    %     % = \left(\frac{t}{n}\right)^{K_0} .
    %     % \leq \left(\frac{2}{n}\right)^{\mu \alpha_1} .
    % \end{align*}
    % Therefore, there exists some constant $K_1 > 0$ such that
    % \begin{align*}
    %     \sum_{t=1}^n \frac{\alpha_t}{t} \prod_{j=t+1}^n \left(1 - \mu \alpha_1 \right) 
    %         \leq 
    %     \frac{\alpha_1 e^{(\mu + 1) \alpha_1}}{n^{\mu \alpha_1}} \sum_{t=1}^n t^{-a - 1 + \mu \alpha_1}
    %     \leq K_1 \frac{\alpha_1 e^{(\mu + 1)\alpha_1}}{\mu \alpha_1 - a} n^{-a} .
    % \end{align*}
    % {\color{red}Finish up!
    % Note that I need to strengthen the bound by, instead of using $a=1$ as the extreme case for the above bound, derive (and re-state for $a < 1$ instead of $a \leq 1$) a bound that decays at rate $o(\alpha_n)$. 
    % }


    % {\color{blue}A stronger bound for $a < 1$;}
    % \begin{align*}
    %     \prod_{j=t+1}^n 
    % \end{align*}
\end{proof}



% {\color{red}Lower bound:} Setting $\phi_j = j^{-a} \prod_{k=j+1}^t (1 - c k^{-a})$, we use $\log (1 - x) \geq - (x + x^2/2)$ for $x \in (0, 1)$ to get {\color{red}Check}
% \begin{align*}
%     \log \phi_j = -a \log j + \sum_{k=j+1}^t \log (1 - c k^{-a}) 
%     &\geq - a \log j - \sum_{k=j+1}^t (ck^{-a} + \frac{c^2}{2} k^{-2a}) 
%     \\ & 
%     \geq 
%     -a \log j - \frac{2 t^{1-a}}{1-a} + \frac{2 t^{1-2a}}{1 - 2a}
% \end{align*}


% \begin{proposition}\label{prop:fast_decay_steps}
%     If $\mu I \preceq A + A^T \preceq \nu I$ and $\alpha \leq 2 \mu/\nu^2$,
%     \begin{align*}
%         \lVert I - \alpha A \rVert \leq 1 - \frac{\mu}{2} \alpha .
%     \end{align*}
% \end{proposition}
% \begin{proof}
%     \begin{align*}
%         \lVert I - \alpha A \rVert^2 = \sup_{x \neq 0} \left\{1 - \alpha \frac{x^T (A^T + A) x}{\lVert x \rVert^2} + \alpha^2 \frac{x^T A^T A x}{\lVert x \rVert^2}\right\} 
%         \leq 
%         1 - \alpha \mu + \alpha^2 \frac{\nu^2}{4} ,
%     \end{align*}
%     where the last step uses that $\nu = \lVert A + A^T \rVert = 2 \lVert A \rVert$ to get $\lVert A^T A \rVert \leq \lVert A \rVert^2 \leq \nu^2/4$.
% \end{proof}

% Using $1 - x \leq e^{-x}$ for all $x \in [0, 1]$, $\alpha_k = t^{-a} $, and $\sum_{k=j+1}^t \alpha_k \leq \frac{t^{1-a}}{1-a} - \frac{j^{1-a}}{1-a}$, we have 
% \begin{align*}
%     \prod_{k=j+1}^t (1 - \alpha_k \frac{\mu_{ff}}{2}) 
%         &\leq \exp \left(-\frac{\mu_{ff}}{2(1-a)} \left(t^{-a+1} - (j+1)^{-a+1}\right) \right) .
% \end{align*}
% % Moreover, we use that $t^{-a+1} - (t-1)^{-a + 1} \leq \alpha_t$ {\color{red}Check! This is kind of like binomial expansion; or maybe this is related to the step-size condition?} to obtain that
% % \begin{align*}
% %     \prod_{k=j+1}^t (1 - \alpha_k \frac{\mu_{ff}}{2}) \leq \exp\left(-\mu j^{-a}\right) \leq \frac{1}{j \alpha_j}
% % \end{align*}
% {\color{red}Show below or faster rates; I think this is the correct rate based on expected results:
% Note that equality holds when $\alpha_t \approx t^{-1}$. Maybe show that this quantity is monotonic in the exponent.
% }
% \begin{align*}
%     \phi_{jt} = \alpha_j \prod_{k=j+1}^t \left(1 - \alpha_k \frac{\mu_{ff}}{2}\right) \leq \frac{1}{j} .
% \end{align*}
