\section{Connection between $\tilde{\beta}, \beta$ and $\bar{\alpha}$}
\label{app:sec:beta_connection}
From subsection \ref{subsec:fnp}, we have:
\begin{equation}
\label{eq:app:beta_tilde}
    s^{(t+1)}_{i_t} = \left(\sqrt{1 - \tilde{\beta}_{m_{i_t}^t}}\right) s^{(t)}_{i_t} + \left(\sqrt{\tilde{\beta}_{m_{i_t}^t}}\right) \epsilon^{(t)}
\end{equation}
    
And from subsection \ref{subsec:con_den}, we have:
\begin{equation}
\label{eq:app:beta}
    s^{(t, k+1)}_{i_t} = \left(\sqrt{1 - {\beta}(t, k)}\right) s^{(t, k)}_{i_t} + \left(\sqrt{{\beta}(t, k)}\right) \epsilon
\end{equation}

where $s^{(t, 0)}_{i_t} = s^{(t)}_{i_t}$ and $s^{(t, K_{i_t}^t)}_{i_t} = s^{(t+1)}_{i_t}$. Define ${\alpha}(t, k) = 1 - {\beta}(t, k)$. Then, we have:
$$
    s^{(t, k+1)}_{i_t} = \left(\sqrt{\prod_{k' = 0}^k{\alpha}(t, k')}\right) s^{(t, 0)}_{i_t} + \left(\sqrt{1 - {\prod_{k' = 0}^k{\alpha}(t, k')}}\right) \epsilon
$$
where we have merged the Gaussians. Setting $k = K_{i_t}^{t}-1$ and comparing \eqref{eq:app:beta_tilde} and \eqref{eq:app:beta}, we have:
\begin{align}\label{eq:beta_tilde}
    \tilde{\beta}_{m_{i_t}^t} &= 1 - {\prod_{k' = 0}^{K_{i_t}^t - 1}{\alpha}(t, k')}
\end{align}
Recall from subsection \ref{subsec:con_den} that:
\begin{equation}
\label{eq:app:alpha_bar}
    s^{(t, k+1)}_{i_t} = \left(\sqrt{\bar{\alpha}(t, k)}\right) s^{(0)}_{i_t} + \left(\sqrt{1 - \bar{\alpha}(t, k)}\right) \epsilon
\end{equation}
Again rewriting \eqref{eq:app:beta} by merging gaussians, we have:
$$
    s^{(t, k+1)}_{i_t} = \left(\sqrt{\prod_{t' = 0}^{t-1}\prod_{k' = 0}^{K_i^{t'}}{\alpha}(t', k') \prod_{k''=0}^k \alpha(t,k'')}\right) s^{(0, 0)}_{i_t} + \left(\sqrt{1 - {\prod_{t' = 0}^{t-1}\prod_{k' = 0}^{K_i^{t'}}{\alpha}(t', k') \prod_{k''=0}^k \alpha(t,k'')}}\right) \epsilon
$$
Comparing with \eqref{eq:app:alpha_bar}, we have:
\begin{align}
\label{eq:alpha_rel}
    {\bar{\alpha}(t, k)} = \prod_{t' = 0}^{t-1}\prod_{k' = 0}^{K_i^{t'}}{\alpha}(t', k') \prod_{k''=0}^k \alpha(t,k'')
\end{align}

\newpage