
\subsection{Extend Proof System: Peterson Algorithm}
\label{sec:petersoneg}
%
We now turn to our running example and try to complete the proof using the inference rules we have derived in the previous sections. 

\begin{lemma} For any thread \( A \), the following holds:
\[
    \vdash A\ \EntersCS\ \Implies\ A\ \Knows\ \neg (B\ \EntersCS)
\]
\end{lemma}

\begin{proof}
We proceed through the following steps using the extended proof system:

\begin{enumerate}

\item \textbf{Assumption Decomposition}:
Assume \( A\ \EntersCS \). By conjunction elimination (\(\land\)E):
\begin{align*}
    &1.\ (\lnot!\FlagOne \neq 1) \lor (\lnot!\Victim \neq 0) \\
    &2.\ A\ \Writes\ 1\ \To\ \FlagZero\ \HappensBefore\ A\ \Writes\ 0\ \To\ \Victim \\
    &3.\ \neg(A\ \Writes\ \FlagZero)\ \Since\ A\ \Writes\ 1\ \To\ \FlagZero \\
    &4.\ \neg(A\ \Writes\ \Victim)\ \Since\ A\ \Writes\ 0\ \To\ \Victim
\end{align*}

\item \textbf{Epistemic Foundation}:
When \( A\ \At\ \Label_6 \) (critical section entry):
\begin{proposition}[Local Knowledge]
\label{prop:local}
\[
A\ \At\ \Label_6\ \vdash\ A\ \Knows\ (!\FlagZero = 1\ \land\ !\Victim \neq 1 )
\]
\end{proposition}
\begin{proof}
Apply \(\textsc{=E}\) rule to \( A \)'s write operations, using:
\begin{itemize}
\item From \( A\ \Writes\ 1\ \To\ \FlagZero\ \), we know \( A\ \Knows\ A\ \Says\ !\FlagZero = 1 \)
\item From \( A\ \Writes\ 0\ \To\ \Victim \), we know \(A\ \Knows\ A\ \Says\ !\Victim = 0 \)
\end{itemize}
Since $!\FlagZero = 1$ and $!\Victim = 0$ are universally valid in $A$'s local context (no interference after writes), combining via \(\land\)I and \(\textsc{=EK}\) we can get the final result.
\end{proof}

\item \textbf{Temporal Constraints}:
From \( A\ \Writes\ 1\ \To\ \FlagZero\ \HappensBefore\ A\ \Writes\ 0\ \To\ \Victim \):
\[
A\ \Knows\ \left( B\ \Writes\ 1\ \To\ \FlagOne\ \HappensBefore\ B\ \Writes\ 1\ \To\ \Victim \right)
\]
Because, by the definition of $\HappensBefore$, $B$'s actions cannot interleave between $A$'s writes (fair scheduling). Combined with Proposition~\ref{prop:local}, this precludes \( B\ \EntersCS \).

\item \textbf{Final Derivation}:
Combine results from the previous steps and \(\textsc{T}\) axiom:
\[
A\ \Knows\ \neg(B\ \EntersCS)
\]
By \(\Implies\)-introduction:
\[
\vdash A\ \EntersCS\ \Implies\ A\ \Knows\ \neg(B\ \EntersCS)
\]
\end{enumerate}
\end{proof}





