\subsection{Proof of \cref{prop: adam solution}}
\label{subapp: proof of adam}
\begin{proof}
    From \cref{lemma: block diagonal simplification}, we have
    \begin{align*}
        &\Fnorm{\Ft-\mF}\\
        =& \sum_{i=1}^n \Fnorm{\mM_i} - 2\tr\left(\mM_i^T\E[\vg_i\vg_i^T]\right)\\
        =& \sum_{i=1}^n\sum_{j=1}^m M_{i,jj}^2 - 2M_{i,jj}\E[g_{i,j}^2]
    \end{align*}
    By taking the derivative w.r.t $M_{i,jj}$, we have
    \begin{align*}
        M_{i,jj} = \E[g_{i,j}^2]
    \end{align*}
    Thus, we have $\Ft = \diag(\E[\vecg^2])$.
\end{proof}