\begin{figure}
    \centering
\begin{tikzpicture}[scale=0.6,decoration={
    markings,
    mark=at position 0.50 with {\arrow{>}}}]
\begin{scope}[shift={(0,0)}]
%\draw[thin,yellow] (0,0) grid (9,5);
\draw[thick,dashed] (0,5) -- (9,5);
\draw[line width = 0.45mm, blue] (0,0) -- (9,0);

\draw[thick,postaction={decorate}] (0.75,0) .. controls (0.95,1) and (1.8,2) .. (2,2);
\draw[thick,postaction={decorate}] (3.25,0) .. controls (3.05,1) and (2.2,2) .. (2,2);
\node at (0.75,-0.35) {$b$};
\node at (3.25,-0.35) {$a-b$};

\draw[thick,postaction={decorate}] (5.75,0) .. controls (5.95,1) and (6.8,2) .. (7,2);
\draw[thick,postaction={decorate}] (8.25,0) .. controls (8.05,1) and (7.2,2) .. (7,2);
\node at (5.75,-0.35) {$b-a$};
\node at (8.25,-0.35) {$1-b$};

\draw[thick,postaction={decorate}] (2,2) .. controls (2.2,2.5) and (4.3,3.5) .. (4.5,3.5);
\draw[thick,postaction={decorate}] (7,2) .. controls (6.8,2.5) and (4.7,3.5) .. (4.5,3.5);
\node at (2.5,3) {$a$};
\node at (6.90,3) {$1-a$};

\draw[thick,postaction={decorate}] (4.5,3.5) -- (4.5,5);
\node at (5,4.15) {$1$};

\node at (10.5,2.5) {$=$};
\end{scope}

\begin{scope}[shift={(12.6,0)}]
%\draw[thin,yellow] (0,0) grid (9,5);

\node at (0.5,2.5) {$a\left[\dfrac{b}{a} \right]$};
\node at (2,2.5) {$+$};
\node at (4.5,2.5) {$(1-a)\left[ \dfrac{1-b}{1-a} \right]$};
\node at (7,2.5) {$+$};
\node at (8,2.5) {$\left[ a \right]$};

\draw[thick,fill] (9.1,2.5) arc (0:360:1.5mm);
\end{scope}

\begin{scope}[shift={(21.5,0)}]
%\draw[thin,yellow] (0,0) grid (2,5);

\draw[thick,dashed] (-9,5) -- (2.5,5);

\draw[line width = 0.45mm, blue] (-9,0) -- (2.5,0);

\draw[thick,postaction={decorate}] (1,0) -- (1,5);

\node at (1.5,2.5) {$1$};
\end{scope}

\end{tikzpicture}
    \caption{The three additive vertices are absorbed by the blue boundary wall, emitting three floating vertices with the weights $a\left[\dfrac{b}{a}\right]$, $(1-a)\left[\dfrac{1-b}{1-a}\right]$, and $[a]$. Since the floating vertices are additive, we can replace three floating vertices with one floating vertex with the label as the sum $a\left[\dfrac{b}{a}\right]+(1-a)\left[\dfrac{1-b}{1-a}\right] + [a] $.  }
    \label{fig5_016}
\end{figure}