\label{app:interactions}
\textbf{Fourier to M\"obius Coefficients:}
The M\"obius Coefficients, also referred to as the \emph{Harsanyi dividends}, can be recovered through \cite{saminger-platz_bases_2016}:
\begin{equation}
I^M(S) = (-2)^{|S|}\sum_{T\supseteq S}F(T).
\label{eq:mobius}
\end{equation}
\textbf{Fourier to Banzhaf Interaction Indices:} Banzhaf Interactions Indices \cite{roubens1996interaction} have a close relationship to Fourier coefficients. As shown in \cite{grabisch2000equivalent}:
\begin{equation}
    I^{BII}(S) = \sum_{T \supseteq S} \frac{2^{|S|}}{2^{|T|}}I^{M}(T).
\end{equation}
Using the relationship from Eq.~\ref{eq:mobius},
\begin{align}
    I^{BII}(S) &= \sum_{T \supseteq S} \frac{2^{|S|}}{2^{|T|}}(-2)^{|T|}\sum_{R \supseteq T}F(R) \\
    &= 2^{|S|}
    \sum_{\substack{T \supseteq S}} 
    (-1)^{|T|} \sum_{R \supseteq T}F(R)\\
    &= 2^{|S|}
    \sum_{\substack{R \supseteq S}} F(R)\sum_{S \subseteq T \subseteq R}
    (-1)^{|T|},\\
    &= (-2)^{|S|}F(S)
\end{align}
where the last line follows due to $\sum_{S \subseteq T \subseteq R}
    (-1)^{|T|}$ evaluating to 0 unless $R = S$.

When $S$ is a singleton, we recover the relationship between Fourier Coefficients and the Banzhaf Value $BV(i)$:
\begin{equation}
BV(i) = I^{BII}(\{i\}) = -2F(\{i\}).
\end{equation}

\textbf{Fourier to Shapley Interaction Indices:}
Shapley Interaction Indices \cite{GRABISCH1997167} are a generalization of Shapley values to interactions. Using the following relationship to M\"obius Coefficients \cite{grabisch2000equivalent}:
\begin{align}
    I^{SII}(S) &= \sum_{T \supseteq S} \frac{I^M(S)}{|T|-|S| + 1}\\
    &= \sum_{T \supseteq S} \sum_{R \supseteq T}\frac{(-2)^{|T|}F(R)}{|T|-|S| + 1}\\
    &= \sum_{R \supseteq S} F(R)\sum_{S \subseteq T \subseteq R}\frac{(-2)^{|T|}}{|T|-|S| + 1}\\
    &= \sum_{R \supseteq S} F(R)\sum_{j = |S|}^{|R|}\frac{(-2)^{j}}{j-|S| + 1 }\binom{|R| - |S|}{j - |S|}\\
    &= \sum_{R \supseteq S} F(R)\sum_{k=0}^{|R|-|S|}\frac{(-2)^{k+|S|}}{k + 1}\binom{|R| - |S|}{k}\\
    &= (-2)^{|S|}\sum_{R \supseteq S} F(R)\sum_{k=0}^{|R|-|S|}\frac{(-2)^{k}}{k + 1}\binom{|R| - |S|}{k}
\end{align}
Consider the following integral and an application of the binomial theorem:
\begin{align}
    \int_0^t (1+x)^{|R|-|S|}dx &=\int_0^t \sum_{k=0}^{|R|-|S|} \binom{|R| - |S|}{k} x^k  dx\\
    &= \sum_{k=0}^{|R|-|S|} \binom{|R| - |S|}{k} \int_0^t x^k  dx \\
    &= \sum_{k=0}^{|R|-|S|} \binom{|R| - |S|}{k} \left(\frac{t^{k+1}}{k+1}\right)
\end{align}
Evaluating at $t=-2$:
\begin{align}
\sum_{k=0}^{|R|-|S|} \binom{|R| - |S|}{k} \left(\frac{(-2)^{k}}{k+1}\right) &= -\frac{1}{2} \int_0^{-2} (1+x)^{|R|-|S|}dx\\
&= -\frac{1}{2}\cdot \frac{(-1)^{|R|-|S|+1}-1}{|R|-|S|+1}\\
&= \begin{cases}
			\frac{1}{|R|-|S|+1}, & \text{if Parity($|R|$) = Parity($|S|$) }\\
            0, & \text{otherwise}
		 \end{cases}
\end{align}
As a result, we find the relationship between Shapley Interaction Indices and Fourier Coefficients:
\begin{equation}
I^{SII}(S) = (-2)^{|S|}\sum_{\substack{R \supseteq S, \\ (-1)^{|R|} = (-1)^{|S|}}} \frac{F(R)}{|R|-|S|+1}.
\end{equation}

When $S$ is a singleton, we recover the relationship between Fourier Coefficients and the Shapley Value $SV(i)$:
\begin{equation}
SV(i) = I^{SII}(\{i\}) = (-2)\sum_{\substack{R \supseteq \{i\}, \\ |R| \text{ is odd}}} \frac{F(R)}{|R|}.
\end{equation}


\textbf{Fourier to Faith-Banzhaf Interaction Indices:} Faith-Banzhaf Interaction Indices \cite{tsai2023faith} of up to degree $\ell$ are the unique minimizer to the following regression objective: 
\begin{equation}
   \sum_{S \subseteq [n]}  \left(f(S) - \sum_{T \subseteq S, |T| \leq \ell} I^{FBII}(T,\ell) \right)^2. 
\end{equation}

Let $g(S)$ be the XOR polynomial up to degree $\ell$ that minimizes the regression objective. Appealing to Parseval's identity, 
\begin{equation}
   \sum_{S \subseteq [n]}  \left(f(S) - g(S)\right)^2 =    \sum_{S \subseteq [n]}  \left(F(S) - G(S)\right)^2 = \sum_{S\subseteq [n],|S| \leq \ell } \left(F(S) - G(S)\right)^2 + \sum_{S\subseteq [n],|S| > \ell } F(S)^2, 
\end{equation}
which is minimized when $G(S) = F(S)$ for $|S| \leq \ell$. Using Eq.~\ref{eq:mobius}, it can be seen that the Faith-Banzhaf Interaction Indices correspond to the M\"obius Coefficients of the function $f(S)$ truncated up to degree $\ell$:
\begin{equation}
       I^{FBII}(S,\ell) = (-2)^{|S|}\sum_{T\supseteq S, |T| \leq \ell}F(T).
\end{equation}


\textbf{Fourier to Faith-Shapley Interaction Indices:} Faith-Shapley Interaction Indices \cite{tsai2023faith} of up to degree $\ell$ have the following relationship to M\"obius Coefficients: 
\begin{align}
   I^{FSII}(S,\ell) &= I^M(S) + (-1)^{\ell - |S|} \frac{|S|}{\ell+|S|}\binom{\ell}{|S|}\sum_{T\supset S, |T|>\ell}\frac{\binom{|T|-1}{\ell}}{\binom{|T|+\ell -1}{\ell + |S|}} I^M(T) \\
   &= (-2)^{|S|}\sum_{T\supseteq S}F(T) + (-1)^{\ell - |S|} \frac{|S|}{\ell+|S|}\binom{\ell}{|S|}\sum_{T\supset S, |T|>\ell}\frac{\binom{|T|-1}{\ell}}{\binom{|T|+\ell -1}{\ell + |S|}} (-2)^{|T|}\sum_{R\supseteq T}F(R) \\
   &= (-2)^{|S|}\sum_{T\supseteq S}F(T) + (-1)^{\ell - |S|} \frac{|S|}{\ell+|S|}\binom{\ell}{|S|}\sum_{R\supset S, |R| > \ell }F(R) \sum_{S \subset T\subseteq R, |T|>\ell}\frac{\binom{|T|-1}{\ell}}{\binom{|T|+\ell -1}{\ell + |S|}} (-2)^{|T|}.
\end{align}



\textbf{Fourier to Shapley-Taylor Interaction Indices:}
Shapley-Taylor Interactions Indices \cite{dhamdhere2019shapley} of up to degree $\ell$ are related to M\"obius Coefficients in the following way:
\begin{equation}
    I^{STII}(S,\ell) = \begin{cases}
I^M(S), \quad \textnormal{if } |S| < \ell\\
\sum_{T \supseteq S} \binom{|T|}{\ell}^{-1}I^M(T), \quad \textnormal{if } |S| = \ell.
\end{cases}
\end{equation}

From an application of Eq.~\ref{eq:mobius},

\begin{equation}
    I^{STII}(S,\ell) = \begin{cases}
(-2)^{|S|}\sum_{T\supseteq S}F(T), \quad \textnormal{if } |S| < \ell\\
\sum_{T \supseteq S} \binom{|T|}{\ell}^{-1}(-2)^{|T|}\sum_{R\supseteq T}F(R), \quad \textnormal{if } |S| = \ell.
\end{cases}
\end{equation}
Simplifying the sum in the $|S|=\ell$ case:
\begin{align}
    \sum_{T \supseteq S} \binom{|T|}{\ell}^{-1}(-2)^{|T|}\sum_{R\supseteq T}F(R) &= \sum_{R \supseteq S}F(R)\sum_{S\subseteq T\subseteq R}\binom{|T|}{\ell}^{-1}(-2)^{|T|}\\
    &= \sum_{R \supseteq S}F(R)\sum_{k = \ell}^{|R|}\binom{k}{\ell}^{-1}(-2)^{k}\binom{|R|-\ell}{k-\ell}\\
\end{align}
Hence, 
\begin{equation}
    I^{STII}(S,\ell) = \begin{cases}
(-2)^{|S|}\sum_{T\supseteq S}F(T), \quad \textnormal{if } |S| < \ell\\
\sum_{T \supseteq S}F(T)\sum_{k = \ell}^{|T|}\binom{k}{\ell}^{-1}(-2)^{k}\binom{|T|-\ell}{k-\ell}, \quad \textnormal{if } |S| = \ell.
\end{cases}
\end{equation}